# §22.7 Landen Transformations

:::{note}
**See also:**

Annotations for Ch.22
:::


## §22.7(i) Descending Landen Transformation

:::{note}
**Keywords:**

[Jacobian elliptic functions](http://dlmf.nist.gov/search/search?q=Jacobian%20elliptic%20functions) , [Landen transformations](http://dlmf.nist.gov/search/search?q=Landen%20transformations) , [descending](http://dlmf.nist.gov/search/search?q=descending)

**Notes:**

See Lawden ([1989](./bib/L.html#bib1385 "Elliptic Functions and Applications"), pp. 79–80), Walker ([1996](./bib/W.html#bib2359 "Elliptic Functions. A Constructive Approach"), p. 148), Whittaker and Watson ([1927](./bib/W.html#bib2404 "A Course of Modern Analysis"), pp. 507–508).

**Referenced by:**

§22.17(ii) , §22.20(iii)

**See also:**

Annotations for §22.7 and Ch.22
:::

With


<a id="E1"></a>
$$
k_{1}=\frac{1-k^{\prime}}{1+k^{\prime}}, \tag{22.7.1}
$$


<a id="E2"></a>
$$
\operatorname{sn}\left(z,k\right)=\frac{(1+k_{1})\operatorname{sn}\left(z/(1+k_{1}),k_{1}\right)}{1+k_{1}{\operatorname{sn}}^{2}\left(z/(1+k_{1}),k_{1}\right)}, \tag{22.7.2}
$$


<a id="E3"></a>
$$
\operatorname{cn}\left(z,k\right)=\frac{\operatorname{cn}\left(z/(1+k_{1}),k_{1}\right)\operatorname{dn}\left(z/(1+k_{1}),k_{1}\right)}{1+k_{1}{\operatorname{sn}}^{2}\left(z/(1+k_{1}),k_{1}\right)}, \tag{22.7.3}
$$


<a id="E4"></a>
$$
\operatorname{dn}\left(z,k\right)=\frac{{\operatorname{dn}}^{2}\left(z/(1+k_{1}),k_{1}\right)-(1-k_{1})}{1+k_{1}-{\operatorname{dn}}^{2}\left(z/(1+k_{1}),k_{1}\right)}. \tag{22.7.4}
$$


## §22.7(ii) Ascending Landen Transformation

:::{note}
**Keywords:**

[Jacobian elliptic functions](http://dlmf.nist.gov/search/search?q=Jacobian%20elliptic%20functions) , [Landen transformations](http://dlmf.nist.gov/search/search?q=Landen%20transformations) , [ascending](http://dlmf.nist.gov/search/search?q=ascending)

**Notes:**

See Lawden ([1989](./bib/L.html#bib1385 "Elliptic Functions and Applications"), pp. 79–80), Walker ([1996](./bib/W.html#bib2359 "Elliptic Functions. A Constructive Approach"), p. 148), Whittaker and Watson ([1927](./bib/W.html#bib2404 "A Course of Modern Analysis"), pp. 507–508).

**Referenced by:**

§22.17(ii) , §22.20(iii)

**See also:**

Annotations for §22.7 and Ch.22
:::

With

<a id="E5"></a>

<a id="Ex1"></a>
$$
\displaystyle k_{2} \displaystyle=\frac{2\sqrt{k}}{1+k}, \tag{22.7.5}
$$

<a id="Ex2"></a>
$$
\displaystyle k_{2}^{\prime} \displaystyle=\frac{1-k}{1+k},
$$

:::{note}
**Defines:**

$k_{2}$ : change of variable (locally) and $k_{2}^{\prime}$ : change of variable (locally)

**Symbols:**

$k$: modulus

**A&S Ref:**

16.14.1

**See also:**

Annotations for §22.7(ii) , §22.7 and Ch.22
:::


<a id="E6"></a>
$$
\operatorname{sn}\left(z,k\right)=\frac{(1+k_{2}^{\prime})\operatorname{sn}\left(z/(1+k_{2}^{\prime}),k_{2}\right)\operatorname{cn}\left(z/(1+k_{2}^{\prime}),k_{2}\right)}{\operatorname{dn}\left(z/(1+k_{2}^{\prime}),k_{2}\right)}, \tag{22.7.6}
$$


<a id="E7"></a>
$$
\operatorname{cn}\left(z,k\right)=\frac{(1+k_{2}^{\prime})({\operatorname{dn}}^{2}\left(z/(1+k_{2}^{\prime}),k_{2}\right)-k_{2}^{\prime})}{k_{2}^{2}\operatorname{dn}\left(z/(1+k_{2}^{\prime}),k_{2}\right)}, \tag{22.7.7}
$$


<a id="E8"></a>
$$
\operatorname{dn}\left(z,k\right)=\frac{(1-k_{2}^{\prime})({\operatorname{dn}}^{2}\left(z/(1+k_{2}^{\prime}),k_{2}\right)+k_{2}^{\prime})}{k_{2}^{2}\operatorname{dn}\left(z/(1+k_{2}^{\prime}),k_{2}\right)}. \tag{22.7.8}
$$


## §22.7(iii) Generalized Landen Transformations

:::{note}
**Keywords:**

[Jacobian elliptic functions](http://dlmf.nist.gov/search/search?q=Jacobian%20elliptic%20functions) , [Landen transformations](http://dlmf.nist.gov/search/search?q=Landen%20transformations) , [generalized](http://dlmf.nist.gov/search/search?q=generalized)

**See also:**

Annotations for §22.7 and Ch.22
:::

See Khare and Sukhatme ([2004](./bib/K.html#bib1265 "Connecting Jacobi elliptic functions with different modulus parameters")).
