# ยง18.12 Generating Functions

:::{note}
**Keywords:**

[classical orthogonal polynomials](http://dlmf.nist.gov/search/search?q=classical%20orthogonal%20polynomials) , [generating functions](http://dlmf.nist.gov/search/search?q=generating%20functions)

**Notes:**

For ( 18.12.1 ) see Andrews et al. ([1999](./bib/index.html#bib103 "Special Functions"), (6.4.3)). For ( 18.12.2 ) see Bateman ([1905](./bib/B.html#bib215 "A generalisation of the Legendre polynomial"), pp. 113โ114) and Koornwinder ([1974](./bib/K.html#bib1322 "Jacobi polynomials. II. An analytic proof of the product formula"), p. 128). For ( 18.12.3 ) see Andrews et al. ([1999](./bib/index.html#bib103 "Special Functions"), (6.4.7)). For ( 18.12.4 ) see Szegล ([1975](./bib/S.html#bib2194 "Orthogonal Polynomials"), (4.7.23)). ( 18.12.5 ) follows by combining ( 18.12.4 ) and its $z$ -differentiated form. For ( 18.12.6 ) see Rainville ([1960](./bib/R.html#bib1921 "Special Functions"), ยง144, (7)). For ( 18.12.7 ) see Andrews et al. ([1999](./bib/index.html#bib103 "Special Functions"), (5.1.16)). ( 18.12.8 ) is an immediate consequence of ( 18.12.7 ). For ( 18.12.9 ) see Szegล ([1975](./bib/S.html#bib2194 "Orthogonal Polynomials"), (4.7.25)). ( 18.12.10 ) is the special case $\lambda=1$ of ( 18.12.4 ) in view of ( 18.7.4 ). ( 18.12.11 ) is the special case $\lambda=\frac{1}{2}$ of ( 18.12.4 ). ( 18.12.12 ) is the special case $\lambda=\frac{1}{2}$ of ( 18.12.6 ). For ( 18.12.13 ) see Andrews et al. ([1999](./bib/index.html#bib103 "Special Functions"), (6.2.4)). For ( 18.12.14 ) see Szegล ([1975](./bib/S.html#bib2194 "Orthogonal Polynomials"), (5.1.16)). For ( 18.12.15 ) see Andrews et al. ([1999](./bib/index.html#bib103 "Special Functions"), (6.1.7)).

**Referenced by:**

ยง18.10(iii) , Erratum (V1.2.0) ยง18.12

**Addition (effective with 1.2.0):**

Equations ( 18.12.2_5 ), ( 18.12.3_5 ), ( 18.12.17 ) were added.

**See also:**

Annotations for Ch.18
:::

The $z$ -radii of convergence will depend on $x$ , and in first instance we will assume $x\in[-1,1]$ for Jacobi, ultraspherical, Chebyshev and Legendre, $x\in[0,\infty)$ for Laguerre, and $x\in\mathbb{R}$ for Hermite. With the notation of ยงยง 10.2(ii) , 10.25(ii) , [15.2](./15.2.md "ยง15.2 Definitions and Analytical Properties โฃ Properties โฃ Chapter 15 Hypergeometric Function") , and [16.2](./16.2.md "ยง16.2 Definition and Analytic Properties โฃ Generalized Hypergeometric Functions โฃ Chapter 16 Generalized Hypergeometric Functions and Meijer ๐บ-Function") ,

:::{note}
**Keywords:**

[Jacobi polynomials](http://dlmf.nist.gov/search/search?q=Jacobi%20polynomials) , [generating functions](http://dlmf.nist.gov/search/search?q=generating%20functions)

**See also:**

Annotations for ยง18.12 and Ch.18
:::


<a id="E1"></a>
$$
\frac{2^{\alpha+\beta}}{R(1+R-z)^{\alpha}(1+R+z)^{\beta}}=\sum_{n=0}^{\infty}P^{(\alpha,\beta)}_{n}\left(x\right)z^{n}, \tag{18.12.1}
$$


<a id="E2"></a>
$$
{{}_{0}{\mathbf{F}}_{1}}\left({-\atop\alpha+1};\frac{(x-1)z}{2}\right)\*{{}_{0}{\mathbf{F}}_{1}}\left({-\atop\beta+1};\frac{(x+1)z}{2}\right)=\left(\tfrac{1}{2}(1-x)z\right)^{-\frac{1}{2}\alpha}J_{\alpha}\left(\sqrt{2(1-x)z}\right)\*\left(\tfrac{1}{2}(1+x)z\right)^{-\frac{1}{2}\beta}I_{\beta}\left(\sqrt{2(1+x)z}\right)=\sum_{n=0}^{\infty}\frac{P^{(\alpha,\beta)}_{n}\left(x\right)}{\Gamma\left(n+\alpha+1\right)\Gamma\left(n+\beta+1\right)}z^{n}, \tag{18.12.2}
$$


<a id="E2_5"></a>
$$
{{}_{2}F_{1}}\left({\gamma,\alpha+\beta+1-\gamma\atop\alpha+1};\frac{1-R-z}{2}\right)\*{{}_{2}F_{1}}\left({\gamma,\alpha+\beta+1-\gamma\atop\beta+1};\frac{1-R+z}{2}\right)=\sum_{n=0}^{\infty}\frac{{\left(\gamma\right)_{n}}{\left(\alpha+\beta+1-\gamma\right)_{n}}}{{\left(\alpha+1\right)_{n}}{\left(\beta+1\right)_{n}}}P^{(\alpha,\beta)}_{n}\left(x\right)z^{n}, \tag{18.12.2_5}
$$

with $\gamma$ arbitrary. Note that ( 18.12.2_5 ) yields ( 18.12.1 ) by putting $\gamma=0$ and ( 18.12.2 ) by replacing $z$ by $-\gamma^{-2}z$ and next letting $\gamma\to\infty$ .


<a id="E3"></a>
$$
(1+z)^{-\alpha-\beta-1}\*{{}_{2}F_{1}}\left({\tfrac{1}{2}(\alpha+\beta+1),\tfrac{1}{2}(\alpha+\beta+2)\atop\beta+1};\frac{2(x+1)z}{(1+z)^{2}}\right)=\sum_{n=0}^{\infty}\frac{{\left(\alpha+\beta+1\right)_{n}}}{{\left(\beta+1\right)_{n}}}P^{(\alpha,\beta)}_{n}\left(x\right)z^{n}, \tag{18.12.3}
$$


<a id="E3_5"></a>
$$
\frac{1+z}{(1-2xz+z^{2})^{\beta+\frac{3}{2}}}=\sum_{n=0}^{\infty}\frac{{\left(2\beta+2\right)_{n}}}{{\left(\beta+1\right)_{n}}}P^{(\beta+1,\beta)}_{n}\left(x\right)z^{n}, \tag{18.12.3_5}
$$

and similar formulas as ( 18.12.3 ) and ( 18.12.3_5 ) by symmetry; compare the second row in Table 18.6.1 . See Ismail ([2009](./bib/I.html#bib2902 "Classical and Quantum Orthogonal Polynomials in One Variable"), (4.3.2)) for another variant of ( 18.12.3 ).

:::{note}
**Keywords:**

[generating functions](http://dlmf.nist.gov/search/search?q=generating%20functions) , [ultraspherical polynomials](http://dlmf.nist.gov/search/search?q=ultraspherical%20polynomials)

**See also:**

Annotations for ยง18.12 and Ch.18
:::


<a id="E4"></a>
$$
(1-2xz+z^{2})^{-\lambda}=\sum_{n=0}^{\infty}C^{(\lambda)}_{n}\left(x\right)z^{n}=\sum_{n=0}^{\infty}\frac{{\left(2\lambda\right)_{n}}}{{\left(\lambda+\tfrac{1}{2}\right)_{n}}}P^{(\lambda-\frac{1}{2},\lambda-\frac{1}{2})}_{n}\left(x\right)z^{n}, \tag{18.12.4}
$$


<a id="E5"></a>
$$
\frac{1-xz}{(1-2xz+z^{2})^{\lambda+1}}=\sum_{n=0}^{\infty}\frac{n+2\lambda}{2\lambda}C^{(\lambda)}_{n}\left(x\right)z^{n}, \tag{18.12.5}
$$


<a id="E6"></a>
$$
\Gamma\left(\lambda+\tfrac{1}{2}\right){\mathrm{e}}^{z\cos\theta}(\tfrac{1}{2}z\sin\theta)^{\frac{1}{2}-\lambda}J_{\lambda-\frac{1}{2}}\left(z\sin\theta\right)=\sum_{n=0}^{\infty}\frac{C^{(\lambda)}_{n}\left(\cos\theta\right)}{{\left(2\lambda\right)_{n}}}z^{n}, \tag{18.12.6}
$$

:::{note}
**Keywords:**

[Chebyshev polynomials](http://dlmf.nist.gov/search/search?q=Chebyshev%20polynomials) , [generating functions](http://dlmf.nist.gov/search/search?q=generating%20functions)

**See also:**

Annotations for ยง18.12 and Ch.18
:::

<a id="EGx1"></a>

$$
\displaystyle\frac{1-z^{2}}{1-2xz+z^{2}} \displaystyle=1+2\sum_{n=1}^{\infty}T_{n}\left(x\right)z^{n}, \tag{18.12.7}
$$

:::{note}
**Symbols:**

$T_{\NVar{n}}\left(\NVar{x}\right)$: Chebyshev polynomial of the first kind , $z$: complex variable , $n$: nonnegative integer and $x$: real variable

**Referenced by:**

ยง18.12

**See also:**

Annotations for ยง18.12 , ยง18.12 and Ch.18
:::

$$
\displaystyle\frac{1-xz}{1-2xz+z^{2}} \displaystyle=\sum_{n=0}^{\infty}T_{n}\left(x\right)z^{n}, \tag{18.12.8}
$$

:::{note}
**Symbols:**

$T_{\NVar{n}}\left(\NVar{x}\right)$: Chebyshev polynomial of the first kind , $z$: complex variable , $n$: nonnegative integer and $x$: real variable

**A&S Ref:**

22.9.6

**Referenced by:**

ยง18.12

**See also:**

Annotations for ยง18.12 , ยง18.12 and Ch.18
:::


<a id="E9"></a>
$$
-\ln\left(1-2xz+z^{2}\right)=2\sum_{n=1}^{\infty}\frac{T_{n}\left(x\right)}{n}z^{n}, \tag{18.12.9}
$$


<a id="E10"></a>
$$
\frac{1}{1-2xz+z^{2}}=\sum_{n=0}^{\infty}U_{n}\left(x\right)z^{n}, \tag{18.12.10}
$$

:::{note}
**Keywords:**

[Legendre polynomials](http://dlmf.nist.gov/search/search?q=Legendre%20polynomials) , [generating functions](http://dlmf.nist.gov/search/search?q=generating%20functions)

**See also:**

Annotations for ยง18.12 and Ch.18
:::


<a id="E11"></a>
$$
\frac{1}{\sqrt{1-2xz+z^{2}}}=\sum_{n=0}^{\infty}P_{n}\left(x\right)z^{n}, \tag{18.12.11}
$$


<a id="E12"></a>
$$
{\mathrm{e}}^{xz}J_{0}\left(z\sqrt{1-x^{2}}\right)=\sum_{n=0}^{\infty}\frac{P_{n}\left(x\right)}{n!}z^{n}. \tag{18.12.12}
$$

:::{note}
**Keywords:**

[Laguerre polynomials](http://dlmf.nist.gov/search/search?q=Laguerre%20polynomials) , [generating functions](http://dlmf.nist.gov/search/search?q=generating%20functions)

**See also:**

Annotations for ยง18.12 and Ch.18
:::


<a id="E13"></a>
$$
(1-z)^{-\alpha-1}\exp\left(\frac{xz}{z-1}\right)=\sum_{n=0}^{\infty}L^{(\alpha)}_{n}\left(x\right)z^{n}, \tag{18.12.13}
$$


<a id="E14"></a>
$$
\Gamma\left(\alpha+1\right)(xz)^{-\frac{1}{2}\alpha}{\mathrm{e}}^{z}J_{\alpha}\left(2\sqrt{xz}\right)=\sum_{n=0}^{\infty}\frac{L^{(\alpha)}_{n}\left(x\right)}{{\left(\alpha+1\right)_{n}}}z^{n}. \tag{18.12.14}
$$

:::{note}
**Keywords:**

[Hermite polynomials](http://dlmf.nist.gov/search/search?q=Hermite%20polynomials) , [generating functions](http://dlmf.nist.gov/search/search?q=generating%20functions)

**See also:**

Annotations for ยง18.12 and Ch.18
:::


<a id="E15"></a>
$$
{\mathrm{e}}^{2xz-z^{2}}=\sum_{n=0}^{\infty}\frac{H_{n}\left(x\right)}{n!}z^{n}, \tag{18.12.15}
$$


<a id="E16"></a>
$$
{\mathrm{e}}^{xz-\frac{1}{2}z^{2}}=\sum_{n=0}^{\infty}\frac{\mathit{He}_{n}\left(x\right)}{n!}z^{n}, \tag{18.12.16}
$$


<a id="E17"></a>
$$
\frac{1+2xz+4z^{2}}{\left(1+4z^{2}\right)^{\frac{3}{2}}}\exp\left(\frac{4x^{2}z^{2}}{1+4z^{2}}\right)=\sum_{n=0}^{\infty}\frac{H_{n}\left(x\right)}{\left\lfloor n/2\right\rfloor!}z^{n}, \tag{18.12.17}
$$

See ยง 18.18(vii) for Poisson kernels; these are special cases of bilateral generating functions.
