# ยง18.23 Hahn Class: Generating Functions

:::{note}
**Keywords:**

[Hahn class orthogonal polynomials](http://dlmf.nist.gov/search/search?q=Hahn%20class%20orthogonal%20polynomials) , [generating functions](http://dlmf.nist.gov/search/search?q=generating%20functions)

**Notes:**

For ( 18.23.3 )โ( 18.23.5 ), ( 18.23.7 ) see Ismail ([2009](./bib/I.html#bib2902 "Classical and Quantum Orthogonal Polynomials in One Variable"), (6.2.43), (6.1.8), (6.1.22), (5.9.3)). ( 18.23.1 ) and ( 18.23.2 ) follow by expanding the factors on the left as power series in $z$ , and substituting ( 18.20.5 ) on the right. ( 18.23.6 ) is a limiting case of ( 18.26.18 ) via ( 18.26.6 ).

**See also:**

Annotations for Ch.18
:::

For the definition of generalized hypergeometric functions see ยง [16.2](./16.2.md "ยง16.2 Definition and Analytic Properties โฃ Generalized Hypergeometric Functions โฃ Chapter 16 Generalized Hypergeometric Functions and Meijer ๐บ-Function") .

:::{note}
**Keywords:**

[Hahn class orthogonal polynomials](http://dlmf.nist.gov/search/search?q=Hahn%20class%20orthogonal%20polynomials) , [confluent hypergeometric functions](http://dlmf.nist.gov/search/search?q=confluent%20hypergeometric%20functions) , [relations to other functions](http://dlmf.nist.gov/search/search?q=relations%20to%20other%20functions)

**See also:**

Annotations for ยง18.23 and Ch.18
:::


<a id="E1"></a>
$$
{{}_{1}F_{1}}\left({-x\atop\alpha+1};-z\right){{}_{1}F_{1}}\left({x-N\atop\beta+1};z\right)=\sum_{n=0}^{N}\frac{{\left(-N\right)_{n}}}{{\left(\beta+1\right)_{n}}n!}Q_{n}\left(x;\alpha,\beta,N\right)z^{n}, \tag{18.23.1}
$$


<a id="E2"></a>
$$
{{}_{2}F_{0}}\left({-x,-x+\beta+N+1\atop-};-z\right)\*{{}_{2}F_{0}}\left({x-N,x+\alpha+1\atop-};z\right)=\sum_{n=0}^{N}\frac{{\left(-N\right)_{n}}{\left(\alpha+1\right)_{n}}}{n!}Q_{n}\left(x;\alpha,\beta,N\right)z^{n}, \tag{18.23.2}
$$

:::{note}
**See also:**

Annotations for ยง18.23 and Ch.18
:::


<a id="E3"></a>
$$
\left(1-\frac{1-p}{p}z\right)^{x}(1+z)^{N-x}=\sum_{n=0}^{N}\genfrac{(}{)}{0.0pt}{}{N}{n}K_{n}\left(x;p,N\right)z^{n}, \tag{18.23.3}
$$

:::{note}
**See also:**

Annotations for ยง18.23 and Ch.18
:::


<a id="E4"></a>
$$
\left(1-\frac{z}{c}\right)^{x}(1-z)^{-x-\beta}=\sum_{n=0}^{\infty}\frac{{\left(\beta\right)_{n}}}{n!}M_{n}\left(x;\beta,c\right)z^{n}, \tag{18.23.4}
$$

:::{note}
**See also:**

Annotations for ยง18.23 and Ch.18
:::


<a id="E5"></a>
$$
{\mathrm{e}}^{z}\left(1-\frac{z}{a}\right)^{x}=\sum_{n=0}^{\infty}\frac{C_{n}\left(x;a\right)}{n!}z^{n}, \tag{18.23.5}
$$

:::{note}
**See also:**

Annotations for ยง18.23 and Ch.18
:::


<a id="E6"></a>
$$
{{}_{1}F_{1}}\left({a+\mathrm{i}x\atop 2\Re a};-\mathrm{i}z\right){{}_{1}F_{1}}\left({\overline{b}-\mathrm{i}x\atop 2\Re b};\mathrm{i}z\right)=\sum_{n=0}^{\infty}\frac{p_{n}\left(x;a,b,\overline{a},\overline{b}\right)}{{\left(2\Re a\right)_{n}}{\left(2\Re b\right)_{n}}}z^{n}. \tag{18.23.6}
$$

:::{note}
**See also:**

Annotations for ยง18.23 and Ch.18
:::


<a id="E7"></a>
$$
(1-{\mathrm{e}}^{\mathrm{i}\phi}z)^{-\lambda+\mathrm{i}x}(1-{\mathrm{e}}^{-\mathrm{i}\phi}z)^{-\lambda-\mathrm{i}x}=\sum_{n=0}^{\infty}P^{(\lambda)}_{n}\left(x;\phi\right)z^{n}, \tag{18.23.7}
$$
