# §19.18 Derivatives and Differential Equations

:::{note}
**See also:**

Annotations for Ch.19
:::


## §19.18(i) Derivatives

:::{note}
**Keywords:**

[derivative](http://dlmf.nist.gov/search/search?q=derivative) , [derivatives](http://dlmf.nist.gov/search/search?q=derivatives) , [hypergeometric $R$-function](http://dlmf.nist.gov/search/search?q=hypergeometric%20R-function) , [symmetric elliptic integrals](http://dlmf.nist.gov/search/search?q=symmetric%20elliptic%20integrals)

**Notes:**

( 19.18.1 ) is derived from ( 19.16.1 ), ( 19.16.5 ), and ( 19.18.4 ). ( 19.18.2 ) follows from ( 19.18.8 ). For ( 19.18.4 ) and ( 19.18.5 ) put $t=-a$ and $c=a+a^{\prime}$ in Carlson ([1977b](./bib/C.html#bib434 "Special Functions of Applied Mathematics"), (5.9-9), (5.9-10)).

**See also:**

Annotations for §19.18 and Ch.19
:::


<a id="E1"></a>
$$
\frac{\partial R_{F}\left(x,y,z\right)}{\partial z}=-\tfrac{1}{6}R_{D}\left(x,y,z\right), \tag{19.18.1}
$$


<a id="E2"></a>
$$
\frac{\mathrm{d}}{\mathrm{d}x}R_{G}\left(x+a,x+b,x+c\right)=\tfrac{1}{2}R_{F}\left(x+a,x+b,x+c\right). \tag{19.18.2}
$$

Let $\partial_{j}=\ifrac{\partial}{\partial z_{j}}$ , and $\mathbf{e}_{j}$ be an $n$ -tuple with 1 in the $j$ th place and 0’s elsewhere. Also define

<a id="E3"></a>

<a id="Ex1"></a>
$$
\displaystyle w_{j} \displaystyle=b_{j}\biggm{/}\sum_{j=1}^{n}b_{j}, \tag{19.18.3}
$$

<a id="Ex2"></a>
$$
\displaystyle a^{\prime} \displaystyle=-a+\sum_{j=1}^{n}b_{j}.
$$

:::{note}
**Symbols:**

$n$: nonnegative integer and $w_{j}$

**See also:**

Annotations for §19.18(i) , §19.18 and Ch.19
:::

The next two equations apply to ( 19.16.14 )–( 19.16.18 ) and ( 19.16.20 )–( 19.16.23 ).


<a id="E4"></a>
$$
\partial_{j}R_{-a}\left(\mathbf{b};\mathbf{z}\right)=-aw_{j}R_{-a-1}\left(\mathbf{b}+\mathbf{e}_{j};\mathbf{z}\right), \tag{19.18.4}
$$


<a id="E5"></a>
$$
(z_{j}\partial_{j}+b_{j})R_{-a}\left(\mathbf{b};\mathbf{z}\right)=w_{j}a^{\prime}R_{-a}\left(\mathbf{b}+\mathbf{e}_{j};\mathbf{z}\right). \tag{19.18.5}
$$


## §19.18(ii) Differential Equations

:::{note}
**Keywords:**

[Euler–Poisson differential equations](http://dlmf.nist.gov/search/search?q=Euler%E2%80%93Poisson%20differential%20equations) , [Euler–Poisson–Darboux equation](http://dlmf.nist.gov/search/search?q=Euler%E2%80%93Poisson%E2%80%93Darboux%20equation) , [Euler’s homogeneity relation](http://dlmf.nist.gov/search/search?q=Euler%20homogeneity%20relation) , [Laplace’s equation](http://dlmf.nist.gov/search/search?q=Laplace%20equation) , [axially symmetric potential theory](http://dlmf.nist.gov/search/search?q=axially%20symmetric%20potential%20theory) , [differential equation](http://dlmf.nist.gov/search/search?q=differential%20equation) , [differential equations](http://dlmf.nist.gov/search/search?q=differential%20equations) , [hypergeometric $R$-function](http://dlmf.nist.gov/search/search?q=hypergeometric%20R-function) , [potential theory](http://dlmf.nist.gov/search/search?q=potential%20theory) , [symmetric elliptic integrals](http://dlmf.nist.gov/search/search?q=symmetric%20elliptic%20integrals) , [wave equation](http://dlmf.nist.gov/search/search?q=wave%20equation)

**Notes:**

( 19.18.6 ) comes from ( 19.18.8 ) and ( 19.20.25 ). For ( 19.18.8 ) and ( 19.18.11 ) see Carlson ([1977b](./bib/C.html#bib434 "Special Functions of Applied Mathematics"), (5.9-2)). For ( 19.18.12 )–( 19.18.17 ) see Carlson ([1977b](./bib/C.html#bib434 "Special Functions of Applied Mathematics"), §5.4).

**See also:**

Annotations for §19.18 and Ch.19
:::


<a id="E6"></a>
$$
\left(\frac{\partial}{\partial x}+\frac{\partial}{\partial y}+\frac{\partial}{\partial z}\right)R_{F}\left(x,y,z\right)=\frac{-1}{2\sqrt{x}\sqrt{y}\sqrt{z}}, \tag{19.18.6}
$$


<a id="E7"></a>
$$
\left(\frac{\partial}{\partial x}+\frac{\partial}{\partial y}+\frac{\partial}{\partial z}\right)R_{G}\left(x,y,z\right)=\tfrac{1}{2}R_{F}\left(x,y,z\right). \tag{19.18.7}
$$


<a id="E8"></a>
$$
\sum_{j=1}^{n}\partial_{j}R_{-a}\left(\mathbf{b};\mathbf{z}\right)=-aR_{-a-1}\left(\mathbf{b};\mathbf{z}\right). \tag{19.18.8}
$$


<a id="E9"></a>
$$
\left(x\frac{\partial}{\partial x}+y\frac{\partial}{\partial y}+z\frac{\partial}{\partial z}\right)R_{F}\left(x,y,z\right)=-\tfrac{1}{2}R_{F}\left(x,y,z\right), \tag{19.18.9}
$$


<a id="E10"></a>
$$
\left((x-y)\frac{\,{\partial}^{2}}{\,\partial x\,\partial y}+\frac{1}{2}\left(\frac{\partial}{\partial y}-\frac{\partial}{\partial x}\right)\right)R_{F}\left(x,y,z\right)=0, \tag{19.18.10}
$$

and two similar equations obtained by permuting $x,y,z$ in ( 19.18.10 ).

More concisely, if $v=R_{-a}\left(\mathbf{b};\mathbf{z}\right)$ , then each of ( 19.16.14 )–( 19.16.18 ) and ( 19.16.20 )–( 19.16.23 ) satisfies *Euler’s homogeneity relation* :


<a id="E11"></a>
$$
\sum_{j=1}^{n}z_{j}\partial_{j}v=-av, \tag{19.18.11}
$$

and also a system of $n(n-1)/2$ *Euler–Poisson differential equations* (of which only $n-1$ are independent):


<a id="E12"></a>
$$
(z_{j}\partial_{j}+b_{j})\partial_{l}v=(z_{l}\partial_{l}+b_{l})\partial_{j}v, \tag{19.18.12}
$$

or equivalently,


<a id="E13"></a>
$$
((z_{j}-z_{l})\partial_{j}\partial_{l}+b_{j}\partial_{l}-b_{l}\partial_{j})v=0. \tag{19.18.13}
$$

Here $j,l=1,2,\dots,n$ and $j\neq l$ . For group-theoretical aspects of this system see Carlson ([1963](./bib/C.html#bib426 "Lauricella’s hypergeometric function F D"), §VI). If $n=2$ , then elimination of $\partial_{2}v$ between ( 19.18.11 ) and ( 19.18.12 ), followed by the substitution $(b_{1},b_{2},z_{1},z_{2})=(b,c-b,1-z,1)$ , produces the Gauss hypergeometric equation ( 15.10.1 ).

The next four differential equations apply to the complete case of $R_{F}$ and $R_{G}$ in the form $R_{-a}\left(\tfrac{1}{2},\tfrac{1}{2};z_{1},z_{2}\right)$ (see ( 19.16.20 ) and ( 19.16.23 )).

The function $w=R_{-a}\left(\tfrac{1}{2},\tfrac{1}{2};x+y,x-y\right)$ satisfies an *Euler–Poisson–Darboux equation* :


<a id="E14"></a>
$$
\frac{{\partial}^{2}w}{{\partial x}^{2}}=\frac{{\partial}^{2}w}{{\partial y}^{2}}+\frac{1}{y}\frac{\partial w}{\partial y}. \tag{19.18.14}
$$

Also $W=R_{-a}\left(\tfrac{1}{2},\tfrac{1}{2};t+r,t-r\right)$ , with $r=\sqrt{x^{2}+y^{2}}$ , satisfies a *wave equation* :


<a id="E15"></a>
$$
\frac{{\partial}^{2}W}{{\partial t}^{2}}=\frac{{\partial}^{2}W}{{\partial x}^{2}}+\frac{{\partial}^{2}W}{{\partial y}^{2}}. \tag{19.18.15}
$$

Similarly, the function $u=R_{-a}\left(\tfrac{1}{2},\tfrac{1}{2};x+iy,x-iy\right)$ satisfies an equation of *axially symmetric potential theory* :


<a id="E16"></a>
$$
\frac{{\partial}^{2}u}{{\partial x}^{2}}+\frac{{\partial}^{2}u}{{\partial y}^{2}}+\frac{1}{y}\frac{\partial u}{\partial y}=0, \tag{19.18.16}
$$

and $U=R_{-a}\left(\tfrac{1}{2},\tfrac{1}{2};z+i\rho,z-i\rho\right)$ , with $\rho=\sqrt{x^{2}+y^{2}}$ , satisfies *Laplace’s equation* :


<a id="E17"></a>
$$
\frac{{\partial}^{2}U}{{\partial x}^{2}}+\frac{{\partial}^{2}U}{{\partial y}^{2}}+\frac{{\partial}^{2}U}{{\partial z}^{2}}=0. \tag{19.18.17}
$$
