# §19.22 Quadratic Transformations

:::{note}
**See also:**

Annotations for Ch.19
:::


## §19.22(i) Complete Integrals

:::{note}
**Notes:**

In ( 19.22.18 ), ( 19.22.21 ), and ( 19.22.20 ), put $z=0$ to obtain ( 19.22.1 ), ( 19.22.2 ), and ( 19.22.4 ), respectively. ( 19.22.3 ) is derivable from ( 19.22.2 ) and ( 19.21.3 ), or more directly by putting $p=y$ in ( 19.22.7 ). For ( 19.22.7 ) see Carlson ([1976](./bib/C.html#bib432 "Quadratic transformations of Appell functions"), (4.14), (4.13)), where $(\pi/4)R_{L}(y,z,p)=R_{F}\left(0,y,z\right)-(p/3)R_{J}\left(0,y,z,p\right)$ .

**Referenced by:**

§19.22(ii) , §19.22(iii)

**See also:**

Annotations for §19.22 and Ch.19
:::

Let $\Re x>0$ , $\Re y>0$ , $a=(x+y)/2$ , and $p\neq 0$ . Then

<a id="EGx1"></a>

$$
\displaystyle R_{F}\left(0,x^{2},y^{2}\right) \displaystyle=R_{F}\left(0,xy,a^{2}\right), \tag{19.22.1}
$$

:::{note}
**Symbols:**

$R_{F}\left(\NVar{x},\NVar{y},\NVar{z}\right)$: symmetric elliptic integral of first kind

**Referenced by:**

§19.22(i) , §19.28

**See also:**

Annotations for §19.22(i) , §19.22 and Ch.19
:::

$$
\displaystyle 2R_{G}\left(0,x^{2},y^{2}\right) \displaystyle=4R_{G}\left(0,xy,a^{2}\right)-xyR_{F}\left(0,xy,a^{2}\right), \tag{19.22.2}
$$

:::{note}
**Symbols:**

$R_{F}\left(\NVar{x},\NVar{y},\NVar{z}\right)$: symmetric elliptic integral of first kind and $R_{G}\left(\NVar{x},\NVar{y},\NVar{z}\right)$: symmetric elliptic integral of second kind

**Referenced by:**

§19.22(i)

**See also:**

Annotations for §19.22(i) , §19.22 and Ch.19
:::

$$
\displaystyle 2y^{2}R_{D}\left(0,x^{2},y^{2}\right) \displaystyle=\tfrac{1}{4}(y^{2}-x^{2})R_{D}\left(0,xy,a^{2}\right)+3R_{F}\left(0,xy,a^{2}\right). \tag{19.22.3}
$$

:::{note}
**Symbols:**

$R_{D}\left(\NVar{x},\NVar{y},\NVar{z}\right)$: elliptic integral symmetric in only two variables and $R_{F}\left(\NVar{x},\NVar{y},\NVar{z}\right)$: symmetric elliptic integral of first kind

**Referenced by:**

§19.22(i) , §19.22(i) , §19.22(iii)

**See also:**

Annotations for §19.22(i) , §19.22 and Ch.19
:::


<a id="E4"></a>
$$
(p_{\pm}^{2}-p_{\mp}^{2})R_{J}\left(0,x^{2},y^{2},p^{2}\right)=2(p_{\pm}^{2}-a^{2})R_{J}\left(0,xy,a^{2},p_{\pm}^{2}\right)-3R_{F}\left(0,xy,a^{2}\right)+3\pi/(2p), \tag{19.22.4}
$$

where


<a id="E5"></a>
$$
2p_{\pm}=\sqrt{(p+x)(p+y)}\pm\sqrt{(p-x)(p-y)}, \tag{19.22.5}
$$

and hence

<a id="E6"></a>

<a id="Ex1"></a>
$$
\displaystyle p_{+}p_{-} \displaystyle=pa, \tag{19.22.6}
$$

<a id="Ex2"></a>
$$
\displaystyle p_{+}^{2}+p_{-}^{2} \displaystyle=p^{2}+xy,
$$

<a id="Ex3"></a>
$$
\displaystyle p_{+}^{2}-p_{-}^{2} \displaystyle=\sqrt{(p^{2}-x^{2})(p^{2}-y^{2})},
$$

<a id="Ex4"></a>
$$
\displaystyle 4(p_{\pm}^{2}-a^{2}) \displaystyle=(\sqrt{p^{2}-x^{2}}\pm\sqrt{p^{2}-y^{2}})^{2}.
$$

:::{note}
**Symbols:**

$p_{\pm}$: modified parameter

**Referenced by:**

§19.22(iii)

**See also:**

Annotations for §19.22(i) , §19.22 and Ch.19
:::


### Bartky’s Transformation

:::{note}
**Keywords:**

[Bartky’s transformation](http://dlmf.nist.gov/search/search?q=Bartky%20transformation) , [symmetric elliptic integrals](http://dlmf.nist.gov/search/search?q=symmetric%20elliptic%20integrals)

**See also:**

Annotations for §19.22(i) , §19.22 and Ch.19
:::


<a id="E7"></a>
$$
2p^{2}R_{J}\left(0,x^{2},y^{2},p^{2}\right)=v_{+}v_{-}R_{J}\left(0,xy,a^{2},v^{2}_{+}\right)+3R_{F}\left(0,xy,a^{2}\right), \tag{19.22.7}
$$

If $p=y$ , then ( 19.22.7 ) reduces to ( 19.22.3 ), but if $p=x$ or $p=y$ , then both sides of ( 19.22.4 ) are 0 by ( 19.20.9 ). If $x<p<y$ or $y<p<x$ , then $p_{+}$ and $p_{-}$ are complex conjugates.


## §19.22(ii) Gauss’s Arithmetic-Geometric Mean (AGM)

:::{note}
**Keywords:**

[arithmetic-geometric mean](http://dlmf.nist.gov/search/search?q=arithmetic-geometric%20mean) , [symmetric elliptic integrals](http://dlmf.nist.gov/search/search?q=symmetric%20elliptic%20integrals)

**Notes:**

The formulas in § 19.22(ii) come from iterating those in § 19.22(i) . See ( 19.16.20 ), ( 19.16.23 ), and Carlson ([2002](./bib/C.html#bib444 "Three improvements in reduction and computation of elliptic integrals"), Section 2).

**Referenced by:**

§15.17(iv) , §19.22(ii) , §19.36(ii)

**See also:**

Annotations for §19.22 and Ch.19
:::

The AGM, $M\left(a_{0},g_{0}\right)$ , of two positive numbers $a_{0}$ and $g_{0}$ is defined in § 19.8(i) . Again, we assume that $a_{0}\geq g_{0}$ (except in ( 19.22.10 )), and define $c_{n}=\sqrt{a_{n}^{2}-g_{n}^{2}}$ . Then


<a id="E8"></a>
$$
\frac{2}{\pi}R_{F}\left(0,a_{0}^{2},g_{0}^{2}\right)=\frac{1}{M\left(a_{0},g_{0}\right)}, \tag{19.22.8}
$$


<a id="E9"></a>
$$
\frac{4}{\pi}R_{G}\left(0,a_{0}^{2},g_{0}^{2}\right)=\frac{1}{M\left(a_{0},g_{0}\right)}\left(a_{0}^{2}-\sum_{n=0}^{\infty}2^{n-1}c_{n}^{2}\right)=\frac{1}{M\left(a_{0},g_{0}\right)}\left(a_{1}^{2}-\sum_{n=2}^{\infty}2^{n-1}c_{n}^{2}\right), \tag{19.22.9}
$$

and


<a id="E10"></a>
$$
R_{D}\left(0,g_{0}^{2},a_{0}^{2}\right)=\frac{3\pi}{4M\left(a_{0},g_{0}\right)a_{0}^{2}}\sum_{n=0}^{\infty}Q_{n}, \tag{19.22.10}
$$

where

<a id="E11"></a>

<a id="Ex5"></a>
$$
\displaystyle Q_{0} \displaystyle=1, \tag{19.22.11}
$$

<a id="Ex6"></a>
$$
\displaystyle Q_{n+1} \displaystyle=\tfrac{1}{2}Q_{n}\frac{a_{n}-g_{n}}{a_{n}+g_{n}}.
$$

:::{note}
**Symbols:**

$n$: nonnegative integer , $Q_{n}$ , $a_{n}$: iterate and $g_{n}$: iterate

**Referenced by:**

§19.22(ii)

**See also:**

Annotations for §19.22(ii) , §19.22 and Ch.19
:::

$Q_{n}$ has the same sign as $a_{0}-g_{0}$ for $n\geq 1$ .


<a id="E12"></a>
$$
R_{J}\left(0,g_{0}^{2},a_{0}^{2},p_{0}^{2}\right)=\frac{3\pi}{4M\left(a_{0},g_{0}\right)p_{0}^{2}}\sum_{n=0}^{\infty}Q_{n}, \tag{19.22.12}
$$

where $p_{0}>0$ and

<a id="E13"></a>

<a id="Ex7"></a>
$$
\displaystyle p_{n+1} \displaystyle=\frac{p_{n}^{2}+a_{n}g_{n}}{2p_{n}}, \tag{19.22.13}
$$

<a id="Ex8"></a>
$$
\displaystyle\varepsilon_{n} \displaystyle=\frac{p_{n}^{2}-a_{n}g_{n}}{p_{n}^{2}+a_{n}g_{n}},
$$

<a id="Ex9"></a>
$$
\displaystyle Q_{0} \displaystyle=1,
$$

<a id="Ex10"></a>
$$
\displaystyle Q_{n+1} \displaystyle=\tfrac{1}{2}Q_{n}\varepsilon_{n}.
$$

:::{note}
**Symbols:**

$n$: nonnegative integer , $Q_{n}$ , $\varepsilon_{n}$ , $p_{j}$: coefficient , $a_{n}$: iterate and $g_{n}$: iterate

**Referenced by:**

§19.22(ii)

**See also:**

Annotations for §19.22(ii) , §19.22 and Ch.19
:::

(If $p_{0}=a_{0}$ , then $p_{n}=a_{n}$ and ( 19.22.13 ) reduces to ( 19.22.11 ).) As $n\to\infty$ , $p_{n}$ and $\varepsilon_{n}$ converge quadratically to $M\left(a_{0},g_{0}\right)$ and 0, respectively, and $Q_{n}$ converges to 0 faster than quadratically. If the last variable of $R_{J}$ is negative, then the Cauchy principal value is


<a id="E14"></a>
$$
R_{J}\left(0,g_{0}^{2},a_{0}^{2},-q_{0}^{2}\right)=\frac{-3\pi}{4M\left(a_{0},g_{0}\right)(q_{0}^{2}+a_{0}^{2})}\*\left(2+\frac{a_{0}^{2}-g_{0}^{2}}{q_{0}^{2}+g_{0}^{2}}\sum_{n=0}^{\infty}Q_{n}\right), \tag{19.22.14}
$$

and ( 19.22.13 ) still applies, provided that


<a id="E15"></a>
$$
p_{0}^{2}=a_{0}^{2}(q_{0}^{2}+g_{0}^{2})/(q_{0}^{2}+a_{0}^{2}). \tag{19.22.15}
$$


## §19.22(iii) Incomplete Integrals

:::{note}
**Keywords:**

[Gauss transformations](http://dlmf.nist.gov/search/search?q=Gauss%20transformations) , [Landen transformations](http://dlmf.nist.gov/search/search?q=Landen%20transformations) , [symmetric elliptic integrals](http://dlmf.nist.gov/search/search?q=symmetric%20elliptic%20integrals) , [transformations replaced by symmetry](http://dlmf.nist.gov/search/search?q=transformations%20replaced%20by%20symmetry)

**Notes:**

For ( 19.22.18 ) see Carlson ([1964](./bib/C.html#bib427 "Normal elliptic integrals of the first and second kinds"), (5.13)). For ( 19.22.19 ) put $p=z$ in ( 19.22.20 ). For ( 19.22.20 ) see Zill and Carlson ([1970](./bib/Z.html#bib2498 "Symmetric elliptic integrals of the third kind"), (5.7)) and Carlson ([1990](./bib/C.html#bib440 "Landen Transformations of Integrals"), (8.5)). For ( 19.22.21 ) see Carlson ([1964](./bib/C.html#bib427 "Normal elliptic integrals of the first and second kinds"), (5.16)). For ( 19.22.22 ) put $z=y$ in ( 19.22.18 ). In the ascending Landen case let $k^{2}=(z_{+}^{2}-z_{-}^{2})/(z_{+}^{2}-a^{2})$ and $k_{1}^{2}=(z^{2}-y^{2})/(z^{2}-x^{2})$ to get the second equation in ( 19.8.11 ). In the descending Gauss case let $k_{1}^{2}=(a^{2}-z_{-}^{2})/(a^{2}-z_{+}^{2})$ and $k^{2}=(z^{2}-y^{2})/(z^{2}-x^{2})$ to get the first equation in ( 19.8.11 ).

**Referenced by:**

§19.22(iii)

**See also:**

Annotations for §19.22 and Ch.19
:::

Let $x$ , $y$ , and $z$ have positive real parts, assume $p\neq 0$ , and retain ( 19.22.5 ) and ( 19.22.6 ). Define

<a id="E16"></a>

<a id="Ex11"></a>
$$
\displaystyle a \displaystyle=(x+y)/2, \tag{19.22.16}
$$

<a id="Ex12"></a>
$$
\displaystyle 2z_{\pm} \displaystyle=\sqrt{(z+x)(z+y)}\pm\sqrt{(z-x)(z-y)},
$$

:::{note}
**Referenced by:**

§19.22(iii) , §19.36(ii)

**See also:**

Annotations for §19.22(iii) , §19.22 and Ch.19
:::

so that

<a id="E17"></a>

<a id="Ex13"></a>
$$
\displaystyle z_{+}z_{-} \displaystyle=za, \tag{19.22.17}
$$

<a id="Ex14"></a>
$$
\displaystyle z_{+}^{2}+z_{-}^{2} \displaystyle=z^{2}+xy,
$$

<a id="Ex15"></a>
$$
\displaystyle z_{+}^{2}-z_{-}^{2} \displaystyle=\sqrt{(z^{2}-x^{2})(z^{2}-y^{2})},
$$

<a id="Ex16"></a>
$$
\displaystyle 4(z_{\pm}^{2}-a^{2}) \displaystyle=(\sqrt{z^{2}-x^{2}}\pm\sqrt{z^{2}-y^{2}})^{2}.
$$

:::{note}
**Referenced by:**

§19.36(ii)

**See also:**

Annotations for §19.22(iii) , §19.22 and Ch.19
:::

Then


<a id="E18"></a>
$$
R_{F}\left(x^{2},y^{2},z^{2}\right)=R_{F}\left(a^{2},z_{-}^{2},z_{+}^{2}\right), \tag{19.22.18}
$$


<a id="E19"></a>
$$
(z_{\pm}^{2}-z_{\mp}^{2})R_{D}\left(x^{2},y^{2},z^{2}\right)={2(z_{\pm}^{2}-a^{2})}R_{D}\left(a^{2},z_{\mp}^{2},z_{\pm}^{2}\right)-3R_{F}\left(x^{2},y^{2},z^{2}\right)+(3/z), \tag{19.22.19}
$$


<a id="E20"></a>
$$
(p_{\pm}^{2}-p_{\mp}^{2})R_{J}\left(x^{2},y^{2},z^{2},p^{2}\right)=2(p_{\pm}^{2}-a^{2})R_{J}\left(a^{2},z_{+}^{2},z_{-}^{2},p_{\pm}^{2}\right)-3R_{F}\left(x^{2},y^{2},z^{2}\right)+3R_{C}\left(z^{2},p^{2}\right), \tag{19.22.20}
$$


<a id="E21"></a>
$$
2R_{G}\left(x^{2},y^{2},z^{2}\right)=4R_{G}\left(a^{2},z_{+}^{2},z_{-}^{2}\right)-xyR_{F}\left(x^{2},y^{2},z^{2}\right)-z, \tag{19.22.21}
$$


<a id="E22"></a>
$$
R_{C}\left(x^{2},y^{2}\right)=R_{C}\left(a^{2},ay\right). \tag{19.22.22}
$$

If $x,y,z$ are real and positive, then ( 19.22.18 )–( 19.22.21 ) are ascending Landen transformations when $x,y<z$ (implying $a<z_{-}<z_{+}$ ), and descending Gauss transformations when $z<x,y$ (implying $z_{+}<z_{-}<a$ ). Ascent and descent correspond respectively to increase and decrease of $k$ in Legendre’s notation. Descending Gauss transformations include, as special cases, transformations of complete integrals into complete integrals; ascending Landen transformations do not.

If $p=x$ or $p=y$ , then ( 19.22.20 ) reduces to $0=0$ by ( 19.20.13 ), and if $z=x$ or $z=y$ then ( 19.22.19 ) reduces to $0=0$ by ( 19.20.20 ) and ( 19.22.22 ). If $x<z<y$ or $y<z<x$ , then $z_{+}$ and $z_{-}$ are complex conjugates. However, if $x$ and $y$ are complex conjugates and $z$ and $p$ are real, then the right-hand sides of all transformations in §§ 19.22(i) and 19.22(iii) —except ( 19.22.3 ) and ( 19.22.22 )—are free of complex numbers and $p_{\pm}^{2}-p_{\mp}^{2}=\pm|p^{2}-x^{2}|\neq 0$ .

The transformations inverse to the ones just described are the descending Landen transformations and the ascending Gauss transformations. The equations inverse to ( 19.22.5 ) and ( 19.22.16 ) are given by

<a id="E23"></a>

<a id="Ex17"></a>
$$
\displaystyle x+y \displaystyle=2a, \tag{19.22.23}
$$

<a id="Ex18"></a>
$$
\displaystyle x-y \displaystyle=(\ifrac{2}{a})\sqrt{(a^{2}-z_{+}^{2})(a^{2}-z_{-}^{2})},
$$

<a id="Ex19"></a>
$$
\displaystyle z \displaystyle=\ifrac{z_{+}z_{-}}{a},
$$

:::{note}
**See also:**

Annotations for §19.22(iii) , §19.22 and Ch.19
:::

and the corresponding equations with $z$ , $z_{+}$ , and $z_{-}$ replaced by $p$ , $p_{+}$ , and $p_{-}$ , respectively. These relations need to be used with caution because $y$ is negative when $0<a<z_{+}z_{-}\left(z_{+}^{2}+z_{-}^{2}\right)^{-1/2}$ .
