# §20.4 Values at z = 0

:::{note}
**Keywords:**

[derivatives](http://dlmf.nist.gov/search/search?q=derivatives) , [theta functions](http://dlmf.nist.gov/search/search?q=theta%20functions) , [values at $z=0$](http://dlmf.nist.gov/search/search?q=values%20at%20z%3D0)

**See also:**

Annotations for Ch.20
:::


## §20.4(i) Functions and First Derivatives

:::{note}
**Notes:**

See Walker ([1996](./bib/W.html#bib2359 "Elliptic Functions. A Constructive Approach"), pp. 90–92), Whittaker and Watson ([1927](./bib/W.html#bib2404 "A Course of Modern Analysis"), pp. 470–471), and Lawden ([1989](./bib/L.html#bib1385 "Elliptic Functions and Applications"), pp. 12–15). Note that these are special cases of ( 20.5.1 )–( 20.5.4 ).

**See also:**

Annotations for §20.4 and Ch.20
:::


<a id="E1"></a>
$$
\theta_{1}\left(0,q\right)=\theta_{2}'\left(0,q\right)=\theta_{3}'\left(0,q\right)=\theta_{4}'\left(0,q\right)=0, \tag{20.4.1}
$$

<a id="EGx1"></a>

$$
\displaystyle\theta_{1}'\left(0,q\right) \displaystyle=2q^{1/4}\prod_{n=1}^{\infty}\left(1-q^{2n}\right)^{3}=2q^{1/4}{\left(q^{2};q^{2}\right)_{\infty}}^{3}, \tag{20.4.2}
$$

:::{note}
**Symbols:**

$\theta_{\NVar{j}}\left(\NVar{z},\NVar{q}\right)$: theta function , $\left(\NVar{a};\NVar{q}\right)_{\NVar{n}}$: $q$-Pochhammer symbol (or $q$-shifted factorial) , $n$: integer and $q$: nome

**Referenced by:**

Erratum (V1.0.28) for Equation (20.4.2)

**Addition (effective with 1.0.28):**

The representation in terms of ${\left(q^{2};q^{2}\right)_{\infty}}^{3}$ was added to this equation.

**See also:**

Annotations for §20.4(i) , §20.4 and Ch.20
:::

$$
\displaystyle\theta_{2}\left(0,q\right) \displaystyle=2q^{1/4}\prod\limits_{n=1}^{\infty}\left(1-q^{2n}\right)\left(1+q^{2n}\right)^{2}, \tag{20.4.3}
$$

:::{note}
**Symbols:**

$\theta_{\NVar{j}}\left(\NVar{z},\NVar{q}\right)$: theta function , $n$: integer and $q$: nome

**Referenced by:**

(20.10.3)

**See also:**

Annotations for §20.4(i) , §20.4 and Ch.20
:::

$$
\displaystyle\theta_{3}\left(0,q\right) \displaystyle=\prod\limits_{n=1}^{\infty}\left(1-q^{2n}\right)\left(1+q^{2n-1}\right)^{2}, \tag{20.4.4}
$$

:::{note}
**Symbols:**

$\theta_{\NVar{j}}\left(\NVar{z},\NVar{q}\right)$: theta function , $n$: integer and $q$: nome

**Referenced by:**

(20.10.2)

**See also:**

Annotations for §20.4(i) , §20.4 and Ch.20
:::

$$
\displaystyle\theta_{4}\left(0,q\right) \displaystyle=\prod\limits_{n=1}^{\infty}\left(1-q^{2n}\right)\left(1-q^{2n-1}\right)^{2}. \tag{20.4.5}
$$

:::{note}
**Symbols:**

$\theta_{\NVar{j}}\left(\NVar{z},\NVar{q}\right)$: theta function , $n$: integer and $q$: nome

**Referenced by:**

(20.10.1)

**See also:**

Annotations for §20.4(i) , §20.4 and Ch.20
:::


### Jacobi’s Identity

:::{note}
**Keywords:**

[Jacobi’s identity](http://dlmf.nist.gov/search/search?q=Jacobi%20identity) , [Jacobi’s triple product](http://dlmf.nist.gov/search/search?q=Jacobi%20triple%20product) , [theta functions](http://dlmf.nist.gov/search/search?q=theta%20functions)

**See also:**

Annotations for §20.4(i) , §20.4 and Ch.20
:::


<a id="E6"></a>
$$
\theta_{1}'\left(0,q\right)=\theta_{2}\left(0,q\right)\theta_{3}\left(0,q\right)\theta_{4}\left(0,q\right). \tag{20.4.6}
$$


## §20.4(ii) Higher Derivatives

:::{note}
**Keywords:**

[theta functions](http://dlmf.nist.gov/search/search?q=theta%20functions) , [values at $z=0$](http://dlmf.nist.gov/search/search?q=values%20at%20z%3D0)

**Notes:**

See Whittaker and Watson ([1927](./bib/W.html#bib2404 "A Course of Modern Analysis"), p. 471).

**See also:**

Annotations for §20.4 and Ch.20
:::


<a id="E7"></a>
$$
\theta_{1}''\left(0,q\right)=\theta_{2}'''\left(0,q\right)=\theta_{3}'''\left(0,q\right)=\theta_{4}'''\left(0,q\right)=0. \tag{20.4.7}
$$

<a id="EGx2"></a>

$$
\displaystyle\frac{\theta_{1}'''\left(0,q\right)}{\theta_{1}'\left(0,q\right)} \displaystyle=-1+24\sum_{n=1}^{\infty}\frac{q^{2n}}{(1-q^{2n})^{2}}. \tag{20.4.8}
$$

:::{note}
**Symbols:**

$\theta_{\NVar{j}}\left(\NVar{z},\NVar{q}\right)$: theta function , $n$: integer and $q$: nome

**Referenced by:**

§23.12

**See also:**

Annotations for §20.4(ii) , §20.4 and Ch.20
:::

$$
\displaystyle\frac{\theta_{2}''\left(0,q\right)}{\theta_{2}\left(0,q\right)} \displaystyle=-1-8\sum_{n=1}^{\infty}\frac{q^{2n}}{(1+q^{2n})^{2}}, \tag{20.4.9}
$$

:::{note}
**Symbols:**

$\theta_{\NVar{j}}\left(\NVar{z},\NVar{q}\right)$: theta function , $n$: integer and $q$: nome

**See also:**

Annotations for §20.4(ii) , §20.4 and Ch.20
:::

$$
\displaystyle\frac{\theta_{3}''\left(0,q\right)}{\theta_{3}\left(0,q\right)} \displaystyle=-8\sum_{n=1}^{\infty}\frac{q^{2n-1}}{(1+q^{2n-1})^{2}}, \tag{20.4.10}
$$

:::{note}
**Symbols:**

$\theta_{\NVar{j}}\left(\NVar{z},\NVar{q}\right)$: theta function , $n$: integer and $q$: nome

**See also:**

Annotations for §20.4(ii) , §20.4 and Ch.20
:::

$$
\displaystyle\frac{\theta_{4}''\left(0,q\right)}{\theta_{4}\left(0,q\right)} \displaystyle=8\sum_{n=1}^{\infty}\frac{q^{2n-1}}{(1-q^{2n-1})^{2}}. \tag{20.4.11}
$$

:::{note}
**Symbols:**

$\theta_{\NVar{j}}\left(\NVar{z},\NVar{q}\right)$: theta function , $n$: integer and $q$: nome

**See also:**

Annotations for §20.4(ii) , §20.4 and Ch.20
:::


<a id="E12"></a>
$$
\frac{\theta_{1}'''\left(0,q\right)}{\theta_{1}'\left(0,q\right)}=\frac{\theta_{2}''\left(0,q\right)}{\theta_{2}\left(0,q\right)}+\frac{\theta_{3}''\left(0,q\right)}{\theta_{3}\left(0,q\right)}+\frac{\theta_{4}''\left(0,q\right)}{\theta_{4}\left(0,q\right)}. \tag{20.4.12}
$$
