# §3.4 Differentiation

:::{note}
**Referenced by:**

§3.3(v)

**See also:**

Annotations for Ch.3
:::


## §3.4(i) Equally-Spaced Nodes

:::{note}
**Keywords:**

[Lagrange’s formula for equally-spaced nodes](http://dlmf.nist.gov/search/search?q=Lagrange%20formula%20for%20equally-spaced%20nodes) , [differentiation](http://dlmf.nist.gov/search/search?q=differentiation) , [numerical](http://dlmf.nist.gov/search/search?q=numerical)

**Notes:**

See Hildebrand ([1974](./bib/H.html#bib1077 "Introduction to Numerical Analysis"), pp. 85–89). The coefficients $B_{k}^{n}$ are obtained by differentiation of the $A_{k}^{n}$ ; compare ( 3.4.2 ).

**See also:**

Annotations for §3.4 and Ch.3
:::

The Lagrange $(n+1)$ -point formula is


<a id="E1"></a>
$$
hf^{\prime}_{t}=hf^{\prime}(x_{0}+th)=\sum_{k=n_{0}}^{n_{1}}B_{k}^{n}f_{k}+hR^{\prime}_{n,t}, \tag{3.4.1}
$$

and follows from the differentiated form of ( 3.3.4 ). The $B_{k}^{n}$ are the *differentiated Lagrangian interpolation coefficients* :


<a id="E2"></a>
$$
B_{k}^{n}=\ifrac{\mathrm{d}A_{k}^{n}}{\mathrm{d}t}, \tag{3.4.2}
$$

where $A_{k}^{n}$ is as in ( 3.3.10 ).

If $f^{(n+2)}(x)$ is continuous on the interval $I$ defined in § 3.3(i) , then the remainder in ( 3.4.1 ) is given by


<a id="E3"></a>
$$
hR^{\prime}_{n,t}=\frac{h^{n+1}}{(n+1)!}\left(f^{(n+1)}(\xi_{0})\frac{\mathrm{d}}{\mathrm{d}t}\prod_{k=n_{0}}^{n_{1}}(t-k)+f^{(n+2)}(\xi_{1})\prod_{k=n_{0}}^{n_{1}}(t-k)\right), \tag{3.4.3}
$$

where $\xi_{0}$ and $\xi_{1}\in I$ .

For the values of $n_{0}$ and $n_{1}$ used in the formulas below


<a id="E4"></a>
$$
h\left|R^{\prime}_{n,t}\right|\leq h^{n+1}\left(c_{n}\left|f^{(n+2)}(\xi_{1})\right|+\frac{1}{n+1}\left|f^{(n+1)}(\xi_{0})\right|\right), \tag{3.4.4}
$$

where $c_{n}$ is defined by ( 3.3.12 ), with numerical values as in § 3.3(ii) .


### Two-Point Formula

:::{note}
**See also:**

Annotations for §3.4(i) , §3.4 and Ch.3
:::


<a id="E5"></a>
$$
hf^{\prime}_{t}=-f_{0}+f_{1}+hR^{\prime}_{1,t}, \tag{3.4.5}
$$


### Three-Point Formula

:::{note}
**See also:**

Annotations for §3.4(i) , §3.4 and Ch.3
:::


<a id="E6"></a>
$$
hf^{\prime}_{t}=-\tfrac{1}{2}(1-2t)f_{-1}-2tf_{0}+\tfrac{1}{2}(1+2t)f_{1}+hR^{\prime}_{2,t}, \tag{3.4.6}
$$


### Four-Point Formula

:::{note}
**See also:**

Annotations for §3.4(i) , §3.4 and Ch.3
:::


<a id="E7"></a>
$$
hf^{\prime}_{t}=\sum_{k=-1}^{2}B_{k}^{3}f_{k}+hR^{\prime}_{3,t}, \tag{3.4.7}
$$

<a id="E8"></a>

<a id="Ex1"></a>
$$
\displaystyle B_{-1}^{3} \displaystyle=-\tfrac{1}{6}(2-6t+3t^{2}), \tag{3.4.8}
$$

<a id="Ex2"></a>
$$
\displaystyle B_{0}^{3} \displaystyle=-\tfrac{1}{2}(1+4t-3t^{2}),
$$

<a id="Ex3"></a>
$$
\displaystyle B_{1}^{3} \displaystyle=\tfrac{1}{2}(2+2t-3t^{2}),
$$

<a id="Ex4"></a>
$$
\displaystyle B_{2}^{3} \displaystyle=-\tfrac{1}{6}(1-3t^{2}).
$$

:::{note}
**Symbols:**

$B_{k}^{n}$: differentiated Lagrangian interpolation coefficients

**See also:**

Annotations for §3.4(i) , §3.4(i) , §3.4 and Ch.3
:::


### Five-Point Formula

:::{note}
**See also:**

Annotations for §3.4(i) , §3.4 and Ch.3
:::


<a id="E9"></a>
$$
hf^{\prime}_{t}=\sum_{k=-2}^{2}B_{k}^{4}f_{k}+hR^{\prime}_{4,t}, \tag{3.4.9}
$$

<a id="E10"></a>

<a id="Ex5"></a>
$$
\displaystyle B_{-2}^{4} \displaystyle=\tfrac{1}{12}(1-t-3t^{2}+2t^{3}), \tag{3.4.10}
$$

<a id="Ex6"></a>
$$
\displaystyle B_{-1}^{4} \displaystyle=-\tfrac{1}{6}(4-8t-3t^{2}+4t^{3}),
$$

<a id="Ex7"></a>
$$
\displaystyle B_{0}^{4} \displaystyle=-\tfrac{1}{2}t(5-2t^{2}),
$$

<a id="Ex8"></a>
$$
\displaystyle B_{1}^{4} \displaystyle=\tfrac{1}{6}(4+8t-3t^{2}-4t^{3}),
$$

<a id="Ex9"></a>
$$
\displaystyle B_{2}^{4} \displaystyle=-\tfrac{1}{12}(1+t-3t^{2}-2t^{3}).
$$

:::{note}
**Symbols:**

$B_{k}^{n}$: differentiated Lagrangian interpolation coefficients

**See also:**

Annotations for §3.4(i) , §3.4(i) , §3.4 and Ch.3
:::


### Six-Point Formula

:::{note}
**See also:**

Annotations for §3.4(i) , §3.4 and Ch.3
:::


<a id="E11"></a>
$$
hf^{\prime}_{t}=\sum_{k=-2}^{3}B_{k}^{5}f_{k}+hR^{\prime}_{5,t}, \tag{3.4.11}
$$

<a id="E12"></a>

<a id="Ex10"></a>
$$
\displaystyle B_{-2}^{5} \displaystyle=\tfrac{1}{120}(6-10t-15t^{2}+20t^{3}-5t^{4}), \tag{3.4.12}
$$

<a id="Ex11"></a>
$$
\displaystyle B_{-1}^{5} \displaystyle=-\tfrac{1}{24}(12-32t+3t^{2}+16t^{3}-5t^{4}),
$$

<a id="Ex12"></a>
$$
\displaystyle B_{0}^{5} \displaystyle=-\tfrac{1}{12}(4+30t-15t^{2}-12t^{3}+5t^{4}),
$$

<a id="Ex13"></a>
$$
\displaystyle B_{1}^{5} \displaystyle=\tfrac{1}{12}(12+16t-21t^{2}-8t^{3}+5t^{4}),
$$

<a id="Ex14"></a>
$$
\displaystyle B_{2}^{5} \displaystyle=-\tfrac{1}{24}(6+2t-21t^{2}-4t^{3}+5t^{4}),
$$

<a id="Ex15"></a>
$$
\displaystyle B_{3}^{5} \displaystyle=\tfrac{1}{120}(4-15t^{2}+5t^{4}).
$$

:::{note}
**Symbols:**

$B_{k}^{n}$: differentiated Lagrangian interpolation coefficients

**See also:**

Annotations for §3.4(i) , §3.4(i) , §3.4 and Ch.3
:::


### Seven-Point Formula

:::{note}
**See also:**

Annotations for §3.4(i) , §3.4 and Ch.3
:::


<a id="E13"></a>
$$
hf^{\prime}_{t}=\sum_{k=-3}^{3}B_{k}^{6}f_{k}+hR^{\prime}_{6,t}, \tag{3.4.13}
$$

<a id="E14"></a>

<a id="Ex16"></a>
$$
\displaystyle B_{-3}^{6} \displaystyle=-\tfrac{1}{720}(12-8t-45t^{2}+20t^{3}+15t^{4}-6t^{5}), \tag{3.4.14}
$$

<a id="Ex17"></a>
$$
\displaystyle B_{-2}^{6} \displaystyle=\tfrac{1}{60}(9-9t-30t^{2}+20t^{3}+5t^{4}-3t^{5}),
$$

<a id="Ex18"></a>
$$
\displaystyle B_{-1}^{6} \displaystyle=-\tfrac{1}{48}(36-72t-39t^{2}+52t^{3}+5t^{4}-6t^{5}),
$$

<a id="Ex19"></a>
$$
\displaystyle B_{0}^{6} \displaystyle=-\tfrac{1}{18}t(49-28t^{2}+3t^{4}),
$$

<a id="Ex20"></a>
$$
\displaystyle B_{1}^{6} \displaystyle=\tfrac{1}{48}(36+72t-39t^{2}-52t^{3}+5t^{4}+6t^{5}),
$$

<a id="Ex21"></a>
$$
\displaystyle B_{2}^{6} \displaystyle=-\tfrac{1}{60}(9+9t-30t^{2}-20t^{3}+5t^{4}+3t^{5}),
$$

<a id="Ex22"></a>
$$
\displaystyle B_{3}^{6} \displaystyle=\tfrac{1}{720}(12+8t-45t^{2}-20t^{3}+15t^{4}+6t^{5}).
$$

:::{note}
**Symbols:**

$B_{k}^{n}$: differentiated Lagrangian interpolation coefficients

**See also:**

Annotations for §3.4(i) , §3.4(i) , §3.4 and Ch.3
:::


### Eight-Point Formula

:::{note}
**Keywords:**

[Lagrange’s formula for equally-spaced nodes](http://dlmf.nist.gov/search/search?q=Lagrange%20formula%20for%20equally-spaced%20nodes) , [differentiation](http://dlmf.nist.gov/search/search?q=differentiation) , [numerical](http://dlmf.nist.gov/search/search?q=numerical)

**See also:**

Annotations for §3.4(i) , §3.4 and Ch.3
:::


<a id="E15"></a>
$$
hf^{\prime}_{t}=\sum_{k=-3}^{4}B_{k}^{7}f_{k}+hR^{\prime}_{7,t}, \tag{3.4.15}
$$

<a id="E16"></a>

<a id="Ex23"></a>
$$
\displaystyle B_{-3}^{7} \displaystyle=-\tfrac{1}{5040}(48-56t-168t^{2}+140t^{3}+35t^{4}-42t^{5}+7t^{6}), \tag{3.4.16}
$$

<a id="Ex24"></a>
$$
\displaystyle B_{-2}^{7} \displaystyle=\tfrac{1}{720}(72-108t-213t^{2}+240t^{3}-10t^{4}-36t^{5}+7t^{6}),
$$

<a id="Ex25"></a>
$$
\displaystyle B_{-1}^{7} \displaystyle=-\tfrac{1}{240}(144-360t-48t^{2}+260t^{3}-45t^{4}-30t^{5}+7t^{6}),
$$

<a id="Ex26"></a>
$$
\displaystyle B_{0}^{7} \displaystyle=-\tfrac{1}{144}(36+392t-147t^{2}-224t^{3}+70t^{4}+24t^{5}-7t^{6}),
$$

<a id="Ex27"></a>
$$
\displaystyle B_{1}^{7} \displaystyle=\tfrac{1}{144}(144+216t-264t^{2}-156t^{3}+85t^{4}+18t^{5}-7t^{6}),
$$

<a id="Ex28"></a>
$$
\displaystyle B_{2}^{7} \displaystyle=-\tfrac{1}{240}(72+36t-267t^{2}-80t^{3}+90t^{4}+12t^{5}-7t^{6}),
$$

<a id="Ex29"></a>
$$
\displaystyle B_{3}^{7} \displaystyle=\tfrac{1}{720}(48+8t-192t^{2}-20t^{3}+85t^{4}+6t^{5}-7t^{6}),
$$

<a id="Ex30"></a>
$$
\displaystyle B_{4}^{7} \displaystyle=-\tfrac{1}{5040}(36-147t^{2}+70t^{4}-7t^{6}).
$$

:::{note}
**Symbols:**

$B_{k}^{n}$: differentiated Lagrangian interpolation coefficients

**See also:**

Annotations for §3.4(i) , §3.4(i) , §3.4 and Ch.3
:::

For corresponding formulas for second, third, and fourth derivatives, with $t=0$ , see Collatz ([1960](./bib/C.html#bib559 "The Numerical Treatment of Differential Equations"), Table III, pp. 538–539). For formulas for derivatives with equally-spaced real nodes and based on Sinc approximations (§ 3.3(vi) ), see Stenger ([1993](./bib/S.html#bib2171 "Numerical Methods Based on Sinc and Analytic Functions"), §3.5).


## §3.4(ii) Analytic Functions

:::{note}
**Keywords:**

[analytic functions](http://dlmf.nist.gov/search/search?q=analytic%20functions) , [differentiation](http://dlmf.nist.gov/search/search?q=differentiation) , [numerical](http://dlmf.nist.gov/search/search?q=numerical)

**See also:**

Annotations for §3.4 and Ch.3
:::

If $f$ can be extended analytically into the complex plane, then from Cauchy’s integral formula (§ 1.9(iii) )


<a id="E17"></a>
$$
\frac{1}{k!}\,f^{(k)}(x_{0})=\frac{1}{2\pi i}\int_{C}\frac{f(\zeta)}{(\zeta-x_{0})^{k+1}}\,\,\mathrm{d}\zeta, \tag{3.4.17}
$$

where $C$ is a simple closed contour described in the positive rotational sense such that $C$ and its interior lie in the domain of analyticity of $f$ , and $x_{0}$ is interior to $C$ . Taking $C$ to be a circle of radius $r$ centered at $x_{0}$ , we obtain


<a id="E18"></a>
$$
\frac{1}{k!}\,f^{(k)}(x_{0})=\frac{1}{2\pi r^{k}}\int_{0}^{2\pi}f(x_{0}+re^{i\theta})e^{-ik\theta}\,\mathrm{d}\theta. \tag{3.4.18}
$$

The integral on the right-hand side can be approximated by the composite trapezoidal rule ( 3.5.2 ).


### Example

:::{note}
**See also:**

Annotations for §3.4(ii) , §3.4 and Ch.3
:::

$f(z)=e^{z}$ , $x_{0}=0$ . The integral ( 3.4.18 ) becomes


<a id="E19"></a>
$$
\frac{1}{k!}=\frac{1}{2\pi r^{k}}\int_{0}^{2\pi}e^{r\cos\theta}\cos\left(r\sin\theta-k\theta\right)\,\mathrm{d}\theta. \tag{3.4.19}
$$

With the choice $r=k$ (which is crucial when $k$ is large because of numerical cancellation) the integrand equals $e^{k}$ at the dominant points $\theta=0,2\pi$ , and in combination with the factor $k^{-k}$ in front of the integral sign this gives a rough approximation to $1/k!$ . The choice $r=k$ is motivated by saddle-point analysis; see § 2.4(iv) or examples in § 3.5(ix) . As explained in §§ 3.5(i) and 3.5(ix) the composite trapezoidal rule can be very efficient for computing integrals with analytic periodic integrands.


## §3.4(iii) Partial Derivatives

:::{note}
**Keywords:**

[differentiation](http://dlmf.nist.gov/search/search?q=differentiation) , [numerical](http://dlmf.nist.gov/search/search?q=numerical) , [partial derivatives](http://dlmf.nist.gov/search/search?q=partial%20derivatives)

**See also:**

Annotations for §3.4 and Ch.3
:::


### First-Order

:::{note}
**See also:**

Annotations for §3.4(iii) , §3.4 and Ch.3
:::

For partial derivatives we use the notation $u_{t,s}=u(x_{0}+th,y_{0}+sh)$ .


<a id="E20"></a>
$$
\frac{\partial u_{0,0}}{\partial x}=\frac{1}{2h}\,(u_{1,0}-u_{-1,0})+O\left(h^{2}\right), \tag{3.4.20}
$$


<a id="E21"></a>
$$
\frac{\partial u_{0,0}}{\partial x}=\frac{1}{4h}\,(u_{1,1}-u_{-1,1}+u_{1,-1}-u_{-1,-1})+O\left(h^{2}\right). \tag{3.4.21}
$$


### Second-Order

:::{note}
**See also:**

Annotations for §3.4(iii) , §3.4 and Ch.3
:::


<a id="E22"></a>
$$
\frac{{\partial}^{2}u_{0,0}}{{\partial x}^{2}}=\frac{1}{h^{2}}\,(u_{1,0}-2u_{0,0}+u_{-1,0})+O\left(h^{2}\right), \tag{3.4.22}
$$


<a id="E23"></a>
$$
\frac{{\partial}^{2}u_{0,0}}{{\partial x}^{2}}=\frac{1}{12h^{2}}\,(-u_{2,0}+16u_{1,0}-30u_{0,0}+16u_{-1,0}-u_{-2,0})+O\left(h^{4}\right), \tag{3.4.23}
$$


<a id="E24"></a>
$$
\frac{{\partial}^{2}u_{0,0}}{{\partial x}^{2}}=\frac{1}{3h^{2}}\,(u_{1,1}-2u_{0,1}+u_{-1,1}+u_{1,0}-2u_{0,0}+u_{-1,0}+u_{1,-1}-2u_{0,-1}+u_{-1,-1})+O\left(h^{2}\right). \tag{3.4.24}
$$


<a id="E25"></a>
$$
\frac{\,{\partial}^{2}u_{0,0}}{\,\partial x\,\partial y}=\frac{1}{4h^{2}}\,(u_{1,1}-u_{1,-1}-u_{-1,1}+u_{-1,-1})+O\left(h^{2}\right), \tag{3.4.25}
$$


<a id="E26"></a>
$$
\frac{\,{\partial}^{2}u_{0,0}}{\,\partial x\,\partial y}=-\frac{1}{2h^{2}}\,(u_{1,0}+u_{-1,0}+u_{0,1}+u_{0,-1}-2u_{0,0}-u_{1,1}-u_{-1,-1})+O\left(h^{2}\right). \tag{3.4.26}
$$


### Laplacian

:::{note}
**Keywords:**

[Laplacian](http://dlmf.nist.gov/search/search?q=Laplacian) , [numerical approximations](http://dlmf.nist.gov/search/search?q=numerical%20approximations)

**See also:**

Annotations for §3.4(iii) , §3.4 and Ch.3
:::

<a id="EGx1"></a>

$$
\displaystyle\nabla^{2}u \displaystyle=\frac{{\partial}^{2}u}{{\partial x}^{2}}+\frac{{\partial}^{2}u}{{\partial y}^{2}}\,. \tag{3.4.27}
$$

:::{note}
**Symbols:**

$\frac{\partial\NVar{f}}{\partial\NVar{x}}$: partial derivative of $f$ with respect to $x$ , $\,\partial\NVar{x}$: partial differential of $x$ and $u$: function

**A&S Ref:**

25.3.30

**See also:**

Annotations for §3.4(iii) , §3.4(iii) , §3.4 and Ch.3
:::

$$
\displaystyle\nabla^{2}u_{0,0} \displaystyle=\frac{1}{h^{2}}\,(u_{1,0}+u_{0,1}+u_{-1,0}+u_{0,-1}-4u_{0,0})+O\left(h^{2}\right), \tag{3.4.28}
$$

:::{note}
**Symbols:**

$O\left(\NVar{x}\right)$: order not exceeding and $u$: function

**A&S Ref:**

25.3.30

**See also:**

Annotations for §3.4(iii) , §3.4(iii) , §3.4 and Ch.3
:::


<a id="E29"></a>
$$
\nabla^{2}u_{0,0}=\frac{1}{12h^{2}}\left(-60u_{0,0}+16(u_{1,0}+u_{0,1}+u_{-1,0}+u_{0,-1})-(u_{2,0}+u_{0,2}+u_{-2,0}+u_{0,-2})\right)+O\left(h^{4}\right). \tag{3.4.29}
$$


### Fourth-Order

:::{note}
**See also:**

Annotations for §3.4(iii) , §3.4 and Ch.3
:::

<a id="EGx2"></a>

$$
\displaystyle\frac{{\partial}^{4}u_{0,0}}{{\partial x}^{4}} \displaystyle=\frac{1}{h^{4}}\,(u_{2,0}-4u_{1,0}+6u_{0,0}-4u_{-1,0}+u_{-2,0})+O\left(h^{2}\right). \tag{3.4.30}
$$

:::{note}
**Symbols:**

$O\left(\NVar{x}\right)$: order not exceeding , $\frac{\partial\NVar{f}}{\partial\NVar{x}}$: partial derivative of $f$ with respect to $x$ , $\,\partial\NVar{x}$: partial differential of $x$ and $u$: function

**A&S Ref:**

25.3.28

**See also:**

Annotations for §3.4(iii) , §3.4(iii) , §3.4 and Ch.3
:::

$$
\displaystyle\frac{\,{\partial}^{4}u_{0,0}}{\,{\partial}^{2}x\,{\partial}^{2}y} \displaystyle=\frac{1}{h^{4}}\,(u_{1,1}+u_{-1,1}+u_{1,-1}+u_{-1,-1}-2u_{1,0}-2u_{-1,0}-2u_{0,1}-2u_{0,-1}+4u_{0,0})+O\left(h^{2}\right). \tag{3.4.31}
$$

:::{note}
**Symbols:**

$O\left(\NVar{x}\right)$: order not exceeding , $\,\partial\NVar{x}$: partial differential of $x$ and $u$: function

**A&S Ref:**

25.3.29

**See also:**

Annotations for §3.4(iii) , §3.4(iii) , §3.4 and Ch.3
:::


### Biharmonic Operator

:::{note}
**Keywords:**

[biharmonic operator](http://dlmf.nist.gov/search/search?q=biharmonic%20operator) , [differentiation](http://dlmf.nist.gov/search/search?q=differentiation) , [numerical](http://dlmf.nist.gov/search/search?q=numerical) , [numerical approximation](http://dlmf.nist.gov/search/search?q=numerical%20approximation) , [partial derivatives](http://dlmf.nist.gov/search/search?q=partial%20derivatives)

**See also:**

Annotations for §3.4(iii) , §3.4 and Ch.3
:::


<a id="E32"></a>
$$
\nabla^{4}u=\frac{{\partial}^{4}u}{{\partial x}^{4}}+2\frac{\,{\partial}^{4}u}{\,{\partial}^{2}x\,{\partial}^{2}y}+\frac{{\partial}^{4}u}{{\partial y}^{4}}\,. \tag{3.4.32}
$$


<a id="E33"></a>
$$
\nabla^{4}u_{0,0}=\frac{1}{h^{4}}\,(20u_{0,0}-8(u_{1,0}+u_{0,1}+u_{-1,0}+u_{0,-1})+2(u_{1,1}+u_{1,-1}+u_{-1,1}+u_{-1,-1})+(u_{0,2}+u_{2,0}+u_{-2,0}+u_{0,-2}))+O\left(h^{2}\right), \tag{3.4.33}
$$


<a id="E34"></a>
$$
\nabla^{4}u_{0,0}=\frac{1}{6h^{4}}\,(184u_{0,0}-(u_{0,3}+u_{0,-3}+u_{3,0}+u_{-3,0})+14(u_{0,2}+u_{0,-2}+u_{2,0}+u_{-2,0})-77(u_{0,1}+u_{0,-1}+u_{1,0}+u_{-1,0})+20(u_{1,1}+u_{1,-1}+u_{-1,1}+u_{-1,-1})-(u_{1,2}+u_{2,1}+u_{1,-2}+u_{2,-1}+u_{-1,2}+u_{-2,1}+u_{-1,-2}+u_{-2,-1}))+O\left(h^{4}\right). \tag{3.4.34}
$$

The results in this subsection for the partial derivatives follow from Panow ([1955](./bib/P.html#bib1829 "Formelsammlung zur numerischen Behandlung partieller Differentialgleichungen nach dem Differenzenverfahren"), Table 10). Those for the Laplacian and the biharmonic operator follow from the formulas for the partial derivatives.

For additional formulas involving values of $\nabla^{2}u$ and $\nabla^{4}u$ on square, triangular, and cubic grids, see Collatz ([1960](./bib/C.html#bib559 "The Numerical Treatment of Differential Equations"), Table VI, pp. 542–546).
