# §31.2 Differential Equations

:::{note}
**See also:**

Annotations for Ch.31
:::


## §31.2(i) Heun’s Equation

:::{note}
**Keywords:**

[Heun equation](http://dlmf.nist.gov/search/search?q=Heun%20equation) , [Heun’s equation](http://dlmf.nist.gov/search/search?q=Heun%20equation) , [accessory parameter](http://dlmf.nist.gov/search/search?q=accessory%20parameter) , [classification](http://dlmf.nist.gov/search/search?q=classification) , [classification of parameters](http://dlmf.nist.gov/search/search?q=classification%20of%20parameters) , [exponent parameters](http://dlmf.nist.gov/search/search?q=exponent%20parameters) , [parameters](http://dlmf.nist.gov/search/search?q=parameters) , [singularities](http://dlmf.nist.gov/search/search?q=singularities) , [singularity parameter](http://dlmf.nist.gov/search/search?q=singularity%20parameter)

**Notes:**

See Erdélyi et al. ([1955](./bib/E.html#bib755 "Higher Transcendental Functions. Vol. III"), Chapter XV) and Ronveaux ([1995](./bib/R.html#bib1965 "Heun’s Differential Equations"), Part A, p. 7).

**See also:**

Annotations for §31.2 and Ch.31
:::


<a id="E1"></a>
$$
\frac{{\mathrm{d}}^{2}w}{{\mathrm{d}z}^{2}}+\left(\frac{\gamma}{z}+\frac{\delta}{z-1}+\frac{\epsilon}{z-a}\right)\frac{\mathrm{d}w}{\mathrm{d}z}+\frac{\alpha\beta z-q}{z(z-1)(z-a)}w=0, \tag{31.2.1}
$$

This equation has regular singularities at $0,1,a,\infty$ , with corresponding exponents $\{0,1-\gamma\}$ , $\{0,1-\delta\}$ , $\{0,1-\epsilon\}$ , $\{\alpha,\beta\}$ , respectively (§ 2.7(i) ). All other homogeneous linear differential equations of the second order having four regular singularities in the extended complex plane, $\mathbb{C}\cup\{\infty\}$ , can be transformed into ( 31.2.1 ).

The parameters play different roles: $a$ is the *singularity parameter* ; $\alpha,\beta,\gamma,\delta,\epsilon$ are *exponent parameters* ; $q$ is the *accessory parameter* . The total number of free parameters is six.


## §31.2(ii) Normal Form of Heun’s Equation

:::{note}
**Keywords:**

[Heun’s equation](http://dlmf.nist.gov/search/search?q=Heun%20equation) , [normal form](http://dlmf.nist.gov/search/search?q=normal%20form)

**See also:**

Annotations for §31.2 and Ch.31
:::


<a id="E2"></a>
$$
w(z)=z^{-\gamma/2}(z-1)^{-\delta/2}(z-a)^{-\epsilon/2}W(z), \tag{31.2.2}
$$


<a id="E3"></a>
$$
\frac{{\mathrm{d}}^{2}W}{{\mathrm{d}z}^{2}}=\left(\frac{A}{z}+\frac{B}{z-1}+\frac{C}{z-a}+\frac{D}{z^{2}}+\frac{E}{(z-1)^{2}}+\frac{F}{(z-a)^{2}}\right)W, \tag{31.2.3}
$$

<a id="E4"></a>

<a id="Ex1"></a>
$$
\displaystyle A \displaystyle=-\frac{\gamma\delta}{2}-\frac{\gamma\epsilon}{2a}+\frac{q}{a}, \tag{31.2.4}
$$

<a id="Ex2"></a>
$$
\displaystyle B \displaystyle=\frac{\gamma\delta}{2}-\frac{\delta\epsilon}{2(a-1)}-\frac{q-\alpha\beta}{a-1},
$$

<a id="Ex3"></a>
$$
\displaystyle C \displaystyle=\frac{\gamma\epsilon}{2a}+\frac{\delta\epsilon}{2(a-1)}-\frac{a\alpha\beta-q}{a(a-1)},
$$

<a id="Ex4"></a>
$$
\displaystyle D \displaystyle=\tfrac{1}{2}\gamma\left(\tfrac{1}{2}\gamma-1\right),
$$

<a id="Ex5"></a>
$$
\displaystyle E \displaystyle=\tfrac{1}{2}\delta\left(\tfrac{1}{2}\delta-1\right),
$$

<a id="Ex6"></a>
$$
\displaystyle F \displaystyle=\tfrac{1}{2}\epsilon\left(\tfrac{1}{2}\epsilon-1\right).
$$

:::{note}
**Defines:**

$A$ (locally) , $B$ (locally) , $C$ (locally) , $D$ (locally) , $E$ (locally) and $F$ (locally)

**Symbols:**

$\gamma$: real or complex parameter , $\delta$: real or complex parameter , $\epsilon$: real or complex parameter , $a$: complex parameter , $q$: real or complex parameter , $\alpha$: real or complex parameter and $\beta$: real or complex parameter

**See also:**

Annotations for §31.2(ii) , §31.2 and Ch.31
:::


## §31.2(iii) Trigonometric Form

:::{note}
**Keywords:**

[Heun’s equation](http://dlmf.nist.gov/search/search?q=Heun%20equation) , [trigonometric form](http://dlmf.nist.gov/search/search?q=trigonometric%20form)

**See also:**

Annotations for §31.2 and Ch.31
:::


<a id="E5"></a>
$$
z={\sin}^{2}\theta, \tag{31.2.5}
$$


<a id="E6"></a>
$$
\frac{{\mathrm{d}}^{2}w}{{\mathrm{d}\theta}^{2}}+\left({(2\gamma-1)\cot\theta-(2\delta-1)\tan\theta}-\frac{\epsilon\sin\left(2\theta\right)}{a-{\sin}^{2}\theta}\right)\frac{\mathrm{d}w}{\mathrm{d}\theta}+4\frac{\alpha\beta{\sin}^{2}\theta-q}{a-{\sin}^{2}\theta}w=0. \tag{31.2.6}
$$


## §31.2(iv) Doubly-Periodic Forms

:::{note}
**Notes:**

See Ronveaux ([1995](./bib/R.html#bib1965 "Heun’s Differential Equations"), Part A, p. 26).

**See also:**

Annotations for §31.2 and Ch.31
:::


### Jacobi’s Elliptic Form

:::{note}
**Keywords:**

[Heun’s equation](http://dlmf.nist.gov/search/search?q=Heun%20equation) , [Jacobi’s elliptic](http://dlmf.nist.gov/search/search?q=Jacobi%20elliptic) , [Jacobi’s elliptic form](http://dlmf.nist.gov/search/search?q=Jacobi%20elliptic%20form) , [doubly-periodic forms](http://dlmf.nist.gov/search/search?q=doubly-periodic%20forms)

**See also:**

Annotations for §31.2(iv) , §31.2 and Ch.31
:::

With the notation of § [22.2](./22.2.md "§22.2 Definitions ‣ Properties ‣ Chapter 22 Jacobian Elliptic Functions") let

<a id="E7"></a>

<a id="Ex7"></a>
$$
\displaystyle a \displaystyle=k^{-2}, \tag{31.2.7}
$$

<a id="Ex8"></a>
$$
\displaystyle z \displaystyle={\operatorname{sn}}^{2}\left(\zeta,k\right).
$$

:::{note}
**Defines:**

$k$ : modulus (locally)

**Symbols:**

$\operatorname{sn}\left(\NVar{z},\NVar{k}\right)$: Jacobian elliptic function , $z$: complex variable , $a$: complex parameter and $\zeta$: change of variable

**See also:**

Annotations for §31.2(iv) , §31.2(iv) , §31.2 and Ch.31
:::

Then (suppressing the parameter $k$ )


<a id="E8"></a>
$$
\frac{{\mathrm{d}}^{2}w}{{\mathrm{d}\zeta}^{2}}+\left((2\gamma-1)\frac{\operatorname{cn}\zeta\operatorname{dn}\zeta}{\operatorname{sn}\zeta}-(2\delta-1)\frac{\operatorname{sn}\zeta\operatorname{dn}\zeta}{\operatorname{cn}\zeta}-(2\epsilon-1)k^{2}\frac{\operatorname{sn}\zeta\operatorname{cn}\zeta}{\operatorname{dn}\zeta}\right)\frac{\mathrm{d}w}{\mathrm{d}\zeta}+4k^{2}(\alpha\beta{\operatorname{sn}}^{2}\zeta-q)w=0. \tag{31.2.8}
$$


### Weierstrass’s Form

:::{note}
**Keywords:**

[Heun’s equation](http://dlmf.nist.gov/search/search?q=Heun%20equation) , [Weierstrass’s](http://dlmf.nist.gov/search/search?q=Weierstrass%E2%80%99s) , [Weierstrass’s form](http://dlmf.nist.gov/search/search?q=Weierstrass%20form) , [doubly-periodic forms](http://dlmf.nist.gov/search/search?q=doubly-periodic%20forms)

**See also:**

Annotations for §31.2(iv) , §31.2 and Ch.31
:::

With the notation of §§ 19.2(ii) and [23.2](./23.2.md "§23.2 Definitions and Periodic Properties ‣ Weierstrass Elliptic Functions ‣ Chapter 23 Weierstrass Elliptic and Modular Functions") let

<a id="E9"></a>

<a id="Ex9"></a>
$$
\displaystyle k^{2} \displaystyle=(e_{2}-e_{3})/(e_{1}-e_{3}), \tag{31.2.9}
$$

<a id="Ex10"></a>
$$
\displaystyle\zeta \displaystyle=\mathrm{i}{K^{\prime}}+\xi(e_{1}-e_{3})^{1/2},
$$

<a id="Ex11"></a>
$$
\displaystyle e_{1} \displaystyle=\wp\left(\omega_{1}\right),
$$

<a id="Ex12"></a>
$$
\displaystyle e_{2} \displaystyle=\wp\left(\omega_{2}\right),
$$

<a id="Ex13"></a>
$$
\displaystyle e_{3} \displaystyle=\wp\left(\omega_{3}\right),
$$

<a id="Ex14"></a>
$$
\displaystyle e_{1}+e_{2}+e_{3}=0,
$$

:::{note}
**Defines:**

$\zeta$ : change of variable (locally)

**Symbols:**

$\wp\left(\NVar{z}\right)$ (= $\wp\left(z|\mathbb{L}\right)$ = $\wp\left(z;g_{2},g_{3}\right)$): Weierstrass $\wp$-function , $e_{\NVar{j}}$: Weierstrass lattice roots , ${K^{\prime}}\left(\NVar{k}\right)$: Legendre’s complementary complete elliptic integral of the first kind , $\mathrm{i}$: imaginary unit , $\omega_{j}$: nonzero complex number , $\mathbb{L}$: lattice and $k$: modulus

**See also:**

Annotations for §31.2(iv) , §31.2(iv) , §31.2 and Ch.31
:::

where $2\omega_{1}$ and $2\omega_{3}$ with $\Im\left(\omega_{3}/\omega_{1}\right)>0$ are generators of the lattice $\mathbb{L}$ for $\wp\left(z|\mathbb{L}\right)$ . Then


<a id="E10"></a>
$$
w(\xi)=\left(\wp\left(\xi\right)-e_{3}\right)^{(1-2\gamma)/4}\left(\wp\left(\xi\right)-e_{2}\right)^{(1-2\delta)/4}\*\left(\wp\left(\xi\right)-e_{1}\right)^{(1-2\epsilon)/4}W(\xi), \tag{31.2.10}
$$

where $W(\xi)$ satisfies


<a id="E11"></a>
$$
\ifrac{{\mathrm{d}}^{2}W}{{\mathrm{d}\xi}^{2}}+\left(H+b_{0}\wp\left(\xi\right)+b_{1}\wp\left(\xi+\omega_{1}\right)+b_{2}\wp\left(\xi+\omega_{2}\right)+b_{3}\wp\left(\xi+\omega_{3}\right)\right)W=0, \tag{31.2.11}
$$

with

<a id="E12"></a>

<a id="Ex15"></a>
$$
\displaystyle b_{0} \displaystyle=4\alpha\beta-(\gamma+\delta+\epsilon-\tfrac{1}{2})(\gamma+\delta+\epsilon-\tfrac{3}{2}), \tag{31.2.12}
$$

<a id="Ex16"></a>
$$
\displaystyle b_{1} \displaystyle=-(\epsilon-\tfrac{1}{2})(\epsilon-\tfrac{3}{2}),
$$

<a id="Ex17"></a>
$$
\displaystyle b_{2} \displaystyle=-(\delta-\tfrac{1}{2})(\delta-\tfrac{3}{2}),
$$

<a id="Ex18"></a>
$$
\displaystyle b_{3} \displaystyle=-(\gamma-\tfrac{1}{2})(\gamma-\tfrac{3}{2}),
$$

<a id="Ex19"></a>
$$
\displaystyle H \displaystyle=e_{1}(\gamma+\delta-1)^{2}+e_{2}(\gamma+\epsilon-1)^{2}+e_{3}(\delta+\epsilon-1)^{2}-4\alpha\beta e_{3}-4q(e_{2}-e_{3}).
$$

:::{note}
**Defines:**

$b_{j}$ : coefficients (locally) and $H$ (locally)

**Symbols:**

$e_{\NVar{j}}$: Weierstrass lattice roots , $\gamma$: real or complex parameter , $\delta$: real or complex parameter , $\epsilon$: real or complex parameter , $j$: nonnegative integer , $q$: real or complex parameter , $\alpha$: real or complex parameter , $\beta$: real or complex parameter and $\mathbb{L}$: lattice

**See also:**

Annotations for §31.2(iv) , §31.2(iv) , §31.2 and Ch.31
:::


## §31.2(v) Heun’s Equation Automorphisms

:::{note}
**Keywords:**

[Heun’s equation](http://dlmf.nist.gov/search/search?q=Heun%20equation) , [automorphisms](http://dlmf.nist.gov/search/search?q=automorphisms)

**Referenced by:**

§31.3(iii) , §31.8

**See also:**

Annotations for §31.2 and Ch.31
:::


### F-Homotopic Transformations

:::{note}
**Keywords:**

[$F$-homotopic transformations](http://dlmf.nist.gov/search/search?q=F-homotopic%20transformations) , [Heun’s equation](http://dlmf.nist.gov/search/search?q=Heun%20equation) , [automorphisms](http://dlmf.nist.gov/search/search?q=automorphisms)

**Notes:**

See Ronveaux ([1995](./bib/R.html#bib1965 "Heun’s Differential Equations"), Part A, p. 16).

**See also:**

Annotations for §31.2(v) , §31.2 and Ch.31
:::

$w(z)=z^{1-\gamma}w_{1}(z)$ satisfies ( 31.2.1 ) if $w_{1}$ is a solution of ( 31.2.1 ) with transformed parameters $q_{1}=q+(a\delta+\epsilon)(1-\gamma)$ ; $\alpha_{1}=\alpha+1-\gamma$ , $\beta_{1}=\beta+1-\gamma$ , $\gamma_{1}=2-\gamma$ . Next, $w(z)=(z-1)^{1-\delta}w_{2}(z)$ satisfies ( 31.2.1 ) if $w_{2}$ is a solution of ( 31.2.1 ) with transformed parameters $q_{2}=q+a\gamma(1-\delta)$ ; $\alpha_{2}=\alpha+1-\delta$ , $\beta_{2}=\beta+1-\delta$ , $\delta_{2}=2-\delta$ . Lastly, $w(z)=(z-a)^{1-\epsilon}w_{3}(z)$ satisfies ( 31.2.1 ) if $w_{3}$ is a solution of ( 31.2.1 ) with transformed parameters $q_{3}=q+\gamma(1-\epsilon)$ ; $\alpha_{3}=\alpha+1-\epsilon$ , $\beta_{3}=\beta+1-\epsilon$ , $\epsilon_{3}=2-\epsilon$ . By composing these three steps, there result $2^{3}=8$ possible transformations of the dependent variable (including the identity transformation) that preserve the form of ( 31.2.1 ).


### Homographic Transformations

:::{note}
**Keywords:**

[Heun’s equation](http://dlmf.nist.gov/search/search?q=Heun%20equation) , [automorphisms](http://dlmf.nist.gov/search/search?q=automorphisms) , [homographic transformations](http://dlmf.nist.gov/search/search?q=homographic%20transformations)

**See also:**

Annotations for §31.2(v) , §31.2 and Ch.31
:::

There are $4!=24$ homographies $\tilde{z}(z)=(Az+B)/(Cz+D)$ that take $0,1,a,\infty$ to some permutation of $0,1,a^{\prime},\infty$ , where $a^{\prime}$ may differ from $a$ . If $\tilde{z}=\tilde{z}(z)$ is one of the $3!=6$ homographies that map $\infty$ to $\infty$ , then $w(z)=\tilde{w}(\tilde{z})$ satisfies ( 31.2.1 ) if $\tilde{w}(\tilde{z})$ is a solution of ( 31.2.1 ) with $z$ replaced by $\tilde{z}$ and appropriately transformed parameters. For example, if $\tilde{z}=z/a$ , then the parameters are $\tilde{a}=1/a$ , $\tilde{q}=q/a$ ; $\tilde{\delta}=\epsilon$ , $\tilde{\epsilon}=\delta$ . If $\tilde{z}=\tilde{z}(z)$ is one of the $4!-3!=18$ homographies that do not map $\infty$ to $\infty$ , then an appropriate prefactor must be included on the right-hand side. For example, $w(z)=(1-z)^{-\alpha}\tilde{w}(z/(z-1))$ , which arises from $\tilde{z}=z/(z-1)$ , satisfies ( 31.2.1 ) if $\tilde{w}(\tilde{z})$ is a solution of ( 31.2.1 ) with $z$ replaced by $\tilde{z}$ and transformed parameters $\tilde{a}=a/(a-1)$ , $\tilde{q}=-(q-a\alpha\gamma)/(a-1)$ ; $\tilde{\beta}=\alpha+1-\delta$ , $\tilde{\delta}=\alpha+1-\beta$ .


### Composite Transformations

:::{note}
**Keywords:**

[Heun’s equation](http://dlmf.nist.gov/search/search?q=Heun%20equation) , [automorphisms](http://dlmf.nist.gov/search/search?q=automorphisms) , [composite](http://dlmf.nist.gov/search/search?q=composite)

**See also:**

Annotations for §31.2(v) , §31.2 and Ch.31
:::

There are $8\cdot 24=192$ automorphisms of equation ( 31.2.1 ) by compositions of $F$ -homotopic and homographic transformations. Each is a substitution of dependent and/or independent variables that preserves the form of ( 31.2.1 ). Except for the identity automorphism, each alters the parameters.
