# §4.6 Power Series

:::{note}
**See also:**

Annotations for Ch.4
:::


## §4.6(i) Logarithms

:::{note}
**Keywords:**

[logarithm function](http://dlmf.nist.gov/search/search?q=logarithm%20function) , [power series](http://dlmf.nist.gov/search/search?q=power%20series)

**Notes:**

See Hardy ([1952](./bib/H.html#bib1043 "A Course of Pure Mathematics"), pp. 471–473) for ( 4.6.1 ). The other equations are variations of this.

**See also:**

Annotations for §4.6 and Ch.4
:::


<a id="E1"></a>
$$
\ln\left(1+z\right)=z-\tfrac{1}{2}z^{2}+\tfrac{1}{3}z^{3}-\cdots, \tag{4.6.1}
$$


<a id="E2"></a>
$$
\ln z=\left(\frac{z-1}{z}\right)+\frac{1}{2}\left(\frac{z-1}{z}\right)^{2}+\frac{1}{3}\left(\frac{z-1}{z}\right)^{3}+\cdots, \tag{4.6.2}
$$


<a id="E3"></a>
$$
\ln z=(z-1)-\tfrac{1}{2}(z-1)^{2}+\tfrac{1}{3}(z-1)^{3}-\cdots, \tag{4.6.3}
$$


<a id="E4"></a>
$$
\ln z=2\left(\left(\frac{z-1}{z+1}\right)+\frac{1}{3}\left(\frac{z-1}{z+1}\right)^{3}+\frac{1}{5}\left(\frac{z-1}{z+1}\right)^{5}+\cdots\right), \tag{4.6.4}
$$


<a id="E5"></a>
$$
\ln\left(\frac{z+1}{z-1}\right)=2\left(\frac{1}{z}+\frac{1}{3z^{3}}+\frac{1}{5z^{5}}+\cdots\right), \tag{4.6.5}
$$


<a id="E6"></a>
$$
\ln\left(z+a\right)=\ln a+2\left(\left(\frac{z}{2a+z}\right)+\frac{1}{3}\left(\frac{z}{2a+z}\right)^{3}+\frac{1}{5}\left(\frac{z}{2a+z}\right)^{5}+\cdots\right), \tag{4.6.6}
$$


## §4.6(ii) Powers

:::{note}
**Notes:**

See Hardy ([1952](./bib/H.html#bib1043 "A Course of Pure Mathematics"), pp. 476–477).

**Referenced by:**

Erratum (V1.0.11) for Clarifications

**Addition (effective with 1.0.11):**

A sentence was added after ( 4.6.7 ) to explain that it is a generalization of ( 1.2.2 ) using ( 1.2.6 )

**See also:**

Annotations for §4.6 and Ch.4
:::


### Binomial Expansion

:::{note}
**Keywords:**

[binomial expansion](http://dlmf.nist.gov/search/search?q=binomial%20expansion)

**See also:**

Annotations for §4.6(ii) , §4.6 and Ch.4
:::


<a id="E7"></a>
$$
(1+z)^{a}=1+\frac{a}{1!}z+\frac{a(a-1)}{2!}z^{2}+\frac{a(a-1)(a-2)}{3!}z^{3}+\cdots, \tag{4.6.7}
$$

valid when $a$ is any real or complex constant and $|z|<1$ . If $a=0,1,2,\dots$ , then the series terminates and $z$ is unrestricted. Note that ( 4.6.7 ) is a generalization of the binomial expansion ( 1.2.2 ) with the binomial coefficients defined in ( 1.2.6 ).
