# §5.8 Infinite Products

:::{note}
**Keywords:**

[gamma function](http://dlmf.nist.gov/search/search?q=gamma%20function) , [infinite products](http://dlmf.nist.gov/search/search?q=infinite%20products)

**Notes:**

For ( 5.8.1 )–( 5.8.3 ) see Olver ([1997b](./bib/O.html#bib1809 "Asymptotics and Special Functions"), pp. 34 and 38). For ( 5.8.4 )–( 5.8.5 ) see Whittaker and Watson ([1927](./bib/W.html#bib2404 "A Course of Modern Analysis"), p. 238–239).

**See also:**

Annotations for Ch.5
:::


<a id="E1"></a>
$$
\Gamma\left(z\right)=\lim_{k\to\infty}\frac{k!k^{z}}{z(z+1)\cdots(z+k)}, \tag{5.8.1}
$$


<a id="E2"></a>
$$
\frac{1}{\Gamma\left(z\right)}=ze^{\gamma z}\prod_{k=1}^{\infty}\left(1+\frac{z}{k}\right)e^{-z/k}, \tag{5.8.2}
$$


<a id="E3"></a>
$$
\left|\frac{\Gamma\left(x\right)}{\Gamma\left(x+\mathrm{i}y\right)}\right|^{2}=\prod_{k=0}^{\infty}\left(1+\frac{y^{2}}{(x+k)^{2}}\right), \tag{5.8.3}
$$

If


<a id="E4"></a>
$$
\sum_{k=1}^{m}a_{k}=\sum_{k=1}^{m}b_{k}, \tag{5.8.4}
$$

then


<a id="E5"></a>
$$
\prod_{k=0}^{\infty}\frac{(a_{1}+k)(a_{2}+k)\cdots(a_{m}+k)}{(b_{1}+k)(b_{2}+k)\cdots(b_{m}+k)}=\frac{\Gamma\left(b_{1}\right)\Gamma\left(b_{2}\right)\cdots\Gamma\left(b_{m}\right)}{\Gamma\left(a_{1}\right)\Gamma\left(a_{2}\right)\cdots\Gamma\left(a_{m}\right)}, \tag{5.8.5}
$$

provided that none of the $b_{k}$ is zero or a negative integer.
