# §8.10 Inequalities

:::{note}
**Keywords:**

[incomplete gamma functions](http://dlmf.nist.gov/search/search?q=incomplete%20gamma%20functions) , [inequalities](http://dlmf.nist.gov/search/search?q=inequalities)

**Notes:**

See Olver ([1997b](./bib/O.html#bib1809 "Asymptotics and Special Functions"), pp. 66–67) and Luke ([1969b](./bib/L.html#bib1496 "The Special Functions and their Approximations. Vol. 2"), pp. 195, 201). For ( 8.10.10 )–( 8.10.13 ), see Gautschi ([1959b](./bib/G.html#bib870 "Some elementary inequalities relating to the gamma and incomplete gamma function")), Alzer ([1997b](./bib/index.html#bib69 "On some inequalities for the incomplete gamma function")), and Vietoris ([1983](./bib/V.html#bib2333 "Dritter Beweis der die unvollständige Gammafunktion betreffenden Lochsschen Ungleichungen")).

**Referenced by:**

Erratum (V1.0.10) for References

**Addition (effective with 1.0.10):**

A reference to Neuman ([2013](./bib/N.html#bib2660 "Inequalities and bounds for the incomplete gamma function")) was added after ( 8.10.4 )

**See also:**

Annotations for Ch.8
:::


<a id="E1"></a>
$$
x^{1-a}e^{x}\Gamma\left(a,x\right)\leq 1, \tag{8.10.1}
$$


<a id="E2"></a>
$$
\gamma\left(a,x\right)\geq\frac{x^{a-1}}{a}(1-e^{-x}), \tag{8.10.2}
$$

The inequalities in ( 8.10.1 ) and ( 8.10.2 ) are reversed when $a\geq 1$ . If $\vartheta$ is defined by


<a id="E3"></a>
$$
x^{1-a}e^{x}\Gamma\left(a,x\right)=1+\frac{a-1}{x}\vartheta, \tag{8.10.3}
$$

then $\vartheta\to 1$ as $x\to\infty$ , and


<a id="E4"></a>
$$
0<\vartheta\leq 1, \tag{8.10.4}
$$

For further inequalities of these types see Qi and Mei ([1999](./bib/Q.html#bib1910 "Some inequalities of the incomplete gamma and related functions")) and Neuman ([2013](./bib/N.html#bib2660 "Inequalities and bounds for the incomplete gamma function")).

:::{note}
**Keywords:**

[Padé approximant](http://dlmf.nist.gov/search/search?q=Pad%C3%A9%20approximant) , [incomplete gamma functions](http://dlmf.nist.gov/search/search?q=incomplete%20gamma%20functions)

**See also:**

Annotations for §8.10 and Ch.8
:::

For $n=1,2,\dots$ ,


<a id="E5"></a>
$$
A_{n}<x^{1-a}e^{x}\Gamma\left(a,x\right)<B_{n}, \tag{8.10.5}
$$

where

<a id="E6"></a>

<a id="Ex1"></a>
$$
\displaystyle A_{1} \displaystyle=\frac{x}{x+1-a}, \tag{8.10.6}
$$

<a id="Ex2"></a>
$$
\displaystyle B_{1} \displaystyle=\frac{x+1}{x+2-a},
$$

<a id="Ex3"></a>
$$
\displaystyle A_{2} \displaystyle=\frac{x(x+3-a)}{x^{2}+2(2-a)x+(1-a)(2-a)},
$$

<a id="Ex4"></a>
$$
\displaystyle B_{2} \displaystyle=\frac{x^{2}+(5-a)x+2}{x^{2}+2(3-a)x+(2-a)(3-a)}.
$$

:::{note}
**Symbols:**

$x$: real variable , $a$: parameter , $A_{n}$: minima and $B_{n}$: maxima

**See also:**

Annotations for §8.10 , §8.10 and Ch.8
:::

For hypergeometric polynomial representations of $A_{n}$ and $B_{n}$ , see Luke ([1969b](./bib/L.html#bib1496 "The Special Functions and their Approximations. Vol. 2"), §14.6).

Next, define


<a id="E7"></a>
$$
I=\int_{0}^{x}t^{a-1}e^{t}\,\mathrm{d}t=\Gamma\left(a\right)x^{a}\gamma^{*}\left(a,-x\right), \tag{8.10.7}
$$

Then


<a id="E8"></a>
$$
\frac{(a+1)(a+2)-x}{(a+1)(a+2+x)}<ax^{-a}e^{-x}I<\frac{a+1}{a+1+x}, \tag{8.10.8}
$$

Also, define

<a id="E9"></a>

<a id="Ex5"></a>
$$
\displaystyle c_{a} \displaystyle=(\Gamma\left(1+a\right))^{1/(a-1)}, \tag{8.10.9}
$$

<a id="Ex6"></a>
$$
\displaystyle d_{a} \displaystyle=(\Gamma\left(1+a\right))^{-1/a}.
$$

:::{note}
**Symbols:**

$\Gamma\left(\NVar{z}\right)$: gamma function , $a$: parameter , $c_{a}$: coefficients and $d_{a}$: coefficients

**See also:**

Annotations for §8.10 , §8.10 and Ch.8
:::

Then


<a id="E10"></a>
$$
\frac{x}{2a}\left(\left(1+\frac{2}{x}\right)^{a}-1\right)<x^{1-a}e^{x}\Gamma\left(a,x\right)\leq\frac{x}{ac_{a}}\left(\left(1+\frac{c_{a}}{x}\right)^{a}-1\right), \tag{8.10.10}
$$

and


<a id="E11"></a>
$$
(1-e^{-\alpha_{a}x})^{a}\leq P\left(a,x\right)\leq(1-e^{-\beta_{a}x})^{a}, \tag{8.10.11}
$$

where

<a id="E12"></a>

<a id="Ex7"></a>
$$
\displaystyle\alpha_{a} \displaystyle=\begin{cases}1,&0<a<1,\\
d_{a},&a>1,\end{cases} \tag{8.10.12}
$$

<a id="Ex8"></a>
$$
\displaystyle\beta_{a} \displaystyle=\begin{cases}d_{a},&0<a<1,\\
1,&a>1.\end{cases}
$$

:::{note}
**Symbols:**

$a$: parameter , $d_{a}$: coefficients , $\alpha_{a}$ and $\beta_{a}$

**See also:**

Annotations for §8.10 , §8.10 and Ch.8
:::

Equalities in ( 8.10.11 ) apply only when $a=1$ .

Lastly,


<a id="E13"></a>
$$
\frac{\Gamma\left(n,n\right)}{\Gamma\left(n\right)}<\frac{1}{2}<\frac{\Gamma\left(n,n-1\right)}{\Gamma\left(n\right)}, \tag{8.10.13}
$$
