# §8.5 Confluent Hypergeometric Representations

:::{note}
**Keywords:**

[confluent hypergeometric functions](http://dlmf.nist.gov/search/search?q=confluent%20hypergeometric%20functions) , [incomplete gamma functions](http://dlmf.nist.gov/search/search?q=incomplete%20gamma%20functions) , [relations to other functions](http://dlmf.nist.gov/search/search?q=relations%20to%20other%20functions)

**Notes:**

See Slater ([1960](./bib/S.html#bib2098 "Confluent Hypergeometric Functions"), §5.6) and § 13.2(vii) . For ( 8.5.4 ) see ( 13.18.4 ).

**See also:**

Annotations for Ch.8
:::

For the confluent hypergeometric functions $M$ , ${\mathbf{M}}$ , $U$ , and the Whittaker functions $M_{\kappa,\mu}$ and $W_{\kappa,\mu}$ , see §§ 13.2(i) and 13.14(i) .


<a id="E1"></a>
$$
\gamma\left(a,z\right)=a^{-1}z^{a}e^{-z}M\left(1,1+a,z\right)=a^{-1}z^{a}M\left(a,1+a,-z\right), \tag{8.5.1}
$$


<a id="E2"></a>
$$
\gamma^{*}\left(a,z\right)=e^{-z}{\mathbf{M}}\left(1,1+a,z\right)={\mathbf{M}}\left(a,1+a,-z\right). \tag{8.5.2}
$$


<a id="E3"></a>
$$
\Gamma\left(a,z\right)=e^{-z}U\left(1-a,1-a,z\right)=z^{a}e^{-z}U\left(1,1+a,z\right). \tag{8.5.3}
$$


<a id="E4"></a>
$$
\gamma\left(a,z\right)=a^{-1}z^{\frac{1}{2}a-\frac{1}{2}}e^{-\frac{1}{2}z}M_{\frac{1}{2}a-\frac{1}{2},\frac{1}{2}a}\left(z\right). \tag{8.5.4}
$$


<a id="E5"></a>
$$
\Gamma\left(a,z\right)=e^{-\frac{1}{2}z}z^{\frac{1}{2}a-\frac{1}{2}}W_{\frac{1}{2}a-\frac{1}{2},\frac{1}{2}a}\left(z\right). \tag{8.5.5}
$$
