# §8.7 Series Expansions

:::{note}
**Keywords:**

[Bessel functions](http://dlmf.nist.gov/search/search?q=Bessel%20functions) , [Laguerre polynomials](http://dlmf.nist.gov/search/search?q=Laguerre%20polynomials) , [expansions in series of](http://dlmf.nist.gov/search/search?q=expansions%20in%20series%20of) , [incomplete gamma functions](http://dlmf.nist.gov/search/search?q=incomplete%20gamma%20functions) , [modified spherical Bessel functions](http://dlmf.nist.gov/search/search?q=modified%20spherical%20Bessel%20functions) , [power-series expansions](http://dlmf.nist.gov/search/search?q=power-series%20expansions)

**Notes:**

See Erdélyi et al. ([1953b](./bib/E.html#bib752 "Higher Transcendental Functions. Vol. II"), p. 135 and §9.4). ( 8.7.3 ) follows from ( 8.7.1 ) and ( 8.2.3 ). For ( 8.7.5 ) use ( 8.5.2 ) and ( 13.11.1 ).

**Referenced by:**

§8.25(i)

**See also:**

Annotations for Ch.8
:::

For the functions $e_{n}(z)$ , ${\mathsf{i}^{(1)}_{n}}\left(z\right)$ , and $L^{(\alpha)}_{n}\left(x\right)$ see ( 8.4.11 ), §§ 10.47(ii) , and [18.3](./18.3.md "§18.3 Definitions ‣ Classical Orthogonal Polynomials ‣ Chapter 18 Orthogonal Polynomials") , respectively.


<a id="E1"></a>
$$
\gamma^{*}\left(a,z\right)=e^{-z}\sum_{k=0}^{\infty}\frac{z^{k}}{\Gamma\left(a+k+1\right)}=\frac{1}{\Gamma\left(a\right)}\sum_{k=0}^{\infty}\frac{(-z)^{k}}{k!(a+k)}. \tag{8.7.1}
$$


<a id="E2"></a>
$$
\gamma\left(a,x+y\right)-\gamma\left(a,x\right)=\Gamma\left(a,x\right)-\Gamma\left(a,x+y\right)=e^{-x}x^{a-1}\sum_{n=0}^{\infty}\frac{{\left(1-a\right)_{n}}}{(-x)^{n}}(1-e^{-y}e_{n}(y)), \tag{8.7.2}
$$


<a id="E3"></a>
$$
\Gamma\left(a,z\right)=\Gamma\left(a\right)-\sum_{k=0}^{\infty}\frac{(-1)^{k}z^{a+k}}{k!(a+k)}=\Gamma\left(a\right)\left(1-z^{a}e^{-z}\sum_{k=0}^{\infty}\frac{z^{k}}{\Gamma\left(a+k+1\right)}\right), \tag{8.7.3}
$$


<a id="E4"></a>
$$
\gamma\left(a,x\right)=\Gamma\left(a\right)x^{\frac{1}{2}a}e^{-x}\sum_{n=0}^{\infty}e_{n}(-1)x^{\frac{1}{2}n}I_{n+a}\left(\textstyle 2x^{1/2}\right), \tag{8.7.4}
$$


<a id="E5"></a>
$$
\gamma^{*}\left(a,z\right)=e^{-\frac{1}{2}z}\sum_{n=0}^{\infty}\frac{{\left(1-a\right)_{n}}}{\Gamma\left(n+a+1\right)}{\left(2n+1\right)}{\mathsf{i}^{(1)}_{n}}\left(\tfrac{1}{2}z\right). \tag{8.7.5}
$$


<a id="E6"></a>
$$
\Gamma\left(a,x\right)=x^{a}e^{-x}\sum_{n=0}^{\infty}\frac{L^{(a)}_{n}\left(x\right)}{n+1}, \tag{8.7.6}
$$

For an expansion for $\gamma\left(a,ix\right)$ in series of Bessel functions $J_{n}\left(x\right)$ that converges rapidly when $a>0$ and $x$ ( $\geq 0$ ) is small or moderate in magnitude see Barakat ([1961](./bib/B.html#bib187 "Evaluation of the incomplete gamma function of imaginary argument by Chebyshev polynomials")).
