# §10.49 Explicit Formulas

:::{note}
**See also:**

Annotations for Ch.10
:::


## §10.49(i) Unmodified Functions

:::{note}
**Keywords:**

[explicit formulas](http://dlmf.nist.gov/search/search?q=explicit%20formulas) , [spherical Bessel functions](http://dlmf.nist.gov/search/search?q=spherical%20Bessel%20functions) , [unmodified functions](http://dlmf.nist.gov/search/search?q=unmodified%20functions)

**Notes:**

When $\nu=n+\tfrac{1}{2}$ the asymptotic expansions ( 10.17.3 )–( 10.17.6 ) terminate, and as a consequence of the error bounds of § 10.17(iv) they represent the left-hand sides exactly.

**Referenced by:**

§10.16 , §10.49(ii) , §10.61(v) , §10.74(i) , §11.4(i)

**See also:**

Annotations for §10.49 and Ch.10
:::

Define $a_{k}(\nu)$ as in ( 10.17.1 ). Then


<a id="E1"></a>
$$
a_{k}(n+\tfrac{1}{2})=\begin{cases}\dfrac{(n+k)!}{2^{k}k!(n-k)!},&k=0,1,\dotsc,n,\\
0,&k=n+1,n+2,\dotsc.\end{cases} \tag{10.49.1}
$$


<a id="E2"></a>
$$
\mathsf{j}_{n}\left(z\right)=\sin\left(z-\tfrac{1}{2}n\pi\right)\sum_{k=0}^{\left\lfloor n/2\right\rfloor}(-1)^{k}\frac{a_{2k}(n+\tfrac{1}{2})}{z^{2k+1}}+\cos\left(z-\tfrac{1}{2}n\pi\right)\sum_{k=0}^{\left\lfloor(n-1)/2\right\rfloor}(-1)^{k}\frac{a_{2k+1}(n+\tfrac{1}{2})}{z^{2k+2}}. \tag{10.49.2}
$$

<a id="E3"></a>

<a id="Ex1"></a>
$$
\displaystyle\mathsf{j}_{0}\left(z\right) \displaystyle=\frac{\sin z}{z}, \tag{10.49.3}
$$

<a id="Ex2"></a>
$$
\displaystyle\mathsf{j}_{1}\left(z\right) \displaystyle=\frac{\sin z}{z^{2}}-\frac{\cos z}{z},
$$

<a id="Ex3"></a>
$$
\displaystyle\mathsf{j}_{2}\left(z\right) \displaystyle=\left(-\frac{1}{z}+\frac{3}{z^{3}}\right)\sin z-\frac{3}{z^{2}}\cos z.
$$

:::{note}
**Symbols:**

$\cos\NVar{z}$: cosine function , $\sin\NVar{z}$: sine function , $\mathsf{j}_{\NVar{n}}\left(\NVar{z}\right)$: spherical Bessel function of the first kind and $z$: complex variable

**A&S Ref:**

10.1.11 (corrected)

**Referenced by:**

§10.49(iii) , §10.56

**See also:**

Annotations for §10.49(i) , §10.49 and Ch.10
:::


<a id="E4"></a>
$$
\mathsf{y}_{n}\left(z\right)=-\cos\left(z-\tfrac{1}{2}n\pi\right)\sum_{k=0}^{\left\lfloor n/2\right\rfloor}(-1)^{k}\frac{a_{2k}(n+\tfrac{1}{2})}{z^{2k+1}}+\sin\left(z-\tfrac{1}{2}n\pi\right)\sum_{k=0}^{\left\lfloor(n-1)/2\right\rfloor}(-1)^{k}\frac{a_{2k+1}(n+\tfrac{1}{2})}{z^{2k+2}}. \tag{10.49.4}
$$

<a id="E5"></a>

<a id="Ex4"></a>
$$
\displaystyle\mathsf{y}_{0}\left(z\right) \displaystyle=-\frac{\cos z}{z}, \tag{10.49.5}
$$

<a id="Ex5"></a>
$$
\displaystyle\mathsf{y}_{1}\left(z\right) \displaystyle=-\frac{\cos z}{z^{2}}-\frac{\sin z}{z},
$$

<a id="Ex6"></a>
$$
\displaystyle\mathsf{y}_{2}\left(z\right) \displaystyle=\left(\frac{1}{z}-\frac{3}{z^{3}}\right)\cos z-\frac{3}{z^{2}}\sin z.
$$

:::{note}
**Symbols:**

$\cos\NVar{z}$: cosine function , $\sin\NVar{z}$: sine function , $\mathsf{y}_{\NVar{n}}\left(\NVar{z}\right)$: spherical Bessel function of the second kind and $z$: complex variable

**A&S Ref:**

10.1.12 (corrected)

**Referenced by:**

§10.50 , §10.56

**See also:**

Annotations for §10.49(i) , §10.49 and Ch.10
:::

<a id="EGx1"></a>

$$
\displaystyle{\mathsf{h}^{(1)}_{n}}\left(z\right) \displaystyle=e^{iz}\sum_{k=0}^{n}i^{k-n-1}\frac{a_{k}(n+\frac{1}{2})}{z^{k+1}}, \tag{10.49.6}
$$

:::{note}
**Symbols:**

$\mathrm{e}$: base of natural logarithm , $\mathrm{i}$: imaginary unit , ${\mathsf{h}^{(1)}_{\NVar{n}}}\left(\NVar{z}\right)$: spherical Bessel function of the third kind , $n$: integer , $k$: nonnegative integer , $z$: complex variable and $a_{k}(\nu)$: polynomial coefficient

**A&S Ref:**

10.1.16

**Referenced by:**

§10.52(ii)

**See also:**

Annotations for §10.49(i) , §10.49 and Ch.10
:::

$$
\displaystyle{\mathsf{h}^{(2)}_{n}}\left(z\right) \displaystyle=e^{-iz}\sum_{k=0}^{n}(-i)^{k-n-1}\frac{a_{k}(n+\frac{1}{2})}{z^{k+1}}. \tag{10.49.7}
$$

:::{note}
**Symbols:**

$\mathrm{e}$: base of natural logarithm , $\mathrm{i}$: imaginary unit , ${\mathsf{h}^{(2)}_{\NVar{n}}}\left(\NVar{z}\right)$: spherical Bessel function of the third kind , $n$: integer , $k$: nonnegative integer , $z$: complex variable and $a_{k}(\nu)$: polynomial coefficient

**A&S Ref:**

10.1.17 (corrected)

**See also:**

Annotations for §10.49(i) , §10.49 and Ch.10
:::


## §10.49(ii) Modified Functions

:::{note}
**Keywords:**

[Bessel polynomials](http://dlmf.nist.gov/search/search?q=Bessel%20polynomials) , [explicit formulas](http://dlmf.nist.gov/search/search?q=explicit%20formulas) , [modified functions](http://dlmf.nist.gov/search/search?q=modified%20functions) , [spherical Bessel functions](http://dlmf.nist.gov/search/search?q=spherical%20Bessel%20functions)

**Notes:**

Use the same method as for § 10.49(i) , or combine the results of § 10.49(i) with ( 10.47.12 ) and ( 10.47.13 ).

**Referenced by:**

§10.39 , §10.74(i) , §11.4(i) , §18.34(i) , §18.34(iii) , §3.5(viii)

**See also:**

Annotations for §10.49 and Ch.10
:::

Again, with $a_{k}(n+\tfrac{1}{2})$ as in ( 10.49.1 ),


<a id="E8"></a>
$$
{\mathsf{i}^{(1)}_{n}}\left(z\right)=\tfrac{1}{2}e^{z}\sum_{k=0}^{n}(-1)^{k}\frac{a_{k}(n+\frac{1}{2})}{z^{k+1}}+(-1)^{n+1}\*\tfrac{1}{2}e^{-z}\sum_{k=0}^{n}\frac{a_{k}(n+\frac{1}{2})}{z^{k+1}}. \tag{10.49.8}
$$

<a id="E9"></a>

<a id="Ex7"></a>
$$
\displaystyle{\mathsf{i}^{(1)}_{0}}\left(z\right) \displaystyle=\frac{\sinh z}{z}, \tag{10.49.9}
$$

<a id="Ex8"></a>
$$
\displaystyle{\mathsf{i}^{(1)}_{1}}\left(z\right) \displaystyle=-\frac{\sinh z}{z^{2}}+\frac{\cosh z}{z},
$$

<a id="Ex9"></a>
$$
\displaystyle{\mathsf{i}^{(1)}_{2}}\left(z\right) \displaystyle=\left(\frac{1}{z}+\frac{3}{z^{3}}\right)\sinh z-\frac{3}{z^{2}}\cosh z.
$$

:::{note}
**Symbols:**

$\cosh\NVar{z}$: hyperbolic cosine function , $\sinh\NVar{z}$: hyperbolic sine function , ${\mathsf{i}^{(1)}_{\NVar{n}}}\left(\NVar{z}\right)$: modified spherical Bessel function and $z$: complex variable

**A&S Ref:**

10.2.13

**Referenced by:**

§18.34(i)

**See also:**

Annotations for §10.49(ii) , §10.49 and Ch.10
:::


<a id="E10"></a>
$$
{\mathsf{i}^{(2)}_{n}}\left(z\right)=\tfrac{1}{2}e^{z}\sum_{k=0}^{n}(-1)^{k}\frac{a_{k}(n+\frac{1}{2})}{z^{k+1}}+(-1)^{n}\tfrac{1}{2}e^{-z}\sum_{k=0}^{n}\frac{a_{k}(n+\frac{1}{2})}{z^{k+1}}. \tag{10.49.10}
$$

<a id="E11"></a>

<a id="Ex10"></a>
$$
\displaystyle{\mathsf{i}^{(2)}_{0}}\left(z\right) \displaystyle=\frac{\cosh z}{z}, \tag{10.49.11}
$$

<a id="Ex11"></a>
$$
\displaystyle{\mathsf{i}^{(2)}_{1}}\left(z\right) \displaystyle=-\frac{\cosh z}{z^{2}}+\frac{\sinh z}{z},
$$

<a id="Ex12"></a>
$$
\displaystyle{\mathsf{i}^{(2)}_{2}}\left(z\right) \displaystyle=\left(\frac{1}{z}+\frac{3}{z^{3}}\right)\cosh z-\frac{3}{z^{2}}\sinh z.
$$

:::{note}
**Symbols:**

$\cosh\NVar{z}$: hyperbolic cosine function , $\sinh\NVar{z}$: hyperbolic sine function , ${\mathsf{i}^{(2)}_{\NVar{n}}}\left(\NVar{z}\right)$: modified spherical Bessel function and $z$: complex variable

**A&S Ref:**

10.2.14

**See also:**

Annotations for §10.49(ii) , §10.49 and Ch.10
:::


<a id="E12"></a>
$$
\mathsf{k}_{n}\left(z\right)=\tfrac{1}{2}\pi e^{-z}\sum_{k=0}^{n}\frac{a_{k}(n+\frac{1}{2})}{z^{k+1}}. \tag{10.49.12}
$$

<a id="E13"></a>

<a id="Ex13"></a>
$$
\displaystyle\mathsf{k}_{0}\left(z\right) \displaystyle=\tfrac{1}{2}\pi\frac{e^{-z}}{z}, \tag{10.49.13}
$$

<a id="Ex14"></a>
$$
\displaystyle\mathsf{k}_{1}\left(z\right) \displaystyle=\tfrac{1}{2}\pi e^{-z}\left(\frac{1}{z}+\frac{1}{z^{2}}\right),
$$

<a id="Ex15"></a>
$$
\displaystyle\mathsf{k}_{2}\left(z\right) \displaystyle=\tfrac{1}{2}\pi e^{-z}\left(\frac{1}{z}+\frac{3}{z^{2}}+\frac{3}{z^{3}}\right).
$$

:::{note}
**Symbols:**

$\pi$: the ratio of the circumference of a circle to its diameter , $\mathrm{e}$: base of natural logarithm , $\mathsf{k}_{\NVar{n}}\left(\NVar{z}\right)$: modified spherical Bessel function and $z$: complex variable

**A&S Ref:**

10.2.17

**See also:**

Annotations for §10.49(ii) , §10.49 and Ch.10
:::

$\sum_{k=0}^{n}a_{k}(n+\tfrac{1}{2})z^{n-k}$ is sometimes called the *Bessel polynomial of degree* $n$ . For a survey of properties of these polynomials and their generalizations see Grosswald ([1978](./bib/G.html#bib998 "Bessel Polynomials")). See also § [18.34](./18.34.md "§18.34 Bessel Polynomials ‣ Other Orthogonal Polynomials ‣ Chapter 18 Orthogonal Polynomials") , de Bruin et al. ([1981a](./bib/D.html#bib628 "On the zeros of generalized Bessel polynomials. I"), [b](./bib/D.html#bib629 "On the zeros of generalized Bessel polynomials. II")), and Dunster ([2001c](./bib/D.html#bib710 "Uniform asymptotic expansions for the reverse generalized Bessel polynomials, and related functions")).


## §10.49(iii) Rayleigh’s Formulas

:::{note}
**Keywords:**

[Rayleigh’s formulas](http://dlmf.nist.gov/search/search?q=Rayleigh%20formulas) , [spherical Bessel functions](http://dlmf.nist.gov/search/search?q=spherical%20Bessel%20functions)

**Notes:**

For the first of( 10.49.14 ) combine the second of ( 10.51.3 ), with $n=0$ and $m=n$ , and the first of ( 10.49.3 ). Similarly for the other results.

**See also:**

Annotations for §10.49 and Ch.10
:::

<a id="E14"></a>

<a id="Ex16"></a>
$$
\displaystyle\mathsf{j}_{n}\left(z\right) \displaystyle=z^{n}\left(-\frac{1}{z}\frac{\mathrm{d}}{\mathrm{d}z}\right)^{n}\frac{\sin z}{z}, \tag{10.49.14}
$$

<a id="Ex17"></a>
$$
\displaystyle\mathsf{y}_{n}\left(z\right) \displaystyle=-z^{n}\left(-\frac{1}{z}\frac{\mathrm{d}}{\mathrm{d}z}\right)^{n}\frac{\cos z}{z}.
$$

:::{note}
**Symbols:**

$\cos\NVar{z}$: cosine function , $\frac{\mathrm{d}\NVar{f}}{\mathrm{d}\NVar{x}}$: derivative of $f$ with respect to $x$ , $\sin\NVar{z}$: sine function , $\mathsf{j}_{\NVar{n}}\left(\NVar{z}\right)$: spherical Bessel function of the first kind , $\mathsf{y}_{\NVar{n}}\left(\NVar{z}\right)$: spherical Bessel function of the second kind , $n$: integer and $z$: complex variable

**A&S Ref:**

10.1.25, 10.1.26

**Referenced by:**

§10.49(iii)

**See also:**

Annotations for §10.49(iii) , §10.49 and Ch.10
:::

<a id="E15"></a>

<a id="Ex18"></a>
$$
\displaystyle{\mathsf{i}^{(1)}_{n}}\left(z\right) \displaystyle=z^{n}\left(\frac{1}{z}\frac{\mathrm{d}}{\mathrm{d}z}\right)^{n}\frac{\sinh z}{z}, \tag{10.49.15}
$$

<a id="Ex19"></a>
$$
\displaystyle{\mathsf{i}^{(2)}_{n}}\left(z\right) \displaystyle=z^{n}\left(\frac{1}{z}\frac{\mathrm{d}}{\mathrm{d}z}\right)^{n}\frac{\cosh z}{z}.
$$

:::{note}
**Symbols:**

$\frac{\mathrm{d}\NVar{f}}{\mathrm{d}\NVar{x}}$: derivative of $f$ with respect to $x$ , $\cosh\NVar{z}$: hyperbolic cosine function , $\sinh\NVar{z}$: hyperbolic sine function , ${\mathsf{i}^{(1)}_{\NVar{n}}}\left(\NVar{z}\right)$: modified spherical Bessel function , ${\mathsf{i}^{(2)}_{\NVar{n}}}\left(\NVar{z}\right)$: modified spherical Bessel function , $n$: integer and $z$: complex variable

**A&S Ref:**

10.2.24, 10.2 25

**See also:**

Annotations for §10.49(iii) , §10.49 and Ch.10
:::


<a id="E16"></a>
$$
\mathsf{k}_{n}\left(z\right)=(-1)^{n}\tfrac{1}{2}\pi z^{n}\left(\frac{1}{z}\frac{\mathrm{d}}{\mathrm{d}z}\right)^{n}\frac{e^{-z}}{z}. \tag{10.49.16}
$$


## §10.49(iv) Sums or Differences of Squares

:::{note}
**Keywords:**

[explicit formulas](http://dlmf.nist.gov/search/search?q=explicit%20formulas) , [spherical Bessel functions](http://dlmf.nist.gov/search/search?q=spherical%20Bessel%20functions) , [sums or differences of squares](http://dlmf.nist.gov/search/search?q=sums%20or%20differences%20of%20squares)

**Notes:**

From ( 10.18.6 ), ( 10.47.3 ), and ( 10.47.4 ), ${\mathsf{j}_{n}}^{2}\left(z\right)+{\mathsf{y}_{n}}^{2}\left(z\right)=(\pi/(2z)){M_{n+\frac{1}{2}}}^{2}\left(z\right)$ . Then apply ( 10.18.17 ). To derive ( 10.49.20 ) combine ( 10.47.12 ) and ( 10.49.18 ).

**See also:**

Annotations for §10.49 and Ch.10
:::

Denote


<a id="E17"></a>
$$
s_{k}(n+\tfrac{1}{2})=\frac{(2k)!(n+k)!}{2^{2k}(k!)^{2}(n-k)!}, \tag{10.49.17}
$$

Then


<a id="E18"></a>
$$
{\mathsf{j}_{n}}^{2}\left(z\right)+{\mathsf{y}_{n}}^{2}\left(z\right)=\sum_{k=0}^{n}\frac{s_{k}(n+\frac{1}{2})}{z^{2k+2}}. \tag{10.49.18}
$$

<a id="E19"></a>

<a id="Ex20"></a>
$$
\displaystyle{\mathsf{j}_{0}}^{2}\left(z\right)+{\mathsf{y}_{0}}^{2}\left(z\right) \displaystyle=z^{-2}, \tag{10.49.19}
$$

<a id="Ex21"></a>
$$
\displaystyle{\mathsf{j}_{1}}^{2}\left(z\right)+{\mathsf{y}_{1}}^{2}\left(z\right) \displaystyle=z^{-2}+z^{-4},
$$

<a id="Ex22"></a>
$$
\displaystyle{\mathsf{j}_{2}}^{2}\left(z\right)+{\mathsf{y}_{2}}^{2}\left(z\right) \displaystyle=z^{-2}+3z^{-4}+9z^{-6}.
$$

:::{note}
**Symbols:**

$\mathsf{j}_{\NVar{n}}\left(\NVar{z}\right)$: spherical Bessel function of the first kind , $\mathsf{y}_{\NVar{n}}\left(\NVar{z}\right)$: spherical Bessel function of the second kind and $z$: complex variable

**A&S Ref:**

10.1.28--10.1.30

**See also:**

Annotations for §10.49(iv) , §10.49 and Ch.10
:::


<a id="E20"></a>
$$
\left({\mathsf{i}^{(1)}_{n}}\left(z\right)\right)^{2}-\left({\mathsf{i}^{(2)}_{n}}\left(z\right)\right)^{2}=(-1)^{n+1}\sum_{k=0}^{n}(-1)^{k}\frac{s_{k}(n+\frac{1}{2})}{z^{2k+2}}. \tag{10.49.20}
$$

<a id="E21"></a>

<a id="Ex23"></a>
$$
\displaystyle\Big{(}{\mathsf{i}^{(1)}_{0}}\left(z\right)\Big{)}^{2}-\Big{(}{\mathsf{i}^{(2)}_{0}}\left(z\right)\Big{)}^{2} \displaystyle=-z^{-2}, \tag{10.49.21}
$$

<a id="Ex24"></a>
$$
\displaystyle\Big{(}{\mathsf{i}^{(1)}_{1}}\left(z\right)\Big{)}^{2}-\Big{(}{\mathsf{i}^{(2)}_{1}}\left(z\right)\Big{)}^{2} \displaystyle=z^{-2}-z^{-4},
$$

<a id="Ex25"></a>
$$
\displaystyle\Big{(}{\mathsf{i}^{(1)}_{2}}\left(z\right)\Big{)}^{2}-\Big{(}{\mathsf{i}^{(2)}_{2}}\left(z\right)\Big{)}^{2} \displaystyle=-z^{-2}+3z^{-4}-9z^{-6}.
$$

:::{note}
**Symbols:**

${\mathsf{i}^{(1)}_{\NVar{n}}}\left(\NVar{z}\right)$: modified spherical Bessel function , ${\mathsf{i}^{(2)}_{\NVar{n}}}\left(\NVar{z}\right)$: modified spherical Bessel function and $z$: complex variable

**A&S Ref:**

10.2.27--10.2.29

**See also:**

Annotations for §10.49(iv) , §10.49 and Ch.10
:::
