# §10.51 Recurrence Relations and Derivatives

:::{note}
**See also:**

Annotations for Ch.10
:::


## §10.51(i) Unmodified Functions

:::{note}
**Keywords:**

[derivatives](http://dlmf.nist.gov/search/search?q=derivatives) , [recurrence relations](http://dlmf.nist.gov/search/search?q=recurrence%20relations) , [spherical Bessel functions](http://dlmf.nist.gov/search/search?q=spherical%20Bessel%20functions)

**Notes:**

For ( 10.51.1 ) and ( 10.51.2 ) combine ( 10.6.1 ) and ( 10.6.2 ) with the definitions ( 10.47.3 )–( 10.47.5 ). For ( 10.51.3 ) apply induction with the aid of ( 10.51.2 ).

**See also:**

Annotations for §10.51 and Ch.10
:::

Let $f_{n}(z)$ denote any of $\mathsf{j}_{n}\left(z\right)$ , $\mathsf{y}_{n}\left(z\right)$ , ${\mathsf{h}^{(1)}_{n}}\left(z\right)$ , or ${\mathsf{h}^{(2)}_{n}}\left(z\right)$ . Then

<a id="E1"></a>

<a id="Ex1"></a>
$$
\displaystyle f_{n-1}(z)+f_{n+1}(z) \displaystyle=((2n+1)/z)f_{n}(z), \tag{10.51.1}
$$

<a id="Ex2"></a>
$$
\displaystyle nf_{n-1}(z)-(n+1)f_{n+1}(z) \displaystyle=(2n+1)f_{n}^{\prime}(z),
$$

:::{note}
**Symbols:**

$n$: integer , $z$: complex variable and $f_{n}(z)$: a spherical Bessel function

**A&S Ref:**

10.1.19, 10.1.20

**Referenced by:**

§10.50 , §10.51(i) , §10.56

**See also:**

Annotations for §10.51(i) , §10.51 and Ch.10
:::

<a id="E2"></a>

<a id="Ex3"></a>
$$
\displaystyle f_{n}^{\prime}(z) \displaystyle=f_{n-1}(z)-((n+1)/z)f_{n}(z), \tag{10.51.2}
$$

<a id="Ex4"></a>
$$
\displaystyle f_{n}^{\prime}(z) \displaystyle=-f_{n+1}(z)+(n/z)f_{n}(z),
$$

:::{note}
**Symbols:**

$n$: integer , $z$: complex variable and $f_{n}(z)$: a spherical Bessel function

**A&S Ref:**

10.1.21, 10.1.22

**Referenced by:**

§10.50 , §10.51(i)

**See also:**

Annotations for §10.51(i) , §10.51 and Ch.10
:::

<a id="E3"></a>

<a id="Ex5"></a>
$$
\displaystyle\left(\frac{1}{z}\frac{\mathrm{d}}{\mathrm{d}z}\right)^{m}(z^{n+1}f_{n}(z)) \displaystyle=z^{n-m+1}f_{n-m}(z), \tag{10.51.3}
$$

<a id="Ex6"></a>
$$
\displaystyle\left(\frac{1}{z}\frac{\mathrm{d}}{\mathrm{d}z}\right)^{m}(z^{-n}f_{n}(z)) \displaystyle=(-1)^{m}z^{-n-m}f_{n+m}(z),
$$

:::{note}
**Symbols:**

$\frac{\mathrm{d}\NVar{f}}{\mathrm{d}\NVar{x}}$: derivative of $f$ with respect to $x$ , $m$: integer , $n$: integer , $z$: complex variable and $f_{n}(z)$: a spherical Bessel function

**A&S Ref:**

10.1.23, 10.1.24

**Referenced by:**

§10.49(iii) , §10.51(i)

**See also:**

Annotations for §10.51(i) , §10.51 and Ch.10
:::


## §10.51(ii) Modified Functions

:::{note}
**Keywords:**

[derivatives](http://dlmf.nist.gov/search/search?q=derivatives) , [recurrence relations](http://dlmf.nist.gov/search/search?q=recurrence%20relations) , [spherical Bessel functions](http://dlmf.nist.gov/search/search?q=spherical%20Bessel%20functions)

**Notes:**

For ( 10.51.4 ) and ( 10.51.5 ) combine ( 10.29.1 ) and ( 10.29.2 ) with the definitions ( 10.47.7 ) and ( 10.47.9 ). For ( 10.51.6 ) apply induction with the aid of ( 10.51.5 ).

**See also:**

Annotations for §10.51 and Ch.10
:::

Let $g_{n}(z)$ denote ${\mathsf{i}^{(1)}_{n}}\left(z\right)$ , ${\mathsf{i}^{(2)}_{n}}\left(z\right)$ , or $(-1)^{n}$ $\mathsf{k}_{n}\left(z\right)$ . Then

<a id="E4"></a>

<a id="Ex7"></a>
$$
\displaystyle g_{n-1}(z)-g_{n+1}(z) \displaystyle=((2n+1)/z)g_{n}(z) \tag{10.51.4}
$$

<a id="Ex8"></a>
$$
\displaystyle ng_{n-1}(z)+(n+1)g_{n+1}(z) \displaystyle=(2n+1)g_{n}^{\prime}(z),
$$

:::{note}
**Symbols:**

$n$: integer , $z$: complex variable and $g_{n}(z)$: a spherical Bessel function

**A&S Ref:**

10.2.18, 10.2.19

**Referenced by:**

§10.51(ii)

**See also:**

Annotations for §10.51(ii) , §10.51 and Ch.10
:::

<a id="E5"></a>

<a id="Ex9"></a>
$$
\displaystyle g_{n}^{\prime}(z) \displaystyle=g_{n-1}(z)-((n+1)/z)g_{n}(z), \tag{10.51.5}
$$

<a id="Ex10"></a>
$$
\displaystyle g_{n}^{\prime}(z) \displaystyle=g_{n+1}(z)+(n/z)g_{n}(z),
$$

:::{note}
**Symbols:**

$n$: integer , $z$: complex variable and $g_{n}(z)$: a spherical Bessel function

**A&S Ref:**

10.2.20, 10.2.21

**Referenced by:**

§10.51(ii)

**See also:**

Annotations for §10.51(ii) , §10.51 and Ch.10
:::

<a id="E6"></a>

<a id="Ex11"></a>
$$
\displaystyle\left(\frac{1}{z}\frac{\mathrm{d}}{\mathrm{d}z}\right)^{m}(z^{n+1}g_{n}(z)) \displaystyle=z^{n-m+1}g_{n-m}(z), \tag{10.51.6}
$$

<a id="Ex12"></a>
$$
\displaystyle\left(\frac{1}{z}\frac{\mathrm{d}}{\mathrm{d}z}\right)^{m}(z^{-n}g_{n}(z)) \displaystyle=z^{-n-m}g_{n+m}(z),
$$

:::{note}
**Symbols:**

$\frac{\mathrm{d}\NVar{f}}{\mathrm{d}\NVar{x}}$: derivative of $f$ with respect to $x$ , $m$: integer , $n$: integer , $z$: complex variable and $g_{n}(z)$: a spherical Bessel function

**A&S Ref:**

10.2.22, 10.2.23

**Referenced by:**

§10.51(ii)

**See also:**

Annotations for §10.51(ii) , §10.51 and Ch.10
:::
