# §19.29 Reduction of General Elliptic Integrals

:::{note}
**Keywords:**

[reduction of general elliptic integrals](http://dlmf.nist.gov/search/search?q=reduction%20of%20general%20elliptic%20integrals) , [symmetric elliptic integrals](http://dlmf.nist.gov/search/search?q=symmetric%20elliptic%20integrals)

**See also:**

Annotations for Ch.19
:::


## §19.29(i) Reduction Theorems

:::{note}
**Keywords:**

[general elliptic integrals](http://dlmf.nist.gov/search/search?q=general%20elliptic%20integrals) , [reduction to symmetric elliptic integrals](http://dlmf.nist.gov/search/search?q=reduction%20to%20symmetric%20elliptic%20integrals)

**Notes:**

For ( 19.29.4 ) see Carlson ([1998](./bib/C.html#bib442 "Elliptic Integrals: Symmetry and Symbolic Integration"), (3.6)). For ( 19.29.7 ), a special case of ( 19.29.8 ), see also Carlson ([1987](./bib/C.html#bib438 "A table of elliptic integrals of the second kind"), (4.14)). For ( 19.29.8 ) see Carlson ([1999](./bib/C.html#bib443 "Toward symbolic integration of elliptic integrals"), (4.10)) and Carlson ([1988](./bib/C.html#bib439 "A table of elliptic integrals of the third kind"), (5.6)). For ( 19.29.10 ) see Byrd and Friedman ([1971](./bib/B.html#bib400 "Handbook of Elliptic Integrals for Engineers and Scientists"), p. 76, Eq. (234.13), and p. 74) for notation. Then use Carlson ([2006b](./bib/C.html#bib448 "Table of integrals of squared Jacobian elliptic functions and reductions of related hypergeometric R -functions"), (3.2)) with $(p,q,r)=(n,d,c)$ for reduction to $R_{D}$ .

**Referenced by:**

§19.15 , §19.36(i)

**See also:**

Annotations for §19.29 and Ch.19
:::

These theorems reduce integrals over a real interval $(y,x)$ of certain integrands containing the square root of a quartic or cubic polynomial to symmetric integrals over $(0,\infty)$ containing the square root of a cubic polynomial (compare § 19.16(i) ). Let

<a id="E1"></a>

<a id="Ex1"></a>
$$
\displaystyle X_{\alpha} \displaystyle=\sqrt{a_{\alpha}+b_{\alpha}x}, \tag{19.29.1}
$$

<a id="Ex2"></a>
$$
\displaystyle Y_{\alpha} \displaystyle=\sqrt{a_{\alpha}+b_{\alpha}y},
$$

:::{note}
**Symbols:**

$X_{\alpha}$ , $Y_{\alpha}$ and $\alpha$: parameter

**Referenced by:**

§19.29(ii)

**See also:**

Annotations for §19.29(i) , §19.29 and Ch.19
:::


<a id="E2"></a>
$$
d_{\alpha\beta}=a_{\alpha}b_{\beta}-a_{\beta}b_{\alpha}, \tag{19.29.2}
$$

and assume that the line segment with endpoints $a_{\alpha}+b_{\alpha}x$ and $a_{\alpha}+b_{\alpha}y$ lies in $\mathbb{C}\setminus(-\infty,0)$ for $1\leq\alpha\leq 4$ . If


<a id="E3"></a>
$$
s(t)=\prod_{\alpha=1}^{4}\sqrt{a_{\alpha}+b_{\alpha}t} \tag{19.29.3}
$$

and $\alpha,\beta,\gamma,\delta$ is any permutation of the numbers $1,2,3,4$ , then


<a id="E4"></a>
$$
\int_{y}^{x}\frac{\,\mathrm{d}t}{s(t)}=2R_{F}\left(U_{12}^{2},U_{13}^{2},U_{23}^{2}\right), \tag{19.29.4}
$$

where

<a id="E5"></a>

<a id="Ex3"></a>
$$
\displaystyle U_{\alpha\beta} \displaystyle=(X_{\alpha}X_{\beta}Y_{\gamma}Y_{\delta}+Y_{\alpha}Y_{\beta}X_{\gamma}X_{\delta})/(x-y), \tag{19.29.5}
$$

<a id="Ex4"></a>
$$
\displaystyle U_{\alpha\beta} \displaystyle=U_{\beta\alpha}=U_{\gamma\delta}=U_{\delta\gamma},
$$

<a id="Ex5"></a>
$$
\displaystyle U_{\alpha\beta}^{2}-U_{\alpha\gamma}^{2} \displaystyle=d_{\alpha\delta}d_{\beta\gamma}.
$$

:::{note}
**Symbols:**

$X_{\alpha}$ , $U_{n}$ , $Y_{\alpha}$ , $d_{\alpha\beta}$ , $\alpha$: parameter , $\beta$: parameter , $\gamma$: parameter and $\delta$: parameter

**See also:**

Annotations for §19.29(i) , §19.29 and Ch.19
:::

There are only three distinct $U$ ’s with subscripts $\leq 4$ , and at most one of them can be 0 because the $d$ ’s are nonzero. Then

<a id="E6"></a>

<a id="Ex6"></a>
$$
\displaystyle{U_{\alpha\beta}} {\displaystyle=\sqrt{b_{\alpha}}\sqrt{b_{\beta}}Y_{\gamma}Y_{\delta}+Y_{\alpha}Y_{\beta}\sqrt{b_{\gamma}}\sqrt{b_{\delta}},} \tag{19.29.6}
$$

<a id="Ex7"></a>
$$
\displaystyle U_{\alpha\beta} \displaystyle=X_{\alpha}X_{\beta}\sqrt{-b_{\gamma}}\sqrt{-b_{\delta}}+\sqrt{-b_{\alpha}}\sqrt{-b_{\beta}}X_{\gamma}X_{\delta},
$$

:::{note}
**Symbols:**

$X_{\alpha}$ , $U_{n}$ , $Y_{\alpha}$ , $\alpha$: parameter , $\beta$: parameter , $\gamma$: parameter and $\delta$: parameter

**See also:**

Annotations for §19.29(i) , §19.29 and Ch.19
:::


<a id="E7"></a>
$$
\int_{y}^{x}\frac{a_{\alpha}+b_{\alpha}t}{a_{\delta}+b_{\delta}t}\frac{\,\mathrm{d}t}{s(t)}=\tfrac{2}{3}d_{\alpha\beta}d_{\alpha\gamma}R_{D}\left(U_{\alpha\beta}^{2},U_{\alpha\gamma}^{2},U_{\alpha\delta}^{2}\right)+\frac{2X_{\alpha}Y_{\alpha}}{X_{\delta}Y_{\delta}U_{\alpha\delta}}, \tag{19.29.7}
$$


<a id="E8"></a>
$$
\int_{y}^{x}\frac{a_{\alpha}+b_{\alpha}t}{a_{5}+b_{5}t}\frac{\,\mathrm{d}t}{s(t)}=\frac{2}{3}\frac{d_{\alpha\beta}d_{\alpha\gamma}d_{\alpha\delta}}{d_{\alpha 5}}R_{J}\left(U_{12}^{2},U_{13}^{2},U_{23}^{2},U_{\alpha 5}^{2}\right)+2R_{C}\left(S_{\alpha 5}^{2},Q_{\alpha 5}^{2}\right), \tag{19.29.8}
$$

where

<a id="E9"></a>

<a id="Ex8"></a>
$$
\displaystyle U_{\alpha 5}^{2} \displaystyle=U_{\alpha\beta}^{2}-\frac{d_{\alpha\gamma}d_{\alpha\delta}d_{\beta 5}}{d_{\alpha 5}}=U_{\beta\gamma}^{2}-\frac{d_{\alpha\beta}d_{\alpha\gamma}d_{\delta 5}}{d_{\alpha 5}}\neq 0, \tag{19.29.9}
$$

<a id="Ex9"></a>
$$
\displaystyle S_{\alpha 5} \displaystyle=\frac{1}{x-y}\left(\frac{X_{\beta}X_{\gamma}X_{\delta}}{X_{\alpha}}Y_{5}^{2}+\frac{Y_{\beta}Y_{\gamma}Y_{\delta}}{Y_{\alpha}}X_{5}^{2}\right),
$$

<a id="Ex10"></a>
$$
\displaystyle Q_{\alpha 5} \displaystyle=\frac{X_{5}Y_{5}}{X_{\alpha}Y_{\alpha}}U_{\alpha 5}\neq 0,
$$

<a id="Ex11"></a>
$$
\displaystyle S_{\alpha 5}^{2}-Q_{\alpha 5}^{2} \displaystyle=\frac{d_{\beta 5}d_{\gamma 5}d_{\delta 5}}{d_{\alpha 5}}.
$$

:::{note}
**Symbols:**

$X_{\alpha}$ , $U_{n}$ , $S_{n}$ , $Q_{\alpha\beta}$ , $Y_{\alpha}$ , $d_{\alpha\beta}$ , $\alpha$: parameter , $\beta$: parameter , $\gamma$: parameter and $\delta$: parameter

**See also:**

Annotations for §19.29(i) , §19.29 and Ch.19
:::

The Cauchy principal value is taken when $U_{\alpha 5}^{2}$ or $Q_{\alpha 5}^{2}$ is real and negative. Cubic cases of these formulas are obtained by setting one of the factors in ( 19.29.3 ) equal to 1.

The advantages of symmetric integrals for tables of integrals and symbolic integration are illustrated by ( 19.29.4 ) and its cubic case, which replace the $8+8+12=28$ formulas in Gradshteyn and Ryzhik ([2015](./bib/G.html#bib972 "Table of integrals, series, and products"), 3.147, 3.131, 3.152) after taking $x^{2}$ as the variable of integration in 3.152. Moreover, the requirement that one limit of integration be a branch point of the integrand is eliminated without doubling the number of standard integrals in the result. ( 19.29.7 ) subsumes all 72 formulas in Gradshteyn and Ryzhik ([2015](./bib/G.html#bib972 "Table of integrals, series, and products"), 3.168), and its cubic cases similarly replace the $18+36+18=72$ formulas in Gradshteyn and Ryzhik ([2015](./bib/G.html#bib972 "Table of integrals, series, and products"), 3.133, 3.142, and 3.141(1-18)). For example, 3.142(2) is included as


<a id="E10"></a>
$$
\int_{u}^{b}\sqrt{\frac{a-t}{(b-t)(t-c)^{3}}}\,\mathrm{d}t=-\tfrac{2}{3}{(a-b)}{(b-u)}^{3/2}R_{D}+\frac{2}{b-c}\sqrt{\frac{(a-u)(b-u)}{u-c}}, \tag{19.29.10}
$$

where the arguments of the $R_{D}$ function are, in order, $(a-b)(u-c)$ , $(b-c)(a-u)$ , $(a-b)(b-c)$ .


## §19.29(ii) Reduction to Basic Integrals

:::{note}
**Keywords:**

[basic elliptic integrals](http://dlmf.nist.gov/search/search?q=basic%20elliptic%20integrals) , [general elliptic integrals](http://dlmf.nist.gov/search/search?q=general%20elliptic%20integrals) , [reduction to basic elliptic integrals](http://dlmf.nist.gov/search/search?q=reduction%20to%20basic%20elliptic%20integrals)

**Referenced by:**

§19.15 , §19.34

**See also:**

Annotations for §19.29 and Ch.19
:::

( 19.2.3 ) can be written


<a id="E11"></a>
$$
I(\mathbf{m})=\int_{y}^{x}\prod_{\alpha=1}^{h}(a_{\alpha}+b_{\alpha}t)^{-1/2}\prod_{j=1}^{n}(a_{j}+b_{j}t)^{m_{j}}\,\mathrm{d}t, \tag{19.29.11}
$$

where $x>y$ , $h=3$ or 4, $n\geq h$ , and $m_{j}$ is an integer. Define


<a id="E12"></a>
$$
\mathbf{m}=(m_{1},\dots,m_{n})=\sum_{j=1}^{n}m_{j}\mathbf{e}_{j}, \tag{19.29.12}
$$

where $\mathbf{e}_{j}$ is an $n$ -tuple with 1 in the $j$ th position and 0’s elsewhere. Define also $\boldsymbol{{0}}=(0,\dots,0)$ and retain the notation and conditions associated with ( 19.29.1 ) and ( 19.29.2 ). The integrals in ( 19.29.4 ), ( 19.29.7 ), and ( 19.29.8 ) are $I(\boldsymbol{{0}})$ , $I(\mathbf{e}_{\alpha}-\mathbf{e}_{\delta})$ , and $I(\mathbf{e}_{\alpha}-\mathbf{e}_{5})$ , respectively.

The only cases of $I(\mathbf{m})$ that are integrals of the *first kind* are the two ( $h=3$ or 4) with $\mathbf{m}=\boldsymbol{{0}}$ . The only cases that are integrals of the *third kind* are those in which at least one $m_{j}$ with $j>h$ is a negative integer and those in which $h=4$ and $\sum_{j=1}^{n}m_{j}$ is a positive integer. All other cases are integrals of the *second kind* .

$I(\mathbf{m})$ can be reduced to a linear combination of *basic integrals* and algebraic functions. In the cubic case ( $h=3$ ) the basic integrals are

<a id="E13"></a>

<a id="Ex12"></a>
$$
I(\boldsymbol{{0}}); \tag{19.29.13}
$$

<a id="Ex13"></a>
$$
I(-\mathbf{e}_{j}),
$$

:::{note}
**Symbols:**

$n$: nonnegative integer and $I(\mathbf{m})$: integral

**See also:**

Annotations for §19.29(ii) , §19.29 and Ch.19
:::

In the quartic case ( $h=4$ ) the basic integrals are

<a id="E14"></a>

<a id="Ex14"></a>
$$
I(\boldsymbol{{0}}); \tag{19.29.14}
$$

<a id="Ex15"></a>
$$
I(-\mathbf{e}_{j}),
$$

<a id="Ex16"></a>
$$
I(\mathbf{e}_{\alpha}),
$$

:::{note}
**Symbols:**

$n$: nonnegative integer , $I(\mathbf{m})$: integral and $\alpha$: parameter

**See also:**

Annotations for §19.29(ii) , §19.29 and Ch.19
:::

Basic integrals of type $I(-\mathbf{e}_{j})$ , $1\leq j\leq h$ , are not linearly independent, nor are those of type $I(\mathbf{e}_{j})$ , $1\leq j\leq 4$ .

The reduction of $I(\mathbf{m})$ is carried out by a relation derived from partial fractions and by use of two recurrence relations. These are given in Carlson ([1999](./bib/C.html#bib443 "Toward symbolic integration of elliptic integrals"), (2.19), (3.5), (3.11)) and simplified in Carlson ([2002](./bib/C.html#bib444 "Three improvements in reduction and computation of elliptic integrals"), (1.10), (1.7), (1.8)) by means of modified definitions. Partial fractions provide a reduction to integrals in which $\mathbf{m}$ has at most one nonzero component, and these are then reduced to basic integrals by the recurrence relations. A special case of Carlson ([1999](./bib/C.html#bib443 "Toward symbolic integration of elliptic integrals"), (2.19)) is given by


<a id="E15"></a>
$$
b_{j}I(\mathbf{e}_{l}-\mathbf{e}_{j})=d_{lj}I(-\mathbf{e}_{j})+b_{l}I(\boldsymbol{{0}}), \tag{19.29.15}
$$

which shows how to express the basic integral $I(-\mathbf{e}_{j})$ in terms of symmetric integrals by using ( 19.29.4 ) and either ( 19.29.7 ) or ( 19.29.8 ). The first choice gives a formula that includes the 18+9+18 = 45 formulas in Gradshteyn and Ryzhik ([2015](./bib/G.html#bib972 "Table of integrals, series, and products"), 3.133, 3.156, 3.158), and the second choice includes the 8+8+8+12 = 36 formulas in Gradshteyn and Ryzhik ([2015](./bib/G.html#bib972 "Table of integrals, series, and products"), 3.151, 3.149, 3.137, 3.157) (after setting $x^{2}=t$ in some cases).

If $h=3$ , then the recurrence relation (Carlson ([1999](./bib/C.html#bib443 "Toward symbolic integration of elliptic integrals"), (3.5))) has the special case


<a id="E16"></a>
$$
b_{\beta}b_{\gamma}I(\mathbf{e}_{\alpha})=d_{\alpha\beta}d_{\alpha\gamma}I(-\mathbf{e}_{\alpha})+2b_{\alpha}\left(\frac{s(x)}{a_{\alpha}+b_{\alpha}x}-\frac{s(y)}{a_{\alpha}+b_{\alpha}y}\right), \tag{19.29.16}
$$

where $\alpha,\beta,\gamma$ is any permutation of the numbers $1,2,3$ , and


<a id="E17"></a>
$$
s(t)=\prod_{\alpha=1}^{3}\sqrt{a_{\alpha}+b_{\alpha}t}. \tag{19.29.17}
$$

(This shows why $I(\mathbf{e}_{\alpha})$ is not needed as a basic integral in the cubic case.) In the quartic case this recurrence relation has an extra term in $I(2\mathbf{e}_{\alpha})$ , and hence $I(\mathbf{e}_{\alpha})$ , $1\leq\alpha\leq 4$ , is a basic integral. It can be expressed in terms of symmetric integrals by setting $a_{5}=1$ and $b_{5}=0$ in ( 19.29.8 ).

The other recurrence relation is


<a id="E18"></a>
$$
b_{j}^{q}I(q\mathbf{e}_{l})=\sum_{r=0}^{q}\genfrac{(}{)}{0.0pt}{}{q}{r}b_{l}^{r}d_{lj}^{q-r}I(r\mathbf{e}_{j}), \tag{19.29.18}
$$

see Carlson ([1999](./bib/C.html#bib443 "Toward symbolic integration of elliptic integrals"), (3.11)). An example that uses ( 19.29.15 )–( 19.29.18 ) is given in § [19.34](./19.34.md "§19.34 Mutual Inductance of Coaxial Circles ‣ Applications ‣ Chapter 19 Elliptic Integrals") .

For an implementation by James FitzSimons of the method for reducing $I(\mathbf{m})$ to basic integrals and extensive tables of such reductions, see Carlson ([1999](./bib/C.html#bib443 "Toward symbolic integration of elliptic integrals")) and Carlson and FitzSimons ([2000](./bib/C.html#bib450 "Reduction theorems for elliptic integrands with the square root of two quadratic factors")).

Another method of reduction is given in Gray ([2002](./bib/G.html#bib978 "Automatic reduction of elliptic integrals using Carlson’s relations")). It depends primarily on multivariate recurrence relations that replace one integral by two or more.


## §19.29(iii) Examples

:::{note}
**Keywords:**

[general elliptic integrals](http://dlmf.nist.gov/search/search?q=general%20elliptic%20integrals) , [reduction of general elliptic integrals](http://dlmf.nist.gov/search/search?q=reduction%20of%20general%20elliptic%20integrals) , [reduction to symmetric elliptic integrals](http://dlmf.nist.gov/search/search?q=reduction%20to%20symmetric%20elliptic%20integrals) , [symmetric elliptic integrals](http://dlmf.nist.gov/search/search?q=symmetric%20elliptic%20integrals)

**Notes:**

Take $t^{2}$ as a new variable where appropriate. Then factor quadratic polynomials, use ( 19.29.4 ), and apply ( 19.22.18 ) to remove any complex quantities. For ( 19.29.20 ) use ( 19.29.7 ) with $a_{\alpha}+b_{\alpha}t=t$ and $a_{\delta}+b_{\delta}t=1$ . For ( 19.29.21 ) use ( 19.29.7 ) with $a_{\alpha}+b_{\alpha}t=1$ and $a_{\delta}+b_{\delta}t=t$ . With regard to ( 19.29.28 ) see Carlson ([1977a](./bib/C.html#bib433 "Elliptic integrals of the first kind"), p. 238).

**See also:**

Annotations for §19.29 and Ch.19
:::

The first formula replaces ( 19.14.4 )–( 19.14.10 ). Define $Q_{j}(t)=a_{j}+b_{j}t^{2}$ , $j=1,2$ , and assume both $Q$ ’s are positive for $0\leq y<t<x$ . Then


<a id="E19"></a>
$$
\int_{y}^{x}\frac{\,\mathrm{d}t}{\sqrt{Q_{1}(t)Q_{2}(t)}}=R_{F}\left(U^{2}+a_{1}b_{2},U^{2}+a_{2}b_{1},U^{2}\right), \tag{19.29.19}
$$


<a id="E20"></a>
$$
\int_{y}^{x}\frac{t^{2}\,\mathrm{d}t}{\sqrt{Q_{1}(t)Q_{2}(t)}}=\tfrac{1}{3}a_{1}a_{2}R_{D}\left(U^{2}+a_{1}b_{2},U^{2}+a_{2}b_{1},U^{2}\right)+(xy/U), \tag{19.29.20}
$$

and


<a id="E21"></a>
$$
\int_{y}^{x}\frac{\,\mathrm{d}t}{t^{2}\sqrt{Q_{1}(t)Q_{2}(t)}}=\tfrac{1}{3}b_{1}b_{2}R_{D}\left(U^{2}+a_{1}b_{2},U^{2}+a_{2}b_{1},U^{2}\right)+(xyU)^{-1}, \tag{19.29.21}
$$

where


<a id="E22"></a>
$$
(x^{2}-y^{2})U=x\sqrt{Q_{1}(y)Q_{2}(y)}+y\sqrt{Q_{1}(x)Q_{2}(x)}. \tag{19.29.22}
$$

If both square roots in ( 19.29.22 ) are 0, then the indeterminacy in the two preceding equations can be removed by using ( 19.27.8 ) to evaluate the integral as $R_{G}\left(a_{1}b_{2},a_{2}b_{1},0\right)$ multiplied either by $-2/(b_{1}b_{2})$ or by $-2/(a_{1}a_{2})$ in the cases of ( 19.29.20 ) or ( 19.29.21 ), respectively. If $x=\infty$ , then $U$ is found by taking the limit. For example,


<a id="E23"></a>
$$
\int_{y}^{\infty}\frac{\,\mathrm{d}t}{\sqrt{(t^{2}+a^{2})(t^{2}-b^{2})}}=R_{F}\left(y^{2}+a^{2},y^{2}-b^{2},y^{2}\right). \tag{19.29.23}
$$

Next, for $j=1,2$ , define $Q_{j}(t)=f_{j}+g_{j}t+h_{j}t^{2}$ , and assume both $Q$ ’s are positive for $y<t<x$ . If each has real zeros, then ( 19.29.4 ) may be simpler than


<a id="E24"></a>
$$
\int_{y}^{x}\frac{\,\mathrm{d}t}{\sqrt{Q_{1}(t)Q_{2}(t)}}=4R_{F}\left(U,U+D_{12}+V,U+D_{12}-V\right), \tag{19.29.24}
$$

where

<a id="E25"></a>

<a id="Ex17"></a>
$$
\displaystyle(x-y)^{2}U \displaystyle=S_{1}S_{2}, \tag{19.29.25}
$$

<a id="Ex18"></a>
$$
\displaystyle S_{j} \displaystyle=\left(\sqrt{Q_{j}(x)}+\sqrt{Q_{j}(y)}\right)^{2}-h_{j}(x-y)^{2},
$$

<a id="Ex19"></a>
$$
\displaystyle D_{jl} \displaystyle=2f_{j}h_{l}+2h_{j}f_{l}-g_{j}g_{l},
$$

<a id="Ex20"></a>
$$
\displaystyle V \displaystyle=\sqrt{D_{12}^{2}-D_{11}D_{22}}.
$$

:::{note}
**Symbols:**

$l$: nonnegative integer , $U$ , $D_{jl}$ , $S_{j}$ , $V$ , $Q(t^{2})$ , $f$: coefficient , $g$: coefficient and $h$: coefficient

**Referenced by:**

§19.29(iii)

**See also:**

Annotations for §19.29(iii) , §19.29 and Ch.19
:::

(The variables of $R_{F}$ are real and nonnegative unless both $Q$ ’s have real zeros and those of $Q_{1}$ interlace those of $Q_{2}$ .) If $Q_{1}(t)=(a_{1}+b_{1}t)(a_{2}+b_{2}t)$ , where both linear factors are positive for $y<t<x$ , and $Q_{2}(t)=f_{2}+g_{2}t+h_{2}t^{2}$ , then ( 19.29.25 ) is modified so that

<a id="E26"></a>

<a id="Ex21"></a>
$$
\displaystyle S_{1} \displaystyle=(X_{1}Y_{2}+Y_{1}X_{2})^{2}, \tag{19.29.26}
$$

<a id="Ex22"></a>
$$
\displaystyle X_{j} \displaystyle=\sqrt{a_{j}+b_{j}x},
$$

<a id="Ex23"></a>
$$
\displaystyle Y_{j} \displaystyle=\sqrt{a_{j}+b_{j}y},
$$

<a id="Ex24"></a>
$$
\displaystyle D_{12} \displaystyle=2a_{1}a_{2}h_{2}+2b_{1}b_{2}f_{2}-(a_{1}b_{2}+a_{2}b_{1})g_{2},
$$

<a id="Ex25"></a>
$$
\displaystyle D_{11} \displaystyle=-(a_{1}b_{2}-a_{2}b_{1})^{2}=-d_{12}^{2},
$$

:::{note}
**Symbols:**

$X_{\alpha}$ , $Y_{\alpha}$ , $D_{jl}$ , $S_{j}$ , $f$: coefficient , $g$: coefficient , $h$: coefficient and $d_{\alpha\beta}$

**Referenced by:**

§19.29(iii)

**See also:**

Annotations for §19.29(iii) , §19.29 and Ch.19
:::

with other quantities remaining as in ( 19.29.25 ). In the cubic case, in which $a_{2}=1$ , $b_{2}=0$ , ( 19.29.26 ) reduces further to

<a id="E27"></a>

<a id="Ex26"></a>
$$
\displaystyle S_{1} \displaystyle=(X_{1}+Y_{1})^{2}, \tag{19.29.27}
$$

<a id="Ex27"></a>
$$
\displaystyle D_{12} \displaystyle=2a_{1}h_{2}-b_{1}g_{2},
$$

<a id="Ex28"></a>
$$
\displaystyle D_{11} \displaystyle=-b_{1}^{2}.
$$

:::{note}
**Symbols:**

$X_{\alpha}$ , $Y_{\alpha}$ , $D_{jl}$ , $S_{j}$ , $g$: coefficient and $h$: coefficient

**See also:**

Annotations for §19.29(iii) , §19.29 and Ch.19
:::

For example, because $t^{3}-a^{3}=(t-a)(t^{2}+at+a^{2})$ , we find that when $0\leq a\leq y<x$


<a id="E28"></a>
$$
\int_{y}^{x}\frac{\,\mathrm{d}t}{\sqrt{t^{3}-a^{3}}}=4R_{F}\left(U,U-3a+2\sqrt{3}a,U-3a-2\sqrt{3}a\right), \tag{19.29.28}
$$

where

<a id="E29"></a>

<a id="Ex29"></a>
$$
\displaystyle(x-y)^{2}U \displaystyle=(\sqrt{x-a}+\sqrt{y-a})^{2}\left((\xi+\eta)^{2}-(x-y)^{2}\right), \tag{19.29.29}
$$

<a id="Ex30"></a>
$$
\displaystyle\xi \displaystyle=\sqrt{x^{2}+ax+a^{2}},
$$

<a id="Ex31"></a>
$$
\displaystyle\eta \displaystyle=\sqrt{y^{2}+ay+a^{2}}.
$$

:::{note}
**Symbols:**

$U$

**See also:**

Annotations for §19.29(iii) , §19.29 and Ch.19
:::

Lastly, define $Q(t^{2})=f+gt^{2}+ht^{4}$ and assume $Q(t^{2})$ is positive and monotonic for $y<t<x$ . Then


<a id="E30"></a>
$$
\int_{y}^{x}\frac{\,\mathrm{d}t}{\sqrt{Q(t^{2})}}=2R_{F}\left(U,U-g+2\sqrt{fh},U-g-2\sqrt{fh}\right), \tag{19.29.30}
$$

where


<a id="E31"></a>
$$
(x-y)^{2}U=\left(\sqrt{Q(x^{2})}+\sqrt{Q(y^{2})}\right)^{2}-h(x^{2}-y^{2})^{2}. \tag{19.29.31}
$$

For example, if $0\leq y\leq x$ and $a^{4}\geq 0$ , then


<a id="E32"></a>
$$
\int_{y}^{x}\frac{\,\mathrm{d}t}{\sqrt{t^{4}+a^{4}}}=2R_{F}\left(U,U+2a^{2},U-2a^{2}\right), \tag{19.29.32}
$$

where


<a id="E33"></a>
$$
(x-y)^{2}U=\left(\sqrt{x^{4}+a^{4}}+\sqrt{y^{4}+a^{4}}\right)^{2}-(x^{2}-y^{2})^{2}. \tag{19.29.33}
$$
