# §19.21 Connection Formulas

:::{note}
**Keywords:**

[connection formulas](http://dlmf.nist.gov/search/search?q=connection%20formulas) , [symmetric elliptic integrals](http://dlmf.nist.gov/search/search?q=symmetric%20elliptic%20integrals)

**See also:**

Annotations for Ch.19
:::


## §19.21(i) Complete Integrals

:::{note}
**Notes:**

To prove ( 19.21.1 ) see the text following ( 19.21.6 ), use ( 19.20.10 ), and analytic continuation. For ( 19.21.2 ) put $x=0$ in ( 19.21.9 ). For ( 19.21.3 ) put $x=0$ in ( 19.21.11 ) and ( 19.21.10 ). ( 19.21.6 ) is equivalent to Zill and Carlson ([1970](./bib/Z.html#bib2498 "Symmetric elliptic integrals of the third kind"), (7.15)).

**See also:**

Annotations for §19.21 and Ch.19
:::

Legendre’s relation ( 19.7.1 ) can be written


<a id="E1"></a>
$$
R_{F}\left(0,z+1,z\right)R_{D}\left(0,z+1,1\right)+R_{D}\left(0,z+1,z\right)R_{F}\left(0,z+1,1\right)=3\pi/(2z), \tag{19.21.1}
$$

The case $z=1$ shows that the product of the two lemniscate constants, ( 19.20.2 ) and ( 19.20.22 ), is $\pi/4$ .


<a id="E2"></a>
$$
3R_{F}\left(0,y,z\right)=zR_{D}\left(0,y,z\right)+yR_{D}\left(0,z,y\right). \tag{19.21.2}
$$


<a id="E3"></a>
$$
6R_{G}\left(0,y,z\right)=yz(R_{D}\left(0,y,z\right)+R_{D}\left(0,z,y\right))=3zR_{F}\left(0,y,z\right)+z(y-z)R_{D}\left(0,y,z\right). \tag{19.21.3}
$$

The complete cases of $R_{F}$ and $R_{G}$ have connection formulas resulting from those for the Gauss hypergeometric function (Erdélyi et al. ([1953a](./bib/E.html#bib751 "Higher Transcendental Functions. Vol. I"), §2.9)). Upper signs apply if $0<\operatorname{ph}z<\pi$ , and lower signs if $-\pi<\operatorname{ph}z<0$ :


<a id="E4"></a>
$$
R_{F}\left(0,z-1,z\right)=R_{F}\left(0,1-z,1\right)\mp\mathrm{i}R_{F}\left(0,z,1\right), \tag{19.21.4}
$$


<a id="E5"></a>
$$
2R_{G}\left(0,z-1,z\right)=2R_{G}\left(0,1-z,1\right)\pm\mathrm{i}2R_{G}\left(0,z,1\right)+(z-1)R_{F}\left(0,1-z,1\right)\mp\mathrm{i}zR_{F}\left(0,z,1\right). \tag{19.21.5}
$$

Let $y$ , $z$ , and $p$ be positive and distinct, and permute $y$ and $z$ to ensure that $y$ does not lie between $z$ and $p$ . The complete case of $R_{J}$ can be expressed in terms of $R_{F}$ and $R_{D}$ :


<a id="E6"></a>
$$
(\sqrt{rp}/z)R_{J}\left(0,y,z,p\right)={(r-1)}R_{F}\left(0,y,z\right)R_{D}\left(p,rz,z\right)+R_{D}\left(0,y,z\right)R_{F}\left(p,rz,z\right), \tag{19.21.6}
$$

If $0<p<z$ and $y=z+1$ , then as $p\to 0$ ( 19.21.6 ) reduces to Legendre’s relation ( 19.21.1 ).


## §19.21(ii) Incomplete Integrals

:::{note}
**Notes:**

See Carlson ([1977b](./bib/C.html#bib434 "Special Functions of Applied Mathematics"), (5.9-5), (5.9-6)) and ( 19.20.25 ). To obtain ( 19.21.7 ) eliminate $R_{D}\left(z,x,y\right)$ between ( 19.21.8 ) and ( 19.21.9 ), which follow from Carlson ([1977b](./bib/C.html#bib434 "Special Functions of Applied Mathematics"), (5.9-5, (6.6-5), and (5.9-6)). For ( 19.21.10 ) see Carlson ([1977b](./bib/C.html#bib434 "Special Functions of Applied Mathematics"), Table 9.3-1). To prove ( 19.21.11 ) write $xt/(t+x)=x-(x^{2}/(t+x))$ in ( 19.16.2_5 ) and similarly for $y$ and $z$ . Then use ( 19.21.9 ).

**See also:**

Annotations for §19.21 and Ch.19
:::

$R_{D}\left(x,y,z\right)$ is symmetric only in $x$ and $y$ , but either (nonzero) $x$ or (nonzero) $y$ can be moved to the third position by using


<a id="E7"></a>
$$
(x-y)R_{D}\left(y,z,x\right)+(z-y)R_{D}\left(x,y,z\right)=3R_{F}\left(x,y,z\right)-3y^{1/2}x^{-1/2}z^{-1/2}, \tag{19.21.7}
$$

or the corresponding equation with $x$ and $y$ interchanged.

<a id="EGx1"></a>

$$
\displaystyle R_{D}\left(y,z,x\right)+R_{D}\left(z,x,y\right)+R_{D}\left(x,y,z\right) \displaystyle=3x^{-1/2}y^{-1/2}z^{-1/2}, \tag{19.21.8}
$$

:::{note}
**Symbols:**

$R_{D}\left(\NVar{x},\NVar{y},\NVar{z}\right)$: elliptic integral symmetric in only two variables

**Referenced by:**

§19.21(ii) , §19.33(iii) , Erratum (V1.1.3) for Chapter 19

**Correction (effective with 1.1.3):**

The factors inside the square root on the right-hand side were written as products to ensure the correct multivalued behavior. *Suggested 2021-06-07 by Luc Maisonobe*

**See also:**

Annotations for §19.21(ii) , §19.21 and Ch.19
:::

$$
\displaystyle xR_{D}\left(y,z,x\right)+yR_{D}\left(z,x,y\right)+zR_{D}\left(x,y,z\right) \displaystyle=3R_{F}\left(x,y,z\right). \tag{19.21.9}
$$

:::{note}
**Symbols:**

$R_{D}\left(\NVar{x},\NVar{y},\NVar{z}\right)$: elliptic integral symmetric in only two variables and $R_{F}\left(\NVar{x},\NVar{y},\NVar{z}\right)$: symmetric elliptic integral of first kind

**Referenced by:**

§19.21(i) , §19.21(ii)

**See also:**

Annotations for §19.21(ii) , §19.21 and Ch.19
:::


<a id="E10"></a>
$$
2R_{G}\left(x,y,z\right)=zR_{F}\left(x,y,z\right)-\tfrac{1}{3}(x-z)(y-z)R_{D}\left(x,y,z\right)+x^{1/2}y^{1/2}z^{-1/2}, \tag{19.21.10}
$$

Because $R_{G}$ is completely symmetric, $x,y,z$ can be permuted on the right-hand side of ( 19.21.10 ) so that $(x-z)(y-z)\leq 0$ if the variables are real, thereby avoiding cancellations when $R_{G}$ is calculated from $R_{F}$ and $R_{D}$ (see § 19.36(i) ).


<a id="E11"></a>
$$
6R_{G}\left(x,y,z\right)=3(x+y+z)R_{F}\left(x,y,z\right)-\sum x^{2}R_{D}\left(y,z,x\right)=\sum x(y+z)R_{D}\left(y,z,x\right), \tag{19.21.11}
$$

where both summations extend over the three cyclic permutations of $x,y,z$ .

Connection formulas for $R_{-a}\left(\mathbf{b};\mathbf{z}\right)$ are given in Carlson ([1977b](./bib/C.html#bib434 "Special Functions of Applied Mathematics"), pp. 99, 101, and 123–124).


## §19.21(iii) Change of Parameter of RJ

:::{note}
**Keywords:**

[change of parameter of $R_{J}$](http://dlmf.nist.gov/search/search?q=change%20of%20parameter%20of%20RJ) , [circular cases](http://dlmf.nist.gov/search/search?q=circular%20cases) , [hyperbolic cases](http://dlmf.nist.gov/search/search?q=hyperbolic%20cases) , [symmetric elliptic integrals](http://dlmf.nist.gov/search/search?q=symmetric%20elliptic%20integrals)

**Notes:**

See Zill and Carlson ([1970](./bib/Z.html#bib2498 "Symmetric elliptic integrals of the third kind"), (4.6)).

**Referenced by:**

§19.7(iii)

**See also:**

Annotations for §19.21 and Ch.19
:::

Let $x,y,z$ be real and nonnegative, with at most one of them 0. Change-of-parameter relations can be used to shift the parameter $p$ of $R_{J}$ from either circular region to the other, or from either hyperbolic region to the other (§ 19.20(iii) ). The latter case allows evaluation of Cauchy principal values (see ( 19.20.14 )).


<a id="E12"></a>
$$
(p-x)R_{J}\left(x,y,z,p\right)+(q-x)R_{J}\left(x,y,z,q\right)=3R_{F}\left(x,y,z\right)-3R_{C}\left(\xi,\eta\right), \tag{19.21.12}
$$

where

<a id="E13"></a>

<a id="Ex1"></a>
$$
\displaystyle(p-x)(q-x) \displaystyle=(y-x)(z-x), \tag{19.21.13}
$$

<a id="Ex2"></a>
$$
\displaystyle\xi \displaystyle=yz/x,
$$

<a id="Ex3"></a>
$$
\displaystyle\eta \displaystyle=pq/x,
$$

:::{note}
**Symbols:**

$\xi$ and $\eta$

**See also:**

Annotations for §19.21(iii) , §19.21 and Ch.19
:::

and $x,y,z$ may be permuted. Also,


<a id="E14"></a>
$$
\eta-\xi=p+q-y-z=\frac{(p-y)(p-z)}{p-x}=\frac{(q-y)(q-z)}{q-x}=\frac{(p-y)(q-y)}{x-y}=\frac{(p-z)(q-z)}{x-z}. \tag{19.21.14}
$$

For each value of $p$ , permutation of $x,y,z$ produces three values of $q$ , one of which lies in the same region as $p$ and two lie in the other region of the same type. In ( 19.21.12 ), if $x$ is the largest (smallest) of $x,y$ , and $z$ , then $p$ and $q$ lie in the same region if it is circular (hyperbolic); otherwise $p$ and $q$ lie in different regions, both circular or both hyperbolic. If $x=0$ , then $\xi=\eta=\infty$ and $R_{C}\left(\xi,\eta\right)=0$ ; hence


<a id="E15"></a>
$$
pR_{J}\left(0,y,z,p\right)+qR_{J}\left(0,y,z,q\right)=3R_{F}\left(0,y,z\right), \tag{19.21.15}
$$
