# §3.3 Interpolation

:::{note}
**Keywords:**

[interpolation](http://dlmf.nist.gov/search/search?q=interpolation)

**See also:**

Annotations for Ch.3
:::


## §3.3(i) Lagrange Interpolation

:::{note}
**Keywords:**

[Barycentric form](http://dlmf.nist.gov/search/search?q=Barycentric%20form) , [Barycentric form of Lagrange interpolation](http://dlmf.nist.gov/search/search?q=Barycentric%20form%20of%20Lagrange%20interpolation) , [Lagrange interpolation](http://dlmf.nist.gov/search/search?q=Lagrange%20interpolation) , [abscissas](http://dlmf.nist.gov/search/search?q=abscissas) , [error term](http://dlmf.nist.gov/search/search?q=error%20term) , [formula](http://dlmf.nist.gov/search/search?q=formula) , [nodal](http://dlmf.nist.gov/search/search?q=nodal) , [nodal polynomials](http://dlmf.nist.gov/search/search?q=nodal%20polynomials) , [nodes](http://dlmf.nist.gov/search/search?q=nodes) , [polynomial](http://dlmf.nist.gov/search/search?q=polynomial) , [polynomials](http://dlmf.nist.gov/search/search?q=polynomials) , [remainder terms](http://dlmf.nist.gov/search/search?q=remainder%20terms)

**Notes:**

See Davis ([1975](./bib/D.html#bib617 "Interpolation and Approximation"), pp. 56 and 67–68).

**Referenced by:**

§18.40(ii) , §3.11(v) , §3.11(vi) , §3.3(ii) , §3.3(iii) , §3.3(iv) , §3.4(i) , Erratum (V1.1.3) for Subsection 3.3(i)

**Addition (effective with 1.1.3):**

Equations ( 3.3.3_1 ) and ( 3.3.3_2 ) were added.

**See also:**

Annotations for §3.3 and Ch.3
:::

The *nodes* or *abscissas* $z_{k}$ are real or complex; function values are $f_{k}=f(z_{k})$ . Given $n+1$ distinct points $z_{k}$ and $n+1$ corresponding function values $f_{k}$ , the *Lagrange interpolation polynomial* is the unique polynomial $P_{n}(z)$ of degree not exceeding $n$ such that $P_{n}(z_{k})=f_{k}$ , $k=0,1,\dots,n$ . It is given by


<a id="E1"></a>
$$
P_{n}(z)=\sum_{k=0}^{n}\ell_{k}(z)f_{k}=\omega_{n+1}(z)\sum_{k=0}^{n}\frac{\widetilde{\omega}_{k}}{z-z_{k}}f_{k}=\ifrac{\sum_{k=0}^{n}\frac{\widetilde{\omega}_{k}f_{k}}{z-z_{k}}}{\sum_{k=0}^{n}\frac{\widetilde{\omega}_{k}}{z-z_{k}}}, \tag{3.3.1}
$$

where

<a id="E2"></a>

<a id="Ex1"></a>
$$
\displaystyle\ell_{k}(z) \displaystyle={\sideset{}{{}^{\prime}}{\prod}_{j=0}^{n}}\frac{z-z_{j}}{z_{k}-z_{j}}, \tag{3.3.2}
$$

<a id="Ex2"></a>
$$
\displaystyle\ell_{k}(z_{j}) \displaystyle=\delta_{k,j}.
$$

:::{note}
**Defines:**

$\ell_{k}(z)$ : Lagrange interpolation polynomial (locally)

**Symbols:**

$\delta_{\NVar{j},\NVar{k}}$: Kronecker delta and $z_{\NVar{k}}$: nodes of function

**See also:**

Annotations for §3.3(i) , §3.3 and Ch.3
:::

Here the prime signifies that the factor for $j=k$ is to be omitted, $\delta_{k,j}$ is the Kronecker symbol, and $\omega_{n+1}(z)$ is the *nodal polynomial*


<a id="E3"></a>
$$
\omega_{n+1}(z)=\prod_{k=0}^{n}(z-z_{k}), \tag{3.3.3}
$$

and the weights $\widetilde{\omega}_{k}$ are


<a id="E3_1"></a>
$$
\widetilde{\omega}_{k}=\frac{1}{\omega_{n+1}^{\prime}(z_{k})}={\sideset{}{{}^{\prime}}{\prod}_{j=0}^{n}}\frac{1}{z_{k}-z_{j}}. \tag{3.3.3_1}
$$

The final expression in ( 3.3.1 ) is the *Barycentric form* of the Lagrange interpolation formula. It is a direct consequence of the identity


<a id="E3_2"></a>
$$
1=\sum_{k=0}^{n}\ell_{k}(z)=\omega_{n+1}(z)\sum_{k=0}^{n}\frac{\widetilde{\omega}_{k}}{z-z_{k}}, \tag{3.3.3_2}
$$

and according to Berrut and Trefethen ([2004](./bib/B.html#bib2944 "Barycentric Lagrange interpolation")) it is the most efficient representation of $P_{n}(z)$ .

With an error term the *Lagrange interpolation formula* for $f$ is given by


<a id="E4"></a>
$$
f(z)=\sum_{k=0}^{n}\ell_{k}(z)f_{k}+R_{n}(z). \tag{3.3.4}
$$

If $f$ , $x$ ( $=z$ ), and the nodes $x_{k}$ are real, and $f^{(n+1)}$ is continuous on the smallest closed interval $I$ containing $x,x_{0},x_{1},\dots,x_{n}$ , then the error can be expressed


<a id="E5"></a>
$$
R_{n}(x)=\frac{f^{(n+1)}(\xi)}{(n+1)!}\,\omega_{n+1}(x), \tag{3.3.5}
$$

for some $\xi\in I$ . If $f$ is analytic in a simply-connected domain $D$ (§ 1.13(i) ), then for $z\in D$ ,


<a id="E6"></a>
$$
R_{n}(z)=\frac{\omega_{n+1}(z)}{2\pi\mathrm{i}}\int_{C}\frac{f(\zeta)}{(\zeta-z)\omega_{n+1}(\zeta)}\,\mathrm{d}\zeta, \tag{3.3.6}
$$

where $C$ is a simple closed contour in $D$ described in the positive rotational sense and enclosing the points $z,z_{1},z_{2},\dots,z_{n}$ .


## §3.3(ii) Lagrange Interpolation with Equally-Spaced Nodes

:::{note}
**Keywords:**

[Lagrange interpolation](http://dlmf.nist.gov/search/search?q=Lagrange%20interpolation) , [coefficients](http://dlmf.nist.gov/search/search?q=coefficients) , [equally-spaced nodes](http://dlmf.nist.gov/search/search?q=equally-spaced%20nodes)

**Notes:**

See National Bureau of Standards ([1944](./bib/N.html#bib1698 "Tables of Lagrangian Interpolation Coefficients"), pp. xv–xvii).

**Referenced by:**

§3.4(i)

**See also:**

Annotations for §3.3 and Ch.3
:::

The $(n+1)$ -point formula ( 3.3.4 ) can be written in the form


<a id="E7"></a>
$$
f_{t}=f(x_{0}+th)=\sum_{k=n_{0}}^{n_{1}}A_{k}^{n}f_{k}+R_{n,t}, \tag{3.3.7}
$$

where the nodes $x_{k}=x_{0}+kh$ ( $h>0$ ) and function $f$ are real,

<a id="E8"></a>

<a id="Ex3"></a>
$$
\displaystyle n_{0} \displaystyle=-\tfrac{1}{2}(n-\sigma), \tag{3.3.8}
$$

<a id="Ex4"></a>
$$
\displaystyle n_{1} \displaystyle=\tfrac{1}{2}(n+\sigma),
$$

:::{note}
**A&S Ref:**

25.2.6 (modification of)

**See also:**

Annotations for §3.3(ii) , §3.3 and Ch.3
:::


<a id="E9"></a>
$$
\sigma=\tfrac{1}{2}(1-(-1)^{n}), \tag{3.3.9}
$$

and $A_{k}^{n}$ are the *Lagrangian interpolation coefficients* defined by


<a id="E10"></a>
$$
A_{k}^{n}=\frac{(-1)^{n_{1}+k}}{(k-n_{0})!\,(n_{1}-k)!(t-k)}\,\prod_{m=n_{0}}^{n_{1}}(t-m). \tag{3.3.10}
$$

The remainder is given by


<a id="E11"></a>
$$
R_{n,t}=R_{n}(x_{0}+th)=\frac{h^{n+1}}{(n+1)!}f^{(n+1)}(\xi)\prod_{k=n_{0}}^{n_{1}}(t-k), \tag{3.3.11}
$$

where $\xi$ is as in § 3.3(i) .

Let $c_{n}$ be defined by


<a id="E12"></a>
$$
c_{n}=\frac{1}{(n+1)!}\max\prod_{k=n_{0}}^{n_{1}}\left|t-k\right|, \tag{3.3.12}
$$

where the maximum is taken over $t$ -intervals given in the formulas below. Then for these $t$ -intervals,


<a id="E13"></a>
$$
\left|R_{n,t}\right|\leq c_{n}h^{n+1}\left|f^{(n+1)}(\xi)\right|. \tag{3.3.13}
$$


### Linear Interpolation

:::{note}
**Keywords:**

[interpolation](http://dlmf.nist.gov/search/search?q=interpolation) , [linear](http://dlmf.nist.gov/search/search?q=linear)

**See also:**

Annotations for §3.3(ii) , §3.3 and Ch.3
:::

<a id="EGx1"></a>

$$
\displaystyle f_{t} \displaystyle=(1-t)f_{0}+tf_{1}+R_{1,t}, \tag{3.3.14}
$$

:::{note}
**Symbols:**

$R_{n,t}(x)$: remainder and $f_{\NVar{t}}$: function values

**A&S Ref:**

25.2.9

**See also:**

Annotations for §3.3(ii) , §3.3(ii) , §3.3 and Ch.3
:::

$$
\displaystyle c_{1} \displaystyle=\tfrac{1}{8}, \tag{3.3.15}
$$

:::{note}
**Symbols:**

$c_{n}$: bound coefficient

**A&S Ref:**

25.2.10 (modification of)

**See also:**

Annotations for §3.3(ii) , §3.3(ii) , §3.3 and Ch.3
:::


### Three-Point Formula

:::{note}
**See also:**

Annotations for §3.3(ii) , §3.3 and Ch.3
:::


<a id="E16"></a>
$$
f_{t}=\sum_{k=-1}^{1}A_{k}^{2}f_{k}+R_{2,t}, \tag{3.3.16}
$$

<a id="E17"></a>

<a id="Ex5"></a>
$$
\displaystyle A_{-1}^{2} \displaystyle=\tfrac{1}{2}t(t-1), \tag{3.3.17}
$$

<a id="Ex6"></a>
$$
\displaystyle A_{0}^{2} \displaystyle=1-t^{2},
$$

<a id="Ex7"></a>
$$
\displaystyle A_{1}^{2} \displaystyle=\tfrac{1}{2}t(t+1),
$$

:::{note}
**Symbols:**

$A_{k}^{n}$: Lagrangian interpolation coefficients

**See also:**

Annotations for §3.3(ii) , §3.3(ii) , §3.3 and Ch.3
:::


<a id="E18"></a>
$$
c_{2}=1/(9\sqrt{3})=0.0641\ldots, \tag{3.3.18}
$$


### Four-Point Formula

:::{note}
**See also:**

Annotations for §3.3(ii) , §3.3 and Ch.3
:::


<a id="E19"></a>
$$
f_{t}=\sum_{k=-1}^{2}A_{k}^{3}f_{k}+R_{3,t}, \tag{3.3.19}
$$

<a id="E20"></a>

<a id="Ex8"></a>
$$
\displaystyle A_{-1}^{3} \displaystyle=-\tfrac{1}{6}t(t-1)(t-2), \tag{3.3.20}
$$

<a id="Ex9"></a>
$$
\displaystyle A_{0}^{3} \displaystyle=\tfrac{1}{2}(t^{2}-1)(t-2),
$$

<a id="Ex10"></a>
$$
\displaystyle A_{1}^{3} \displaystyle=-\tfrac{1}{2}t(t+1)(t-2),
$$

<a id="Ex11"></a>
$$
\displaystyle A_{2}^{3} \displaystyle=\tfrac{1}{6}t(t^{2}-1),
$$

:::{note}
**Symbols:**

$A_{k}^{n}$: Lagrangian interpolation coefficients

**See also:**

Annotations for §3.3(ii) , §3.3(ii) , §3.3 and Ch.3
:::


<a id="E21"></a>
$$
c_{3}=\begin{cases}\tfrac{3}{128}=0.0234\ldots,&0<t<1,\\
\tfrac{1}{24}=0.0416\ldots,&-1<t<0\mbox{ or }1<t<2.\\
\end{cases} \tag{3.3.21}
$$


### Five-Point Formula

:::{note}
**See also:**

Annotations for §3.3(ii) , §3.3 and Ch.3
:::


<a id="E22"></a>
$$
f_{t}=\sum_{k=-2}^{2}A_{k}^{4}f_{k}+R_{4,t}, \tag{3.3.22}
$$

<a id="E23"></a>

<a id="Ex12"></a>
$$
\displaystyle A_{-2}^{4} \displaystyle=\tfrac{1}{24}t(t^{2}-1)(t-2), \tag{3.3.23}
$$

<a id="Ex13"></a>
$$
\displaystyle A_{-1}^{4} \displaystyle=-\tfrac{1}{6}t(t-1)(t^{2}-4),
$$

<a id="Ex14"></a>
$$
\displaystyle A_{0}^{4} \displaystyle=\tfrac{1}{4}(t^{2}-1)(t^{2}-4),
$$

<a id="Ex15"></a>
$$
\displaystyle A_{1}^{4} \displaystyle=-\tfrac{1}{6}t(t+1)(t^{2}-4),
$$

<a id="Ex16"></a>
$$
\displaystyle A_{2}^{4} \displaystyle=\tfrac{1}{24}t(t^{2}-1)(t+2),
$$

:::{note}
**Symbols:**

$A_{k}^{n}$: Lagrangian interpolation coefficients

**A&S Ref:**

25.2.15 (modification of)

**See also:**

Annotations for §3.3(ii) , §3.3(ii) , §3.3 and Ch.3
:::


<a id="E24"></a>
$$
c_{4}=\begin{cases}0.0118\ldots,&\left|t\right|<1,\\
0.0302\ldots,&1<\left|t\right|<2.\\
\end{cases} \tag{3.3.24}
$$


### Six-Point Formula

:::{note}
**See also:**

Annotations for §3.3(ii) , §3.3 and Ch.3
:::


<a id="E25"></a>
$$
f_{t}=\sum_{k=-2}^{3}A_{k}^{5}f_{k}+R_{5,t}, \tag{3.3.25}
$$

<a id="E26"></a>

<a id="Ex17"></a>
$$
\displaystyle A_{-2}^{5} \displaystyle=-\tfrac{1}{120}t(t^{2}-1)(t-2)(t-3), \tag{3.3.26}
$$

<a id="Ex18"></a>
$$
\displaystyle A_{-1}^{5} \displaystyle=\tfrac{1}{24}t(t-1)(t^{2}-4)(t-3),
$$

<a id="Ex19"></a>
$$
\displaystyle A_{0}^{5} \displaystyle=-\tfrac{1}{12}(t^{2}-1)(t^{2}-4)(t-3),
$$

<a id="Ex20"></a>
$$
\displaystyle A_{1}^{5} \displaystyle=\tfrac{1}{12}t(t+1)(t^{2}-4)(t-3),
$$

<a id="Ex21"></a>
$$
\displaystyle A_{2}^{5} \displaystyle=-\tfrac{1}{24}t(t^{2}-1)(t+2)(t-3),
$$

<a id="Ex22"></a>
$$
\displaystyle A_{3}^{5} \displaystyle=\tfrac{1}{120}t(t^{2}-1)(t^{2}-4),
$$

:::{note}
**Symbols:**

$A_{k}^{n}$: Lagrangian interpolation coefficients

**A&S Ref:**

25.2.17 (modification of)

**See also:**

Annotations for §3.3(ii) , §3.3(ii) , §3.3 and Ch.3
:::


<a id="E27"></a>
$$
c_{5}=\begin{cases}0.00488\ldots,&0<t<1,\\
0.00701\ldots,&-1<t<0\mbox{ or }1<t<2,\\
0.0234\ldots,&-2<t<-1\mbox{ or }2<t<3.\end{cases} \tag{3.3.27}
$$


### Seven-Point Formula

:::{note}
**See also:**

Annotations for §3.3(ii) , §3.3 and Ch.3
:::


<a id="E28"></a>
$$
f_{t}=\sum_{k=-3}^{3}A_{k}^{6}f_{k}+R_{6,t}, \tag{3.3.28}
$$

<a id="E29"></a>

<a id="Ex23"></a>
$$
\displaystyle A_{-3}^{6} \displaystyle=\tfrac{1}{720}t(t^{2}-1)(t-3)(t^{2}-4), \tag{3.3.29}
$$

<a id="Ex24"></a>
$$
\displaystyle A_{-2}^{6} \displaystyle=-\tfrac{1}{120}t(t^{2}-1)(t-2)(t^{2}-9),
$$

<a id="Ex25"></a>
$$
\displaystyle A_{-1}^{6} \displaystyle=\tfrac{1}{48}t(t-1)(t^{2}-4)(t^{2}-9),
$$

<a id="Ex26"></a>
$$
\displaystyle A_{0}^{6} \displaystyle=-\tfrac{1}{36}(t^{2}-1)(t^{2}-4)(t^{2}-9),
$$

<a id="Ex27"></a>
$$
\displaystyle A_{1}^{6} \displaystyle=\tfrac{1}{48}t(t+1)(t^{2}-4)(t^{2}-9),
$$

<a id="Ex28"></a>
$$
\displaystyle A_{2}^{6} \displaystyle=-\tfrac{1}{120}t(t^{2}-1)(t+2)(t^{2}-9),
$$

<a id="Ex29"></a>
$$
\displaystyle A_{3}^{6} \displaystyle=\tfrac{1}{720}t(t^{2}-1)(t+3)(t^{2}-4),
$$

:::{note}
**Symbols:**

$A_{k}^{n}$: Lagrangian interpolation coefficients

**A&S Ref:**

25.2.19 (modification of)

**See also:**

Annotations for §3.3(ii) , §3.3(ii) , §3.3 and Ch.3
:::


<a id="E30"></a>
$$
c_{6}=\begin{cases}0.00245\ldots,&\left|t\right|<1,\\
0.00459\ldots,&1<\left|t\right|<2,\\
0.0190\ldots,&2<\left|t\right|<3.\\
\end{cases} \tag{3.3.30}
$$


### Eight-Point Formula

:::{note}
**Keywords:**

[Lagrange interpolation](http://dlmf.nist.gov/search/search?q=Lagrange%20interpolation) , [equally-spaced nodes](http://dlmf.nist.gov/search/search?q=equally-spaced%20nodes) , [remainder terms](http://dlmf.nist.gov/search/search?q=remainder%20terms)

**See also:**

Annotations for §3.3(ii) , §3.3 and Ch.3
:::


<a id="E31"></a>
$$
f_{t}=\sum_{k=-3}^{4}A_{k}^{7}f_{k}+R_{7,t}, \tag{3.3.31}
$$

<a id="E32"></a>

<a id="Ex30"></a>
$$
\displaystyle A_{-3}^{7} \displaystyle=-\tfrac{1}{5040}t(t^{2}-1)(t-3)(t-4)(t^{2}-4), \tag{3.3.32}
$$

<a id="Ex31"></a>
$$
\displaystyle A_{-2}^{7} \displaystyle=\tfrac{1}{720}t(t^{2}-1)(t-2)(t-4)(t^{2}-9),
$$

<a id="Ex32"></a>
$$
\displaystyle A_{-1}^{7} \displaystyle=-\tfrac{1}{240}t(t-1)(t-4)(t^{2}-4)(t^{2}-9),
$$

<a id="Ex33"></a>
$$
\displaystyle A_{0}^{7} \displaystyle=\tfrac{1}{144}(t^{2}-1)(t-4)(t^{2}-4)(t^{2}-9),
$$

<a id="Ex34"></a>
$$
\displaystyle A_{1}^{7} \displaystyle=-\tfrac{1}{144}t(t+1)(t-4)(t^{2}-4)(t^{2}-9),
$$

<a id="Ex35"></a>
$$
\displaystyle A_{2}^{7} \displaystyle=\tfrac{1}{240}t(t^{2}-1)(t+2)(t-4)(t^{2}-9),
$$

<a id="Ex36"></a>
$$
\displaystyle A_{3}^{7} \displaystyle=-\tfrac{1}{720}t(t^{2}-1)(t+3)(t-4)(t^{2}-4),
$$

<a id="Ex37"></a>
$$
\displaystyle A_{4}^{7} \displaystyle=\tfrac{1}{5040}t(t^{2}-1)(t^{2}-4)(t^{2}-9),
$$

:::{note}
**Symbols:**

$A_{k}^{n}$: Lagrangian interpolation coefficients

**See also:**

Annotations for §3.3(ii) , §3.3(ii) , §3.3 and Ch.3
:::


<a id="E33"></a>
$$
c_{7}=\begin{cases}0.00106\ldots,&0<t<1,\\
0.00139\ldots,&-1<t<0\mbox{ or }1<t<2,\\
0.00321\ldots,&-2<t<-1\mbox{ or }2<t<3,\\
0.0158\ldots,&-3<t<-2\mbox{ or }3<t<4.\\
\end{cases} \tag{3.3.33}
$$


## §3.3(iii) Divided Differences

:::{note}
**Keywords:**

[Lagrange interpolation](http://dlmf.nist.gov/search/search?q=Lagrange%20interpolation) , [definition](http://dlmf.nist.gov/search/search?q=definition) , [divided differences](http://dlmf.nist.gov/search/search?q=divided%20differences) , [integral representation](http://dlmf.nist.gov/search/search?q=integral%20representation) , [via divided differences](http://dlmf.nist.gov/search/search?q=via%20divided%20differences)

**Notes:**

See Davis ([1975](./bib/D.html#bib617 "Interpolation and Approximation"), p. 65) and Hildebrand ([1974](./bib/H.html#bib1077 "Introduction to Numerical Analysis"), Chapter 2).

**See also:**

Annotations for §3.3 and Ch.3
:::

The *divided differences* of $f$ relative to a sequence of distinct points $z_{0},z_{1},z_{2},\dots$ are defined by

<a id="E34"></a>

<a id="Ex38"></a>
$$
\displaystyle\left[z_{0}\right]f \displaystyle=f_{0}, \tag{3.3.34}
$$

<a id="Ex39"></a>
$$
\displaystyle\left[z_{0},z_{1}\right]f \displaystyle=(\left[z_{1}\right]f-\left[z_{0}\right]f)/(z_{1}-z_{0}),
$$

<a id="Ex40"></a>
$$
\displaystyle\left[z_{0},z_{1},z_{2}\right]f \displaystyle=(\left[z_{1},z_{2}\right]f-\left[z_{0},z_{1}\right]f)/(z_{2}-z_{0}),
$$

:::{note}
**Defines:**

$\left[\NVar{z_{0},z_{1},\dots,z_{n}}\right]\NVar{f}$ : divided difference

**Symbols:**

$f(z)$: function , $f_{\NVar{t}}$: function values and $z_{\NVar{k}}$: nodes of function

**A&S Ref:**

25.1.4

**Referenced by:**

Erratum (V1.1.2) for Equation (3.3.34)

**Errata (effective with 1.1.2):**

The leading divided difference operators were previously omitted from these formulas, due to programming error. *Reported 2021-06-01 by Nico Temme*

**See also:**

Annotations for §3.3(iii) , §3.3 and Ch.3
:::

and so on. Explicitly, the *divided difference of order $n$* is given by


<a id="E35"></a>
$$
\left[z_{0},z_{1},\dots,z_{n}\right]f=\sum_{k=0}^{n}\left(\ifrac{f(z_{k})}{\prod_{\begin{subarray}{c}0\leq j\leq n\\
j\neq k\end{subarray}}(z_{k}-z_{j})}\right). \tag{3.3.35}
$$

If $f$ and the $z_{k}$ ( $=x_{k}$ ) are real, and $f$ is $n$ times continuously differentiable on a closed interval containing the $x_{k}$ , then


<a id="E36"></a>
$$
\left[x_{0},x_{1},\dots,x_{n}\right]f=\frac{f^{(n)}(\xi)}{n!} \tag{3.3.36}
$$

and again $\xi$ is as in § 3.3(i) . If $f$ is analytic in a simply-connected domain $D$ , then for $z\in{D}$ ,


<a id="E37"></a>
$$
\left[z_{0},z_{1},\dots,z_{n}\right]f=\frac{1}{2\pi\mathrm{i}}\int_{C}\frac{f(\zeta)}{\omega_{n+1}(\zeta)}\,\mathrm{d}\zeta, \tag{3.3.37}
$$

where $\omega_{n+1}(\zeta)$ is given by ( 3.3.3 ), and $C$ is a simple closed contour in ${D}$ described in the positive rotational sense and enclosing $z_{0},z_{1},\dots,z_{n}$ .


## §3.3(iv) Newton’s Interpolation Formula

:::{note}
**Keywords:**

[Lagrange interpolation](http://dlmf.nist.gov/search/search?q=Lagrange%20interpolation) , [Newton’s interpolation formula](http://dlmf.nist.gov/search/search?q=Newton%20interpolation%20formula)

**Notes:**

See Davis ([1975](./bib/D.html#bib617 "Interpolation and Approximation"), pp. 39–49) and Hildebrand ([1974](./bib/H.html#bib1077 "Introduction to Numerical Analysis"), pp. 60–66).

**See also:**

Annotations for §3.3 and Ch.3
:::

This represents the Lagrange interpolation polynomial in terms of divided differences:


<a id="E38"></a>
$$
f(z)=\left[z_{0}\right]f+(z-z_{0})\left[z_{0},z_{1}\right]f+(z-z_{0})(z-z_{1})\left[z_{0},z_{1},z_{2}\right]f+\cdots+(z-z_{0})(z-z_{1})\cdots(z-z_{n-1})\left[z_{0},z_{1},\dots,z_{n}\right]f+R_{n}(z). \tag{3.3.38}
$$

The interpolation error $R_{n}(z)$ is as in § 3.3(i) . Newton’s formula has the advantage of allowing easy updating: incorporation of a new point $z_{n+1}$ requires only addition of the term with $\left[z_{0},z_{1},\dots,z_{n+1}\right]f$ to ( 3.3.38 ), plus the computation of this divided difference. Another advantage is its robustness with respect to confluence of the set of points $z_{0},z_{1},\dots,z_{n}$ . For example, for $k+1$ coincident points the limiting form is given by $\left[z_{0},z_{0},\dots,z_{0}\right]f=f^{(k)}(z_{0})/k!$ .


## §3.3(v) Inverse Interpolation

:::{note}
**Keywords:**

[interpolation](http://dlmf.nist.gov/search/search?q=interpolation) , [inverse](http://dlmf.nist.gov/search/search?q=inverse)

**Notes:**

See Ostrowski ([1973](./bib/O.html#bib1820 "Solution of Equations in Euclidean and Banach Spaces"), pp. 18–26) and Hildebrand ([1974](./bib/H.html#bib1077 "Introduction to Numerical Analysis"), pp. 68–70).

**Referenced by:**

§3.8(iii)

**See also:**

Annotations for §3.3 and Ch.3
:::

In this method we interchange the roles of the points $z_{k}$ and the function values $f_{k}$ . It can be used for solving a nonlinear scalar equation $f(z)=0$ approximately. Another approach is to combine the methods of § [3.8](./3.8.md "§3.8 Nonlinear Equations ‣ Areas ‣ Chapter 3 Numerical Methods") with direct interpolation and § [3.4](./3.4.md "§3.4 Differentiation ‣ Areas ‣ Chapter 3 Numerical Methods") .


### Example

:::{note}
**Keywords:**

[Airy functions](http://dlmf.nist.gov/search/search?q=Airy%20functions) , [computation](http://dlmf.nist.gov/search/search?q=computation) , [zeros](http://dlmf.nist.gov/search/search?q=zeros)

**See also:**

Annotations for §3.3(v) , §3.3 and Ch.3
:::

To compute the first negative zero $a_{1}=-2.33810\;7410\ldots$ of the Airy function $f(x)=\operatorname{Ai}\left(x\right)$ (§ [9.2](./9.2.md "§9.2 Differential Equation ‣ Airy Functions ‣ Chapter 9 Airy and Related Functions") ). The inverse interpolation polynomial is given by


<a id="E39"></a>
$$
x(f)=\left[f_{0}\right]x+(f-f_{0})\left[f_{0},f_{1}\right]x+(f-f_{0})(f-f_{1})\left[f_{0},f_{1},f_{2}\right]x; \tag{3.3.39}
$$

compare ( 3.3.38 ). With $x_{0}=-2.2$ , $x_{1}=-2.3$ , $x_{2}=-2.4$ , we obtain


<a id="E40"></a>
$$
x=-2.2+1.44011\;1973(f-0.09614\;53780)+0.08865\;85832\*(f-0.09614\;53780)(f-0.02670\;63331), \tag{3.3.40}
$$

and with $f=0$ we find that $x=-2.33823\;2462$ , with 4 correct digits. By using this approximation to $x$ as a new point, $x_{3}=x$ , and evaluating $\left[f_{0},f_{1},f_{2},f_{3}\right]x=1.12388\;6190$ , we find that $x=-2.33810\;7409$ , with 9 correct digits.

For comparison, we use Newton’s interpolation formula ( 3.3.38 )


<a id="E41"></a>
$$
f(x)=0.09614\;53780+0.69439\;04495(x+2.1)-0.03007\;14275(x+2.2)(x+2.3), \tag{3.3.41}
$$

with the derivative


<a id="E42"></a>
$$
f^{\prime}(x)=0.55906\;90257-0.06014\;28550x, \tag{3.3.42}
$$

and compute an approximation to $a_{1}$ by using Newton’s rule (§ 3.8(ii) ) with starting value $x=-2.5$ . This gives the new point $x_{3}=-2.33934\;0514$ . Then by using $x_{3}$ in Newton’s interpolation formula, evaluating $\left[x_{0},x_{1},x_{2},x_{3}\right]f=-0.26608\;28233$ and recomputing $f^{\prime}(x)$ , another application of Newton’s rule with starting value $x_{3}$ gives the approximation $x=2.33810\;7373$ , with 8 correct digits.


## §3.3(vi) Other Interpolation Methods

:::{note}
**Keywords:**

[Hermite](http://dlmf.nist.gov/search/search?q=Hermite) , [Sinc function](http://dlmf.nist.gov/search/search?q=Sinc%20function) , [based on Chebyshev points](http://dlmf.nist.gov/search/search?q=based%20on%20Chebyshev%20points) , [based on Sinc functions](http://dlmf.nist.gov/search/search?q=based%20on%20Sinc%20functions) , [bivariate](http://dlmf.nist.gov/search/search?q=bivariate) , [cardinal function](http://dlmf.nist.gov/search/search?q=cardinal%20function) , [convergence properties](http://dlmf.nist.gov/search/search?q=convergence%20properties) , [interpolation](http://dlmf.nist.gov/search/search?q=interpolation) , [numerical differentiation](http://dlmf.nist.gov/search/search?q=numerical%20differentiation) , [rational](http://dlmf.nist.gov/search/search?q=rational) , [spline](http://dlmf.nist.gov/search/search?q=spline) , [trigonometric](http://dlmf.nist.gov/search/search?q=trigonometric)

**Referenced by:**

§3.4(i) , §3.5(i)

**See also:**

Annotations for §3.3 and Ch.3
:::

For Hermite interpolation, trigonometric interpolation, spline interpolation, rational interpolation (by using continued fractions), interpolation based on Chebyshev points, and bivariate interpolation, see Bulirsch and Rutishauser ([1968](./bib/B.html#bib377 "Interpolation und genäherte Quadratur")), Davis ([1975](./bib/D.html#bib617 "Interpolation and Approximation"), pp. 27–31), and Mason and Handscomb ([2003](./bib/M.html#bib1560 "Chebyshev Polynomials"), Chapter 6). These references also describe convergence properties of the interpolation formulas.

For interpolation of a bounded function $f$ on $\mathbb{R}$ the *cardinal function* of $f$ is defined by


<a id="E43"></a>
$$
C(f,h)(x)=\sum_{k=-\infty}^{\infty}f(kh)S(k,h)(x), \tag{3.3.43}
$$

where


<a id="E44"></a>
$$
S(k,h)(x)=\frac{\sin\left(\pi(x-kh)/h\right)}{\pi(x-kh)/h}, \tag{3.3.44}
$$

is called the *Sinc function* . For theory and applications see Stenger ([1993](./bib/S.html#bib2171 "Numerical Methods Based on Sinc and Analytic Functions"), Chapter 3).
