# §4.7 Derivatives and Differential Equations

:::{note}
**See also:**

Annotations for Ch.4
:::


## §4.7(i) Logarithms

:::{note}
**Keywords:**

[derivatives](http://dlmf.nist.gov/search/search?q=derivatives) , [differential equations](http://dlmf.nist.gov/search/search?q=differential%20equations) , [logarithm function](http://dlmf.nist.gov/search/search?q=logarithm%20function)

**Notes:**

See Levinson and Redheffer ([1970](./bib/L.html#bib1426 "Complex Variables"), pp. 62–69).

**See also:**

Annotations for §4.7 and Ch.4
:::


<a id="E1"></a>
$$
\frac{\mathrm{d}}{\mathrm{d}z}\ln z=\frac{1}{z}, \tag{4.7.1}
$$


<a id="E2"></a>
$$
\frac{\mathrm{d}}{\mathrm{d}z}\operatorname{Ln}z=\frac{1}{z}, \tag{4.7.2}
$$


<a id="E3"></a>
$$
\frac{{\mathrm{d}}^{n}}{{\mathrm{d}z}^{n}}\ln z=(-1)^{n-1}(n-1)!z^{-n}, \tag{4.7.3}
$$


<a id="E4"></a>
$$
\frac{{\mathrm{d}}^{n}}{{\mathrm{d}z}^{n}}\operatorname{Ln}z=(-1)^{n-1}(n-1)!z^{-n}. \tag{4.7.4}
$$

For a nonvanishing analytic function $f(z)$ , the general solution of the differential equation


<a id="E5"></a>
$$
\frac{\mathrm{d}w}{\mathrm{d}z}=\frac{f^{\prime}(z)}{f(z)} \tag{4.7.5}
$$

is


<a id="E6"></a>
$$
w(z)=\operatorname{Ln}\left(f(z)\right)+\hbox{ constant}. \tag{4.7.6}
$$


## §4.7(ii) Exponentials and Powers

:::{note}
**Keywords:**

[derivatives](http://dlmf.nist.gov/search/search?q=derivatives) , [differential equation](http://dlmf.nist.gov/search/search?q=differential%20equation) , [exponential function](http://dlmf.nist.gov/search/search?q=exponential%20function) , [power function](http://dlmf.nist.gov/search/search?q=power%20function)

**Notes:**

See Levinson and Redheffer ([1970](./bib/L.html#bib1426 "Complex Variables"), pp. 53–54 and p. 69).

**See also:**

Annotations for §4.7 and Ch.4
:::


<a id="E7"></a>
$$
\frac{\mathrm{d}}{\mathrm{d}z}e^{z}=e^{z}, \tag{4.7.7}
$$


<a id="E8"></a>
$$
\frac{\mathrm{d}}{\mathrm{d}z}e^{az}=ae^{az}, \tag{4.7.8}
$$


<a id="E9"></a>
$$
\frac{\mathrm{d}}{\mathrm{d}z}a^{z}=a^{z}\ln a, \tag{4.7.9}
$$

When $a^{z}$ is a general power, $\ln a$ is replaced by the branch of $\operatorname{Ln}a$ used in constructing $a^{z}$ .


<a id="E10"></a>
$$
\frac{\mathrm{d}}{\mathrm{d}z}z^{a}=az^{a-1}, \tag{4.7.10}
$$


<a id="E11"></a>
$$
\frac{{\mathrm{d}}^{n}}{{\mathrm{d}z}^{n}}z^{a}=a(a-1)(a-2)\cdots(a-n+1)z^{a-n}. \tag{4.7.11}
$$

The general solution of the differential equation


<a id="E12"></a>
$$
\frac{\mathrm{d}w}{\mathrm{d}z}=f(z)w \tag{4.7.12}
$$

is


<a id="E13"></a>
$$
w=\exp\left(\int f(z)\,\mathrm{d}z\right)+{\rm constant}. \tag{4.7.13}
$$

The general solution of the differential equation


<a id="E14"></a>
$$
\frac{{\mathrm{d}}^{2}w}{{\mathrm{d}z}^{2}}=aw, \tag{4.7.14}
$$

is


<a id="E15"></a>
$$
w=Ae^{\sqrt{a}z}+Be^{-\sqrt{a}z}, \tag{4.7.15}
$$

where $A$ and $B$ are arbitrary constants.

For other differential equations see Kamke ([1977](./bib/K.html#bib1217 "Differentialgleichungen: Lösungsmethoden und Lösungen. Teil I"), pp. 396–413).
