# §8.4 Special Values

:::{note}
**Keywords:**

[incomplete gamma functions](http://dlmf.nist.gov/search/search?q=incomplete%20gamma%20functions) , [special values](http://dlmf.nist.gov/search/search?q=special%20values)

**Notes:**

See Erdélyi et al. ([1953b](./bib/E.html#bib752 "Higher Transcendental Functions. Vol. II"), Chapter 9). ( 8.4.14 ) follows from ( 8.4.6 ) and ( 8.8.6 ). ( 8.4.15 ) follows from the first series in ( 8.7.3 ) by combining $\Gamma\left(a\right)$ with the term $k=n$ of the series, then taking the limit as $a\rightarrow-n$ .

**See also:**

Annotations for Ch.8
:::

For $\operatorname{erf}\left(z\right)$ , $\operatorname{erfc}\left(z\right)$ , and $F\left(z\right)$ , see §§ 7.2(i) , 7.2(ii) . For $E_{n}\left(z\right)$ see § 8.19(i) .


<a id="E1"></a>
$$
\gamma\left(\tfrac{1}{2},z^{2}\right)=2\int_{0}^{z}e^{-t^{2}}\,\mathrm{d}t=\sqrt{\pi}\operatorname{erf}\left(z\right), \tag{8.4.1}
$$

<a id="EGx1"></a>

$$
\displaystyle\gamma^{*}\left(a,0\right) \displaystyle=\frac{1}{\Gamma\left(a+1\right)}, \tag{8.4.2}
$$

:::{note}
**Symbols:**

$\Gamma\left(\NVar{z}\right)$: gamma function , $\gamma^{*}\left(\NVar{a},\NVar{z}\right)$: incomplete gamma function and $a$: parameter

**See also:**

Annotations for §8.4 and Ch.8
:::

$$
\displaystyle\gamma^{*}\left(\tfrac{1}{2},-z^{2}\right) \displaystyle=\frac{2e^{z^{2}}}{z\sqrt{\pi}}F\left(z\right). \tag{8.4.3}
$$

:::{note}
**Symbols:**

$F\left(\NVar{z}\right)$: Dawson’s integral , $\pi$: the ratio of the circumference of a circle to its diameter , $\mathrm{e}$: base of natural logarithm , $\gamma^{*}\left(\NVar{a},\NVar{z}\right)$: incomplete gamma function and $z$: complex variable

**A&S Ref:**

6.5.18

**See also:**

Annotations for §8.4 and Ch.8
:::


<a id="E4"></a>
$$
\Gamma\left(0,z\right)=\int_{z}^{\infty}t^{-1}e^{-t}\,\mathrm{d}t=E_{1}\left(z\right), \tag{8.4.4}
$$


<a id="E5"></a>
$$
\Gamma\left(1,z\right)=e^{-z}, \tag{8.4.5}
$$


<a id="E6"></a>
$$
\Gamma\left(\tfrac{1}{2},z^{2}\right)=2\int_{z}^{\infty}e^{-t^{2}}\,\mathrm{d}t=\sqrt{\pi}\operatorname{erfc}\left(z\right). \tag{8.4.6}
$$

For $n=0,1,2,\dots$ ,

<a id="EGx2"></a>

$$
\displaystyle\gamma\left(n+1,z\right) \displaystyle=n!(1-e^{-z}e_{n}(z)), \tag{8.4.7}
$$

:::{note}
**Symbols:**

$\mathrm{e}$: base of natural logarithm , $!$: factorial (as in $n!$) , $\gamma\left(\NVar{a},\NVar{z}\right)$: incomplete gamma function , $z$: complex variable , $n$: nonnegative integer and $e_{n}(z)$: functions

**Referenced by:**

§8.11(v)

**See also:**

Annotations for §8.4 and Ch.8
:::

$$
\displaystyle\Gamma\left(n+1,z\right) \displaystyle=n!e^{-z}e_{n}(z), \tag{8.4.8}
$$

:::{note}
**Symbols:**

$\mathrm{e}$: base of natural logarithm , $!$: factorial (as in $n!$) , $\Gamma\left(\NVar{a},\NVar{z}\right)$: incomplete gamma function , $z$: complex variable , $n$: nonnegative integer and $e_{n}(z)$: functions

**See also:**

Annotations for §8.4 and Ch.8
:::

$$
\displaystyle P\left(n+1,z\right) \displaystyle=1-e^{-z}e_{n}(z), \tag{8.4.9}
$$

:::{note}
**Symbols:**

$\mathrm{e}$: base of natural logarithm , $P\left(\NVar{a},\NVar{z}\right)$: normalized incomplete gamma function , $z$: complex variable , $n$: nonnegative integer and $e_{n}(z)$: functions

**A&S Ref:**

6.5.13

**See also:**

Annotations for §8.4 and Ch.8
:::

$$
\displaystyle Q\left(n+1,z\right) \displaystyle=e^{-z}e_{n}(z), \tag{8.4.10}
$$

:::{note}
**Symbols:**

$\mathrm{e}$: base of natural logarithm , $Q\left(\NVar{a},\NVar{z}\right)$: normalized incomplete gamma function , $z$: complex variable , $n$: nonnegative integer and $e_{n}(z)$: functions

**See also:**

Annotations for §8.4 and Ch.8
:::

where


<a id="E11"></a>
$$
e_{n}(z)=\sum_{k=0}^{n}\frac{z^{k}}{k!}. \tag{8.4.11}
$$

Also


<a id="E12"></a>
$$
\gamma^{*}\left(-n,z\right)=z^{n}, \tag{8.4.12}
$$


<a id="E13"></a>
$$
\Gamma\left(1-n,z\right)=z^{1-n}E_{n}\left(z\right), \tag{8.4.13}
$$


<a id="E14"></a>
$$
Q\left(n+\tfrac{1}{2},z^{2}\right)=\operatorname{erfc}\left(z\right)+\frac{e^{-z^{2}}}{\sqrt{\pi}}\sum_{k=1}^{n}\frac{z^{2k-1}}{{\left(\tfrac{1}{2}\right)_{k}}}, \tag{8.4.14}
$$


<a id="E15"></a>
$$
\Gamma\left(-n,z\right)=\frac{(-1)^{n}}{n!}\left(E_{1}\left(z\right)-e^{-z}\sum_{k=0}^{n-1}\frac{(-1)^{k}k!}{z^{k+1}}\right)=\frac{(-1)^{n}}{n!}\left(\psi\left(n+1\right)-\ln z\right)-z^{-n}\sum_{\begin{subarray}{c}k=0\\
k\neq n\end{subarray}}^{\infty}\frac{(-z)^{k}}{k!(k-n)}. \tag{8.4.15}
$$
