# ยง8.8 Recurrence Relations and Derivatives

:::{note}
**Keywords:**

[derivatives](http://dlmf.nist.gov/search/search?q=derivatives) , [incomplete gamma functions](http://dlmf.nist.gov/search/search?q=incomplete%20gamma%20functions) , [recurrence relations](http://dlmf.nist.gov/search/search?q=recurrence%20relations)

**Notes:**

These results follow straightforwardly from the definitions in ยง 8.2(i) .

**See also:**

Annotations for Ch.8
:::


<a id="E1"></a>
$$
\gamma\left(a+1,z\right)=a\gamma\left(a,z\right)-z^{a}e^{-z}, \tag{8.8.1}
$$


<a id="E2"></a>
$$
\Gamma\left(a+1,z\right)=a\Gamma\left(a,z\right)+z^{a}e^{-z}. \tag{8.8.2}
$$

If $w(a,z)=\gamma\left(a,z\right)$ or $\Gamma\left(a,z\right)$ , then


<a id="E3"></a>
$$
w(a+2,z)-(a+1+z)w(a+1,z)+azw(a,z)=0. \tag{8.8.3}
$$


<a id="E4"></a>
$$
z\gamma^{*}\left(a+1,z\right)=\gamma^{*}\left(a,z\right)-\frac{e^{-z}}{\Gamma\left(a+1\right)}. \tag{8.8.4}
$$


<a id="E5"></a>
$$
P\left(a+1,z\right)=P\left(a,z\right)-\frac{z^{a}e^{-z}}{\Gamma\left(a+1\right)}, \tag{8.8.5}
$$


<a id="E6"></a>
$$
Q\left(a+1,z\right)=Q\left(a,z\right)+\frac{z^{a}e^{-z}}{\Gamma\left(a+1\right)}. \tag{8.8.6}
$$

For $n=0,1,2,\dots$ ,


<a id="E7"></a>
$$
\gamma\left(a+n,z\right)={\left(a\right)_{n}}\gamma\left(a,z\right)-z^{a}e^{-z}\sum_{k=0}^{n-1}\frac{\Gamma\left(a+n\right)}{\Gamma\left(a+k+1\right)}z^{k}, \tag{8.8.7}
$$


<a id="E8"></a>
$$
\gamma\left(a,z\right)=\frac{\Gamma\left(a\right)}{\Gamma\left(a-n\right)}\gamma\left(a-n,z\right)-z^{a-1}e^{-z}\sum_{k=0}^{n-1}\frac{\Gamma\left(a\right)}{\Gamma\left(a-k\right)}z^{-k}, \tag{8.8.8}
$$


<a id="E9"></a>
$$
\Gamma\left(a+n,z\right)={\left(a\right)_{n}}\Gamma\left(a,z\right)+z^{a}e^{-z}\sum_{k=0}^{n-1}\frac{\Gamma\left(a+n\right)}{\Gamma\left(a+k+1\right)}z^{k}, \tag{8.8.9}
$$


<a id="E10"></a>
$$
\Gamma\left(a,z\right)=\frac{\Gamma\left(a\right)}{\Gamma\left(a-n\right)}\Gamma\left(a-n,z\right)+z^{a-1}e^{-z}\sum_{k=0}^{n-1}\frac{\Gamma\left(a\right)}{\Gamma\left(a-k\right)}z^{-k}, \tag{8.8.10}
$$


<a id="E11"></a>
$$
P\left(a+n,z\right)=P\left(a,z\right)-z^{a}e^{-z}\sum_{k=0}^{n-1}\frac{z^{k}}{\Gamma\left(a+k+1\right)}, \tag{8.8.11}
$$


<a id="E12"></a>
$$
Q\left(a+n,z\right)=Q\left(a,z\right)+z^{a}e^{-z}\sum_{k=0}^{n-1}\frac{z^{k}}{\Gamma\left(a+k+1\right)}. \tag{8.8.12}
$$


<a id="E13"></a>
$$
\frac{\mathrm{d}}{\mathrm{d}z}\gamma\left(a,z\right)=-\frac{\mathrm{d}}{\mathrm{d}z}\Gamma\left(a,z\right)=z^{a-1}e^{-z}, \tag{8.8.13}
$$


<a id="E14"></a>
$$
\left.\frac{\partial}{\partial a}\gamma^{*}\left(a,z\right)\right|_{a=0}=-E_{1}\left(z\right)-\ln z. \tag{8.8.14}
$$

For $E_{1}\left(z\right)$ see ยง 8.19(i) .

For $n=0,1,2,\dots$ ,


<a id="E15"></a>
$$
\frac{{\mathrm{d}}^{n}}{{\mathrm{d}z}^{n}}(z^{-a}\gamma\left(a,z\right))=(-1)^{n}z^{-a-n}\gamma\left(a+n,z\right), \tag{8.8.15}
$$


<a id="E16"></a>
$$
\frac{{\mathrm{d}}^{n}}{{\mathrm{d}z}^{n}}(z^{-a}\Gamma\left(a,z\right))=(-1)^{n}z^{-a-n}\Gamma\left(a+n,z\right), \tag{8.8.16}
$$


<a id="E17"></a>
$$
\frac{{\mathrm{d}}^{n}}{{\mathrm{d}z}^{n}}(e^{z}\gamma\left(a,z\right))=(-1)^{n}{\left(1-a\right)_{n}}e^{z}\gamma\left(a-n,z\right), \tag{8.8.17}
$$


<a id="E18"></a>
$$
\frac{{\mathrm{d}}^{n}}{{\mathrm{d}z}^{n}}(z^{a}e^{z}\gamma^{*}\left(a,z\right))=z^{a-n}e^{z}\gamma^{*}\left(a-n,z\right), \tag{8.8.18}
$$


<a id="E19"></a>
$$
\frac{{\mathrm{d}}^{n}}{{\mathrm{d}z}^{n}}(e^{z}\Gamma\left(a,z\right))=(-1)^{n}{\left(1-a\right)_{n}}e^{z}\Gamma\left(a-n,z\right). \tag{8.8.19}
$$
