# §17.7 Special Cases of Higher ϕsr Functions

:::{note}
**Keywords:**

[$q$-hypergeometric function](http://dlmf.nist.gov/search/search?q=q-hypergeometric%20function) , [special cases](http://dlmf.nist.gov/search/search?q=special%20cases)

**See also:**

Annotations for Ch.17
:::


## §17.7(i) ϕ22 Functions

:::{note}
**Notes:**

See Gasper and Rahman ([2004](./bib/G.html#bib862 "Basic Hypergeometric Series"), pp. 28–29). For ( 17.7.3 ) combine Gasper and Rahman ([2004](./bib/G.html#bib862 "Basic Hypergeometric Series"), p. 359, Equation (III.4)) with ( 17.6.4 ).

**See also:**

Annotations for §17.7 and Ch.17
:::


### q-Analog of Bailey’s F12⁡(−1) Sum

:::{note}
**Keywords:**

[Bailey’s ${{}_{2}F_{1}}(-1)$ sum](http://dlmf.nist.gov/search/search?q=Bailey%202F1%28-1%29%20sum) , [$q$-analog](http://dlmf.nist.gov/search/search?q=q-analog) , [$q$-hypergeometric function](http://dlmf.nist.gov/search/search?q=q-hypergeometric%20function)

**See also:**

Annotations for §17.7(i) , §17.7 and Ch.17
:::


<a id="E1"></a>
$$
{{}_{2}\phi_{2}}\left({a,q/a\atop-q,b};q,-b\right)=\frac{\left(ab,bq/a;q^{2}\right)_{\infty}}{\left(b;q\right)_{\infty}}. \tag{17.7.1}
$$


### q-Analog of Gauss’s F12⁡(−1) Sum

:::{note}
**Keywords:**

[Gauss’s ${{}_{2}F_{1}}(-1)$ sum](http://dlmf.nist.gov/search/search?q=Gauss%202F1%28-1%29%20sum) , [$q$-analog](http://dlmf.nist.gov/search/search?q=q-analog) , [$q$-hypergeometric function](http://dlmf.nist.gov/search/search?q=q-hypergeometric%20function)

**See also:**

Annotations for §17.7(i) , §17.7 and Ch.17
:::


<a id="E2"></a>
$$
{{}_{2}\phi_{2}}\left({a^{2},b^{2}\atop abq^{\frac{1}{2}},-abq^{\frac{1}{2}}};q,-q\right)=\frac{\left(a^{2}q,b^{2}q;q^{2}\right)_{\infty}}{\left(q,a^{2}b^{2}q;q^{2}\right)_{\infty}}. \tag{17.7.2}
$$


### Sum Related to (17.6.4)

:::{note}
**Keywords:**

[Andrews–Askey sum](http://dlmf.nist.gov/search/search?q=Andrews%E2%80%93Askey%20sum) , [$q$-hypergeometric function](http://dlmf.nist.gov/search/search?q=q-hypergeometric%20function)

**See also:**

Annotations for §17.7(i) , §17.7 and Ch.17
:::


<a id="E3"></a>
$$
{{}_{2}\phi_{2}}\left({\ifrac{c^{2}}{b^{2}},b^{2}\atop c,cq};q^{2},q\right)=\frac{1}{2}\frac{\left(b^{2},q;q^{2}\right)_{\infty}}{\left(c,cq;q^{2}\right)_{\infty}}{\left(\frac{\left(c/b;q\right)_{\infty}}{\left(b;q\right)_{\infty}}+\frac{\left(-c/b;q\right)_{\infty}}{\left(-b;q\right)_{\infty}}\right)}. \tag{17.7.3}
$$


## §17.7(ii) ϕ23 Functions

:::{note}
**Notes:**

See Gasper and Rahman ([2004](./bib/G.html#bib862 "Basic Hypergeometric Series"), pp. 17, 58, 356).

**See also:**

Annotations for §17.7 and Ch.17
:::


### q-Pfaff–Saalschütz Sum

:::{note}
**Keywords:**

[$q$-Pfaff–Saalschütz sum](http://dlmf.nist.gov/search/search?q=q-Pfaff--Saalschutz%20sum) , [$q$-hypergeometric function](http://dlmf.nist.gov/search/search?q=q-hypergeometric%20function)

**See also:**

Annotations for §17.7(ii) , §17.7 and Ch.17
:::


<a id="E4"></a>
$$
{{}_{3}\phi_{2}}\left({a,b,q^{-n}\atop c,abq^{1-n}/c};q,q\right)=\frac{\left(c/a,c/b;q\right)_{n}}{\left(c,c/(ab);q\right)_{n}}. \tag{17.7.4}
$$


### Nonterminating Form of the q-Saalschütz Sum

:::{note}
**Keywords:**

[nonterminating form](http://dlmf.nist.gov/search/search?q=nonterminating%20form) , [$q$-Saalschütz sum](http://dlmf.nist.gov/search/search?q=q-Saalschutz%20sum) , [$q$-hypergeometric function](http://dlmf.nist.gov/search/search?q=q-hypergeometric%20function)

**See also:**

Annotations for §17.7(ii) , §17.7 and Ch.17
:::


<a id="E5"></a>
$$
{{}_{3}\phi_{2}}\left({a,b,c\atop e,f};q,q\right)+\frac{\left(q/e,a,b,c,qf/e;q\right)_{\infty}}{\left(e/q,aq/e,bq/e,cq/e,f;q\right)_{\infty}}\*{{}_{3}\phi_{2}}\left({aq/e,bq/e,cq/e\atop q^{2}/e,qf/e};q,q\right)=\frac{\left(q/e,f/a,f/b,f/c;q\right)_{\infty}}{\left(aq/e,bq/e,cq/e,f;q\right)_{\infty}}, \tag{17.7.5}
$$

where $ef=abcq$ .


### F. H. Jackson’s Terminating q-Analog of Dixon’s Sum

:::{note}
**Keywords:**

[Dixon’s sum](http://dlmf.nist.gov/search/search?q=Dixon%20sum) , [F. H. Jackson’s $q$-analog](http://dlmf.nist.gov/search/search?q=F.%20H.%20Jackson%20q-analog) , [$q$-hypergeometric function](http://dlmf.nist.gov/search/search?q=q-hypergeometric%20function)

**See also:**

Annotations for §17.7(ii) , §17.7 and Ch.17
:::


<a id="E6"></a>
$$
{{}_{3}\phi_{2}}\left({q^{-2n},b,c\atop q^{1-2n}/b,q^{1-2n}/c};q,\frac{q^{2-n}}{bc}\right)=\frac{\left(b,c;q\right)_{n}\left(q,bc;q\right)_{2n}}{\left(q,bc;q\right)_{n}\left(b,c;q\right)_{2n}}. \tag{17.7.6}
$$


### Continued Fractions

:::{note}
**Keywords:**

[continued fractions](http://dlmf.nist.gov/search/search?q=continued%20fractions) , [$q$-hypergeometric function](http://dlmf.nist.gov/search/search?q=q-hypergeometric%20function)

**See also:**

Annotations for §17.7(ii) , §17.7 and Ch.17
:::

For continued-fraction representations of a ratio of ${{}_{3}\phi_{2}}$ functions, see Cuyt et al. ([2008](./bib/C.html#bib608 "Handbook of Continued Fractions for Special Functions"), pp. 399–400).


## §17.7(iii) Other ϕsr Functions

:::{note}
**Notes:**

See Gasper and Rahman ([2004](./bib/G.html#bib862 "Basic Hypergeometric Series"), pp. 19, 43–44, 61–62, 81–83, 355–356) and Andrews ([1996](./bib/index.html#bib96 "Pfaff’s method II: Diverse applications")). See also Gao and Guo ([2013](./bib/G.html#bib2839 "Contiguous relations and summation and transformation formulae for basic hypergeometric series")).

**Referenced by:**

Erratum (V1.0.10) for References , Erratum (V1.1.11) for Subsection 17.7(iii)

**Addition (effective with 1.0.10):**

A citation to Gao and Guo ([2013](./bib/G.html#bib2839 "Contiguous relations and summation and transformation formulae for basic hypergeometric series")) was added to the metadata.

**See also:**

Annotations for §17.7 and Ch.17
:::


### q-Analog of Dixon’s F23⁡(1) Sum

:::{note}
**Keywords:**

[Dixon’s ${{}_{3}F_{2}}(1)$ sum](http://dlmf.nist.gov/search/search?q=Dixon%203F2%281%29%20sum) , [$q$-analog](http://dlmf.nist.gov/search/search?q=q-analog) , [$q$-hypergeometric function](http://dlmf.nist.gov/search/search?q=q-hypergeometric%20function)

**See also:**

Annotations for §17.7(iii) , §17.7 and Ch.17
:::


<a id="E7"></a>
$$
{{}_{4}\phi_{3}}\left({a,-qa^{\frac{1}{2}},b,c\atop-a^{\frac{1}{2}},aq/b,aq/c};q,\frac{qa^{\frac{1}{2}}}{bc}\right)=\frac{\left(aq,qa^{\frac{1}{2}}/b,qa^{\frac{1}{2}}/c,aq/(bc);q\right)_{\infty}}{\left(aq/b,aq/c,qa^{\frac{1}{2}},qa^{\frac{1}{2}}/(bc);q\right)_{\infty}}. \tag{17.7.7}
$$


### Gasper–Rahman q-Analog of Watson’s F23 Sum

:::{note}
**Keywords:**

[Gasper–Rahman $q$-analog](http://dlmf.nist.gov/search/search?q=Gasper%E2%80%93Rahman%20q-analog) , [Watson’s ${{}_{3}F_{2}}$ sum](http://dlmf.nist.gov/search/search?q=Watson%203F2%20sum)

**See also:**

Annotations for §17.7(iii) , §17.7 and Ch.17
:::


<a id="E8"></a>
$$
{{}_{8}\phi_{7}}\left({\lambda,q\lambda^{\frac{1}{2}},-q\lambda^{\frac{1}{2}},a,b,c,-c,\lambda q/c^{2}\atop\lambda^{\frac{1}{2}},-\lambda^{\frac{1}{2}},\lambda q/a,\lambda q/b,\lambda q/c,-\lambda q/c,c^{2}};q,-\frac{\lambda q}{ab}\right)=\frac{\left(\lambda q,c^{2}/\lambda;q\right)_{\infty}\left(aq,bq,c^{2}q/a,c^{2}q/b;q^{2}\right)_{\infty}}{\left(\lambda q/a,\lambda q/b;q\right)_{\infty}\left(q,abq,c^{2}q,c^{2}q/(ab);q^{2}\right)_{\infty}}, \tag{17.7.8}
$$

where $\lambda=-c(ab/q)^{\frac{1}{2}}$ .


### Andrews’ q-Analog of the Terminating Version of Watson’s F23 Sum (16.4.6)

:::{note}
**Keywords:**

[Andrews’ terminating $q$-analog](http://dlmf.nist.gov/search/search?q=Andrews%E2%80%99%20terminating%20q-analog) , [Watson’s ${{}_{3}F_{2}}$ sum](http://dlmf.nist.gov/search/search?q=Watson%203F2%20sum)

**Modification (effective with 1.1.11):**

The title of this paragraph was previously “Andrews’ Terminating $q$ -Analog of ( 17.7.8 )”.

**See also:**

Annotations for §17.7(iii) , §17.7 and Ch.17
:::


<a id="E9"></a>
$$
{{}_{4}\phi_{3}}\left({q^{-n},aq^{n},c,-c\atop(aq)^{\frac{1}{2}},-(aq)^{\frac{1}{2}},c^{2}};q,q\right)=\begin{cases}0,&\mbox{$n$ odd,}\\
\dfrac{c^{n}\left(q,aq/c^{2};q^{2}\right)_{n/2}}{\left(aq,c^{2}q;q^{2}\right)_{n/2}},&\mbox{$n$ even.}\end{cases} \tag{17.7.9}
$$


### Gasper–Rahman q-Analog of Whipple’s F23 Sum

:::{note}
**Keywords:**

[Gasper–Rahman $q$-analog](http://dlmf.nist.gov/search/search?q=Gasper%E2%80%93Rahman%20q-analog) , [Whipple’s ${{}_{3}F_{2}}$ sum](http://dlmf.nist.gov/search/search?q=Whipple%203F2%20sum)

**See also:**

Annotations for §17.7(iii) , §17.7 and Ch.17
:::


<a id="E10"></a>
$$
{{}_{8}\phi_{7}}\left({-c,q(-c)^{\frac{1}{2}},-q(-c)^{\frac{1}{2}},a,q/a,c,-d,-q/d\atop(-c)^{\frac{1}{2}},-(-c)^{\frac{1}{2}},-cq/a,-ac,-q,cq/d,cd};q,c\right)=\frac{\left(-c,-cq;q\right)_{\infty}\left(acd,acq/d,cdq/a,cq^{2}/(ad);q^{2}\right)_{\infty}}{\left(cd,cq/d,-ac,-cq/a;q\right)_{\infty}}. \tag{17.7.10}
$$


### Andrews’ q-Analog of the Terminating Version of Whipple’s F23 Sum (16.4.7)

:::{note}
**Modification (effective with 1.1.11):**

The title of this paragraph was previously “Andrews’ Terminating $q$ -Analog”.

**See also:**

Annotations for §17.7(iii) , §17.7 and Ch.17
:::


<a id="E11"></a>
$$
{{}_{4}\phi_{3}}\left({q^{-n},q^{n+1},c,-c\atop e,c^{2}q/e,-q};q,q\right)=q^{\genfrac{(}{)}{0.0pt}{}{n+1}{2}}\frac{\left(eq^{-n},eq^{n+1},c^{2}q^{1-n}/e,c^{2}q^{n+2}/e;q^{2}\right)_{\infty}}{\left(e,c^{2}q/e;q\right)_{\infty}}. \tag{17.7.11}
$$


### First q-Analog of Bailey’s F34⁡(1) Sum

:::{note}
**Keywords:**

[Bailey’s ${{}_{4}F_{3}}(1)$ sum](http://dlmf.nist.gov/search/search?q=Bailey%204F3%281%29%20sum) , [$q$-analogs (first and second)](http://dlmf.nist.gov/search/search?q=q-analogs) , [$q$-analogs (first and second)](http://dlmf.nist.gov/search/search?q=q-analogs%20%28first%20and%20second%29) , [$q$-hypergeometric function](http://dlmf.nist.gov/search/search?q=q-hypergeometric%20function)

**See also:**

Annotations for §17.7(iii) , §17.7 and Ch.17
:::


<a id="E12"></a>
$$
{{}_{4}\phi_{3}}\left({a,aq,b^{2}q^{2n},q^{-2n}\atop b,bq,a^{2}q^{2}};q^{2},q^{2}\right)=\frac{a^{n}\left(-q,b/a;q\right)_{n}}{\left(-aq,b;q\right)_{n}}. \tag{17.7.12}
$$


### Second q-Analog of Bailey’s F34⁡(1) Sum

:::{note}
**See also:**

Annotations for §17.7(iii) , §17.7 and Ch.17
:::


<a id="E13"></a>
$$
{{}_{4}\phi_{3}}\left({a,aq,b^{2}q^{2n-2},q^{-2n}\atop b,bq,a^{2}};q^{2},q^{2}\right)=\frac{a^{n}\left(-q,b/a;q\right)_{n}(1-bq^{n-1})}{\left(-a,b;q\right)_{n}(1-bq^{2n-1})}. \tag{17.7.13}
$$


### F. H. Jackson’s q-Analog of Dougall’s F67⁡(1)Sum

:::{note}
**Keywords:**

[Dougall’s ${{}_{7}F_{6}}(1)$ sum](http://dlmf.nist.gov/search/search?q=Dougall%207F6%281%29%20sum) , [F. H. Jackson’s $q$-analog](http://dlmf.nist.gov/search/search?q=F.%20H.%20Jackson%20q-analog) , [$q$-hypergeometric function](http://dlmf.nist.gov/search/search?q=q-hypergeometric%20function)

**See also:**

Annotations for §17.7(iii) , §17.7 and Ch.17
:::


<a id="E14"></a>
$$
{{}_{8}\phi_{7}}\left({a,qa^{\frac{1}{2}},-qa^{\frac{1}{2}},b,c,d,e,q^{-n}\atop a^{\frac{1}{2}},-a^{\frac{1}{2}},aq/b,aq/c,aq/d,aq/e,aq^{n+1}};q,q\right)=\frac{\left(aq,aq/(bc),aq/(bd),aq/(cd);q\right)_{n}}{\left(aq/b,aq/c,aq/d,aq/(bcd);q\right)_{n}}, \tag{17.7.14}
$$

where $a^{2}q=bcdeq^{-n}$ .


### Limiting Cases of (17.7.14)

:::{note}
**See also:**

Annotations for §17.7(iii) , §17.7 and Ch.17
:::


<a id="E15"></a>
$$
{{}_{6}\phi_{5}}\left({a,qa^{\frac{1}{2}},-qa^{\frac{1}{2}},b,c,d\atop a^{\frac{1}{2}},-a^{\frac{1}{2}},aq/b,aq/c,aq/d};q,\frac{aq}{bcd}\right)=\frac{\left(aq,aq/(bc),aq/(bd),aq/(cd);q\right)_{\infty}}{\left(aq/b,aq/c,aq/d,aq/(bcd);q\right)_{\infty}}, \tag{17.7.15}
$$

and when $d=q^{-n}$ ,


<a id="E16"></a>
$$
{{}_{6}\phi_{5}}\left({a,qa^{\frac{1}{2}},-qa^{\frac{1}{2}},b,c,q^{-n}\atop a^{\frac{1}{2}},-a^{\frac{1}{2}},aq/b,aq/c,aq^{n+1}};q,\frac{aq^{n+1}}{bc}\right)=\frac{\left(aq,aq/(bc);q\right)_{n}}{\left(aq/b,aq/c;q\right)_{n}}. \tag{17.7.16}
$$


### Bailey’s Nonterminating Extension of Jackson’s ϕ78Sum

:::{note}
**See also:**

Annotations for §17.7(iii) , §17.7 and Ch.17
:::


<a id="E17"></a>
$$
{{}_{8}\phi_{7}}\left({a,qa^{\frac{1}{2}},-qa^{\frac{1}{2}},b,c,d,e,f\atop a^{\frac{1}{2}},-a^{\frac{1}{2}},aq/b,aq/c,aq/d,aq/e,aq/f};q,q\right)-\frac{b}{a}\frac{\left(aq,c,d,e,f,bq/a,bq/c,bq/d,bq/e,bq/f;q\right)_{\infty}}{\left(aq/b,aq/c,aq/d,aq/e,aq/f,bc/a,bd/a,be/a,bf/a,b^{2}q/a;q\right)_{\infty}}\*{{}_{8}\phi_{7}}\left({b^{2}/a,qba^{-\frac{1}{2}},-qba^{-\frac{1}{2}},b,bc/a,bd/a,be/a,bf/a\atop ba^{-\frac{1}{2}},-ba^{-\frac{1}{2}},bq/a,bq/c,bq/d,bq/e,bq/f};q,q\right)=\frac{\left(aq,b/a,aq/(cd),aq/(ce),aq/(cf),aq/(de),aq/(df),aq/(ef);q\right)_{\infty}}{\left(aq/c,aq/d,aq/e,aq/f,bc/a,bd/a,be/a,bf/a;q\right)_{\infty}}, \tag{17.7.17}
$$

where $qa^{2}=bcdef$ .


### Gasper–Rahman q-Analogs of the Karlsson–Minton Sums

:::{note}
**See also:**

Annotations for §17.7(iii) , §17.7 and Ch.17
:::


<a id="E18"></a>
$$
{{}_{r+2}\phi_{r+1}}\left({a,b,b_{1}q^{m_{1}},\dots,b_{r}q^{m_{r}}\atop bq,b_{1},\dots,b_{r}};q,a^{-1}q^{1-(m_{1}+\cdots+m_{r})}\right)=\frac{\left(q,bq/a;q\right)_{\infty}\left(b_{1}/b;q\right)_{m_{1}}\cdots\left(b_{r}/b;q\right)_{m_{r}}}{\left(bq,q/a;q\right)_{\infty}\left(b_{1};q\right)_{m_{1}}\cdots\left(b_{r};q\right)_{m_{r}}}b^{m_{1}+\cdots+m_{r}}, \tag{17.7.18}
$$

and


<a id="E19"></a>
$$
{{}_{r+1}\phi_{r}}\left({a,b_{1}q^{m_{1}},\dots,b_{r}q^{m_{r}}\atop b_{1},\dots,b_{r}};q,a^{-1}q^{1-(m_{1}+\cdots+m_{r})}\right)=0, \tag{17.7.19}
$$

where $m_{1},m_{2},\dots,m_{r}$ are arbitrary nonnegative integers.


### Gosper’s Bibasic Sum

:::{note}
**Keywords:**

[bibasic sums and series](http://dlmf.nist.gov/search/search?q=bibasic%20sums%20and%20series) , [$q$-hypergeometric function](http://dlmf.nist.gov/search/search?q=q-hypergeometric%20function)

**See also:**

Annotations for §17.7(iii) , §17.7 and Ch.17
:::


<a id="E20"></a>
$$
\sum_{k=0}^{n}\frac{1-ap^{k}q^{k}}{1-a}\frac{\left(a;p\right)_{k}\left(c;q\right)_{k}}{\left(q;q\right)_{k}\left(ap/c;p\right)_{k}}c^{-k}=\frac{\left(ap;p\right)_{n}\left(cq;q\right)_{n}}{\left(q;q\right)_{n}\left(ap/c;p\right)_{n}}c^{-n}. \tag{17.7.20}
$$


### Gasper’s Extensions of Gosper’s Bibasic Sum

:::{note}
**See also:**

Annotations for §17.7(iii) , §17.7 and Ch.17
:::


<a id="E21"></a>
$$
\sum_{k=0}^{n}\frac{(1-ap^{k}q^{k})(1-bp^{k}q^{-k})}{(1-a)(1-b)}\frac{\left(a,b;p\right)_{k}\left(c,a/(bc);q\right)_{k}}{\left(q,aq/b;q\right)_{k}\left(ap/c,bcp;p\right)_{k}}q^{k}=\frac{\left(ap,bp;p\right)_{n}\left(cq,aq/(bc);q\right)_{n}}{\left(q,aq/b;q\right)_{n}\left(ap/c,bcp;p\right)_{n}}, \tag{17.7.21}
$$


<a id="E22"></a>
$$
\sum_{k=-m}^{n}\frac{(1-adp^{k}q^{k})(1-bp^{k}/(dq^{k}))}{(1-ad)(1-(b/d))}\frac{\left(a,b;p\right)_{k}\left(c,ad^{2}/(bc);q\right)_{k}}{\left(dq,adq/b;q\right)_{k}\left(adp/c,bcp/d;p\right)_{k}}q^{k}=\frac{(1-a)(1-b)(1-c)(1-(ad^{2}/(bc)))}{d(1-ad)(1-(b/d))(1-(c/d))(1-(ad/(bc)))}\left(\frac{\left(ap,bp;p\right)_{n}\left(cq,ad^{2}q/(bc);q\right)_{n}}{\left(dq,adq/b;q\right)_{n}\left(adp/c,bcp/d;p\right)_{n}}-\frac{\left(c/(ad),d/(bc);p\right)_{m+1}\left(1/d,b/(ad);q\right)_{m+1}}{\left(1/c,bc/(ad^{2});q\right)_{m+1}\left(1/a,1/b;p\right)_{m+1}}\right), \tag{17.7.22}
$$

and $n$ -th difference generalization:


<a id="E23"></a>
$$
\left(1-\frac{a}{q}\right)\left(1-\frac{b}{q}\right)\sum_{k=0}^{n}\frac{\left(ap^{k},bp^{-k};q\right)_{n-1}(1-(ap^{2k}/b))}{\left(p;p\right)_{n}\left(p;p\right)_{n-k}\left(ap^{k}/b;q\right)_{n+1}}(-1)^{k}p^{\genfrac{(}{)}{0.0pt}{}{k}{2}}=\delta_{n,0}. \tag{17.7.23}
$$
