# Â§29.15 Fourier Series and Chebyshev Series

:::{note}
**Keywords:**

[Fourier series](http://dlmf.nist.gov/search/search?q=Fourier%20series) , [LamÃ© polynomials](http://dlmf.nist.gov/search/search?q=Lam%C3%A9%20polynomials)

**See also:**

Annotations for Ch.29
:::


## Â§29.15(i) Fourier Coefficients

:::{note}
**Notes:**

The method for constructing the coefficients follows from Â§ [29.6](./29.6.md "Â§29.6 Fourier Series â€£ LamÃ© Functions â€£ Chapter 29 LamÃ© Functions") .

**Referenced by:**

Â§29.20(i) , Â§29.20(ii) , Â§29.6(i)

**See also:**

Annotations for Â§29.15 and Ch.29
:::


### Polynomial ğ‘¢ğ¸2â¢nmâ¡(z,k2)

:::{note}
**See also:**

Annotations for Â§29.15(i) , Â§29.15 and Ch.29
:::

When $\nu=2n$ , $m=0,1,\dots,n$ , the Fourier series ( 29.6.1 ) terminates:


<a id="E1"></a>
$$
\mathit{uE}^{m}_{2n}\left(z,k^{2}\right)=\tfrac{1}{2}A_{0}+\sum_{p=1}^{n}A_{2p}\cos\left(2p\phi\right). \tag{29.15.1}
$$

A convenient way of constructing the coefficients, together with the eigenvalues, is as follows. Equations ( 29.6.4 ), with $p=1,2,\dots,n$ , ( 29.6.3 ), and $A_{2n+2}=0$ can be cast as an algebraic eigenvalue problem in the following way. Let


<a id="E2"></a>
$$
\mathbf{M}=\begin{bmatrix}\beta_{0}&\alpha_{0}&0&\cdots&0\\
\gamma_{1}&\beta_{1}&\alpha_{1}&\ddots&\vdots\\
0&\ddots&\ddots&\ddots&0\\
\vdots&\ddots&\gamma_{n-1}&\beta_{n-1}&\alpha_{n-1}\\
0&\cdots&0&\gamma_{n}&\beta_{n}\end{bmatrix} \tag{29.15.2}
$$

be the tridiagonal matrix with $\alpha_{p}$ , $\beta_{p}$ , $\gamma_{p}$ as in ( 29.3.11 ), ( 29.3.12 ). Let the eigenvalues of $\mathbf{M}$ be $H_{p}$ with


<a id="E3"></a>
$$
H_{0}<H_{1}<\cdots<H_{n}, \tag{29.15.3}
$$

and also let


<a id="E4"></a>
$$
[A_{0},A_{2},\dots,A_{2n}]^{\mathrm{T}} \tag{29.15.4}
$$

be the eigenvector corresponding to $H_{m}$ and normalized so that


<a id="E5"></a>
$$
\tfrac{1}{2}A_{0}^{2}+\sum_{p=1}^{n}A_{2p}^{2}=1 \tag{29.15.5}
$$

and


<a id="E6"></a>
$$
\tfrac{1}{2}A_{0}+\sum_{p=1}^{n}A_{2p}>0. \tag{29.15.6}
$$

Then


<a id="E7"></a>
$$
a^{2m}_{\nu}\left(k^{2}\right)=\tfrac{1}{2}(H_{m}+\nu(\nu+1)k^{2}), \tag{29.15.7}
$$

and ( 29.15.1 ) applies, with $\phi$ again defined as in ( 29.2.5 ).


### Polynomial ğ‘ ğ¸2â¢n+1mâ¡(z,k2)

:::{note}
**See also:**

Annotations for Â§29.15(i) , Â§29.15 and Ch.29
:::

When $\nu=2n+1$ , $m=0,1,\dots,n$ , the Fourier series ( 29.6.16 ) terminates:


<a id="E8"></a>
$$
\mathit{sE}^{m}_{2n+1}\left(z,k^{2}\right)=\sum_{p=0}^{n}A_{2p+1}\cos\left((2p+1)\phi\right). \tag{29.15.8}
$$

In ( 29.15.2 ) replace $\alpha_{p}$ , $\beta_{p}$ , and $\gamma_{p}$ as in ( 29.3.13 ), ( 29.3.14 ). Also, replace ( 29.15.4 ), ( 29.15.5 ), ( 29.15.6 ) by


<a id="E9"></a>
$$
[A_{1},A_{3},\dots,A_{2n+1}]^{\mathrm{T}}, \tag{29.15.9}
$$


<a id="E10"></a>
$$
\sum_{p=0}^{n}A_{2p+1}^{2}=1, \tag{29.15.10}
$$


<a id="E11"></a>
$$
\sum_{p=0}^{n}A_{2p+1}>0. \tag{29.15.11}
$$

Then


<a id="E12"></a>
$$
a^{2m+1}_{\nu}\left(k^{2}\right)=\tfrac{1}{2}(H_{m}+\nu(\nu+1)k^{2}), \tag{29.15.12}
$$

and ( 29.15.8 ) applies.


### Polynomial ğ‘ğ¸2â¢n+1mâ¡(z,k2)

:::{note}
**See also:**

Annotations for Â§29.15(i) , Â§29.15 and Ch.29
:::

When $\nu=2n+1$ , $m=0,1,\dots,n$ , the Fourier series ( 29.6.31 ) terminates:


<a id="E13"></a>
$$
\mathit{cE}^{m}_{2n+1}\left(z,k^{2}\right)=\sum_{p=0}^{n}B_{2p+1}\sin\left((2p+1)\phi\right). \tag{29.15.13}
$$

In ( 29.15.2 ) replace $\alpha_{p}$ , $\beta_{p}$ , and $\gamma_{p}$ as in ( 29.3.15 ), ( 29.3.16 ). Also, replace ( 29.15.4 ), ( 29.15.5 ), ( 29.15.6 ) by


<a id="E14"></a>
$$
[B_{1},B_{3},\dots,B_{2n+1}]^{\mathrm{T}}, \tag{29.15.14}
$$


<a id="E15"></a>
$$
\sum_{p=0}^{n}B_{2p+1}^{2}=1, \tag{29.15.15}
$$


<a id="E16"></a>
$$
\sum_{p=0}^{n}(2p+1)B_{2p+1}>0. \tag{29.15.16}
$$

Then


<a id="E17"></a>
$$
b^{2m+1}_{\nu}\left(k^{2}\right)=\tfrac{1}{2}(H_{m}+\nu(\nu+1)k^{2}), \tag{29.15.17}
$$

and ( 29.15.13 ) applies.


### Polynomial ğ‘‘ğ¸2â¢n+1mâ¡(z,k2)

:::{note}
**See also:**

Annotations for Â§29.15(i) , Â§29.15 and Ch.29
:::

When $\nu=2n+1$ , $m=0,1,\dots,n$ , the Fourier series ( 29.6.8 ) terminates:


<a id="E18"></a>
$$
\mathit{dE}^{m}_{2n+1}\left(z,k^{2}\right)=\operatorname{dn}\left(z,k\right)\left(\tfrac{1}{2}C_{0}+\sum_{p=1}^{n}C_{2p}\cos\left(2p\phi\right)\right). \tag{29.15.18}
$$

In ( 29.15.2 ) replace $\alpha_{p}$ , $\beta_{p}$ , and $\gamma_{p}$ as in ( 29.6.11 ). Also, replace ( 29.15.4 ), ( 29.15.5 ), ( 29.15.6 ) by


<a id="E19"></a>
$$
[C_{0},C_{2},\dots,C_{2n}]^{\mathrm{T}}, \tag{29.15.19}
$$


<a id="E20"></a>
$$
\left(1-\tfrac{1}{2}k^{2}\right)\left(\tfrac{1}{2}C_{0}^{2}+\sum_{p=1}^{n}C_{2p}^{2}\right)-\tfrac{1}{2}k^{2}\sum_{p=0}^{n-1}C_{2p}C_{2p+2}=1, \tag{29.15.20}
$$


<a id="E21"></a>
$$
\tfrac{1}{2}C_{0}+\sum_{p=1}^{n}C_{2p}>0. \tag{29.15.21}
$$

Then


<a id="E22"></a>
$$
a^{2m}_{\nu}\left(k^{2}\right)=\tfrac{1}{2}(H_{m}+\nu(\nu+1)k^{2}), \tag{29.15.22}
$$

and ( 29.15.18 ) applies.


### Polynomial ğ‘ ğ‘ğ¸2â¢n+2mâ¡(z,k2)

:::{note}
**See also:**

Annotations for Â§29.15(i) , Â§29.15 and Ch.29
:::

When $\nu=2n+2$ , $m=0,1,\dots,n$ , the Fourier series ( 29.6.46 ) terminates:


<a id="E23"></a>
$$
\mathit{scE}^{m}_{2n+2}\left(z,k^{2}\right)=\sum_{p=0}^{n}B_{2p+2}\sin\left((2p+2)\phi\right). \tag{29.15.23}
$$

In ( 29.15.2 ) replace $\alpha_{p}$ , $\beta_{p}$ , and $\gamma_{p}$ as in ( 29.3.17 ). Also replace ( 29.15.4 ), ( 29.15.5 ), ( 29.15.6 ) by


<a id="E24"></a>
$$
[B_{2},B_{4},\dots,B_{2n+2}]^{\mathrm{T}}, \tag{29.15.24}
$$


<a id="E25"></a>
$$
\sum_{p=0}^{n}B_{2p+2}^{2}=1, \tag{29.15.25}
$$


<a id="E26"></a>
$$
\sum_{p=0}^{n}(2p+2)B_{2p+2}>0. \tag{29.15.26}
$$

Then


<a id="E27"></a>
$$
b^{2m+2}_{\nu}\left(k^{2}\right)=\tfrac{1}{2}(H_{m}+\nu(\nu+1)k^{2}), \tag{29.15.27}
$$

and ( 29.15.23 ) applies.


### Polynomial ğ‘ ğ‘‘ğ¸2â¢n+2mâ¡(z,k2)

:::{note}
**See also:**

Annotations for Â§29.15(i) , Â§29.15 and Ch.29
:::

When $\nu=2n+2$ , $m=0,1,\dots,n$ , the Fourier series ( 29.6.23 ) terminates:


<a id="E28"></a>
$$
\mathit{sdE}^{m}_{2n+2}\left(z,k^{2}\right)=\operatorname{dn}\left(z,k\right)\sum_{p=0}^{n}C_{2p+1}\cos\left((2p+1)\phi\right). \tag{29.15.28}
$$

In ( 29.15.2 ) replace $\alpha_{p}$ , $\beta_{p}$ , and $\gamma_{p}$ as in ( 29.6.26 ). Also replace ( 29.15.4 ), ( 29.15.5 ), ( 29.15.6 ) by


<a id="E29"></a>
$$
[C_{1},C_{3},\dots,C_{2n+1}]^{\mathrm{T}}, \tag{29.15.29}
$$


<a id="E30"></a>
$$
\left(1-\tfrac{1}{2}k^{2}\right)\sum_{p=0}^{n}C_{2p+1}^{2}-{\tfrac{1}{2}k^{2}\left(\tfrac{1}{2}C_{1}^{2}+\sum_{p=0}^{n-1}C_{2p+1}C_{2p+3}\right)=1}, \tag{29.15.30}
$$


<a id="E31"></a>
$$
\sum_{p=0}^{n}C_{2p+1}>0. \tag{29.15.31}
$$

Then


<a id="E32"></a>
$$
a^{2m+1}_{\nu}\left(k^{2}\right)=\tfrac{1}{2}(H_{m}+\nu(\nu+1)k^{2}), \tag{29.15.32}
$$

and ( 29.15.28 ) applies.


### Polynomial ğ‘ğ‘‘ğ¸2â¢n+2mâ¡(z,k2)

:::{note}
**See also:**

Annotations for Â§29.15(i) , Â§29.15 and Ch.29
:::

When $\nu=2n+2$ , $m=0,1,\dots,n$ , the Fourier series ( 29.6.38 ) terminates:


<a id="E33"></a>
$$
\mathit{cdE}^{m}_{2n+2}\left(z,k^{2}\right)=\operatorname{dn}\left(z,k\right)\sum_{p=0}^{n}D_{2p+1}\sin\left((2p+1)\phi\right). \tag{29.15.33}
$$

In ( 29.15.2 ) replace $\alpha_{p}$ , $\beta_{p}$ , and $\gamma_{p}$ as in ( 29.6.41 ). Also replace ( 29.15.4 ), ( 29.15.5 ), ( 29.15.6 ) by


<a id="E34"></a>
$$
[D_{1},D_{3},\dots,D_{2n+1}]^{\mathrm{T}}, \tag{29.15.34}
$$


<a id="E35"></a>
$$
\left(1-\tfrac{1}{2}k^{2}\right)\sum_{p=0}^{n}D_{2p+1}^{2}+{\tfrac{1}{2}k^{2}\left(\tfrac{1}{2}D_{1}^{2}-\sum_{p=0}^{n-1}D_{2p+1}D_{2p+3}\right)=1}, \tag{29.15.35}
$$


<a id="E36"></a>
$$
\sum_{p=0}^{n}(2p+1)D_{2p+1}>0. \tag{29.15.36}
$$

Then


<a id="E37"></a>
$$
b^{2m+1}_{\nu}\left(k^{2}\right)=\tfrac{1}{2}(H_{m}+\nu(\nu+1)k^{2}), \tag{29.15.37}
$$

and ( 29.15.33 ) applies.


### Polynomial ğ‘ ğ‘ğ‘‘ğ¸2â¢n+3mâ¡(z,k2)

:::{note}
**See also:**

Annotations for Â§29.15(i) , Â§29.15 and Ch.29
:::

When $\nu=2n+3$ , $m=0,1,\dots,n$ , the Fourier series ( 29.6.53 ) terminates:


<a id="E38"></a>
$$
\mathit{scdE}^{m}_{2n+3}\left(z,k^{2}\right)=\operatorname{dn}\left(z,k\right)\sum_{p=0}^{n}D_{2p+2}\sin\left((2p+2)\phi\right). \tag{29.15.38}
$$

In ( 29.15.2 ) replace $\alpha_{p}$ , $\beta_{p}$ , and $\gamma_{p}$ as in ( 29.6.56 ). Also replace ( 29.15.4 ), ( 29.15.5 ), ( 29.15.6 ) by


<a id="E39"></a>
$$
[D_{2},D_{4},\dots,D_{2n+2}]^{\mathrm{T}}, \tag{29.15.39}
$$


<a id="E40"></a>
$$
\left(1-\tfrac{1}{2}k^{2}\right)\sum_{p=0}^{n}D_{2p+2}^{2}-\tfrac{1}{2}k^{2}\sum_{p=1}^{n}D_{2p}D_{2p+2}=1, \tag{29.15.40}
$$


<a id="E41"></a>
$$
\sum_{p=0}^{n}(2p+2)D_{2p+2}>0. \tag{29.15.41}
$$

Then


<a id="E42"></a>
$$
b^{2m+2}_{\nu}\left(k^{2}\right)=\tfrac{1}{2}(H_{m}+\nu(\nu+1)k^{2}), \tag{29.15.42}
$$

and ( 29.15.38 ) applies.


## Â§29.15(ii) Chebyshev Series

:::{note}
**Keywords:**

[Chebyshev series](http://dlmf.nist.gov/search/search?q=Chebyshev%20series) , [LamÃ© polynomials](http://dlmf.nist.gov/search/search?q=Lam%C3%A9%20polynomials) , [explicit formulas](http://dlmf.nist.gov/search/search?q=explicit%20formulas)

**Notes:**

See Arscott ([1964b](./bib/index.html#bib142 "Periodic Differential Equations. An Introduction to Mathieu, LamÃ©, and Allied Functions"), Â§9.6.2) and Ince ([1940a](./bib/I.html#bib1128 "The periodic LamÃ© functions")).

**Referenced by:**

Â§29.12(i)

**See also:**

Annotations for Â§29.15 and Ch.29
:::

The Chebyshev polynomial $T$ of the first kind (Â§ [18.3](./18.3.md "Â§18.3 Definitions â€£ Classical Orthogonal Polynomials â€£ Chapter 18 Orthogonal Polynomials") ) satisfies $\cos\left(p\phi\right)=T_{p}\left(\cos\phi\right)$ . Since ( 29.2.5 ) implies that $\cos\phi=\operatorname{sn}\left(z,k\right)$ , ( 29.15.1 ) can be rewritten in the form


<a id="E43"></a>
$$
\mathit{uE}^{m}_{2n}\left(z,k^{2}\right)=\tfrac{1}{2}A_{0}+\sum_{p=1}^{n}A_{2p}T_{2p}\left(\operatorname{sn}\left(z,k\right)\right). \tag{29.15.43}
$$

This determines the polynomial $P$ of degree $n$ for which $\mathit{uE}^{m}_{2n}\left(z,k^{2}\right)=P({\operatorname{sn}}^{2}\left(z,k\right))$ ; compare Table 29.12.1 . The set of coefficients of this polynomial (without normalization) can also be found directly as an eigenvector of an $(n+1)\times(n+1)$ tridiagonal matrix; see Arscott and Khabaza ([1962](./bib/index.html#bib145 "Tables of LamÃ© Polynomials")).

Using also $\sin\left((p+1)\phi\right)=(\sin\phi)U_{p}\left(\cos\phi\right)$ , with $U$ denoting the Chebyshev polynomial of the second kind (Â§ [18.3](./18.3.md "Â§18.3 Definitions â€£ Classical Orthogonal Polynomials â€£ Chapter 18 Orthogonal Polynomials") ), we obtain

<a id="EGx1"></a>

$$
\displaystyle\mathit{sE}^{m}_{2n+1}\left(z,k^{2}\right) \displaystyle=\sum_{p=0}^{n}A_{2p+1}T_{2p+1}\left(\operatorname{sn}\left(z,k\right)\right), \tag{29.15.44}
$$

:::{note}
**Symbols:**

$T_{\NVar{n}}\left(\NVar{x}\right)$: Chebyshev polynomial of the first kind , $\operatorname{sn}\left(\NVar{z},\NVar{k}\right)$: Jacobian elliptic function , $\mathit{sE}^{\NVar{m}}_{2\NVar{n}+1}\left(\NVar{z},\NVar{k^{2}}\right)$: LamÃ© polynomial , $m$: nonnegative integer , $n$: nonnegative integer , $p$: nonnegative integer , $z$: complex variable , $k$: real parameter and $A_{2p}$: coefficients

**See also:**

Annotations for Â§29.15(ii) , Â§29.15 and Ch.29
:::

$$
\displaystyle\mathit{cE}^{m}_{2n+1}\left(z,k^{2}\right) \displaystyle=\operatorname{cn}\left(z,k\right)\sum_{p=0}^{n}B_{2p+1}U_{2p}\left(\operatorname{sn}\left(z,k\right)\right), \tag{29.15.45}
$$

:::{note}
**Symbols:**

$U_{\NVar{n}}\left(\NVar{x}\right)$: Chebyshev polynomial of the second kind , $\operatorname{cn}\left(\NVar{z},\NVar{k}\right)$: Jacobian elliptic function , $\operatorname{sn}\left(\NVar{z},\NVar{k}\right)$: Jacobian elliptic function , $\mathit{cE}^{\NVar{m}}_{2\NVar{n}+1}\left(\NVar{z},\NVar{k^{2}}\right)$: LamÃ© polynomial , $m$: nonnegative integer , $n$: nonnegative integer , $p$: nonnegative integer , $z$: complex variable , $k$: real parameter and $B_{2p+1}$: coefficents

**See also:**

Annotations for Â§29.15(ii) , Â§29.15 and Ch.29
:::

$$
\displaystyle\mathit{dE}^{m}_{2n+1}\left(z,k^{2}\right) \displaystyle=\operatorname{dn}\left(z,k\right)\left(\tfrac{1}{2}C_{0}+\sum_{p=1}^{n}C_{2p}T_{2p}\left(\operatorname{sn}\left(z,k\right)\right)\right), \tag{29.15.46}
$$

:::{note}
**Symbols:**

$T_{\NVar{n}}\left(\NVar{x}\right)$: Chebyshev polynomial of the first kind , $\operatorname{dn}\left(\NVar{z},\NVar{k}\right)$: Jacobian elliptic function , $\operatorname{sn}\left(\NVar{z},\NVar{k}\right)$: Jacobian elliptic function , $\mathit{dE}^{\NVar{m}}_{2\NVar{n}+1}\left(\NVar{z},\NVar{k^{2}}\right)$: LamÃ© polynomial , $m$: nonnegative integer , $n$: nonnegative integer , $p$: nonnegative integer , $z$: complex variable , $k$: real parameter and $C_{2p}$: coefficents

**See also:**

Annotations for Â§29.15(ii) , Â§29.15 and Ch.29
:::

$$
\displaystyle\mathit{scE}^{m}_{2n+2}\left(z,k^{2}\right) \displaystyle=\operatorname{cn}\left(z,k\right)\sum_{p=0}^{n}B_{2p+2}U_{2p+1}\left(\operatorname{sn}\left(z,k\right)\right), \tag{29.15.47}
$$

:::{note}
**Symbols:**

$U_{\NVar{n}}\left(\NVar{x}\right)$: Chebyshev polynomial of the second kind , $\operatorname{cn}\left(\NVar{z},\NVar{k}\right)$: Jacobian elliptic function , $\operatorname{sn}\left(\NVar{z},\NVar{k}\right)$: Jacobian elliptic function , $\mathit{scE}^{\NVar{m}}_{2\NVar{n}+2}\left(\NVar{z},\NVar{k^{2}}\right)$: LamÃ© polynomial , $m$: nonnegative integer , $n$: nonnegative integer , $p$: nonnegative integer , $z$: complex variable , $k$: real parameter and $B_{2p+1}$: coefficents

**See also:**

Annotations for Â§29.15(ii) , Â§29.15 and Ch.29
:::

$$
\displaystyle\mathit{sdE}^{m}_{2n+2}\left(z,k^{2}\right) \displaystyle=\operatorname{dn}\left(z,k\right)\sum_{p=0}^{n}C_{2p+1}T_{2p+1}\left(\operatorname{sn}\left(z,k\right)\right), \tag{29.15.48}
$$

:::{note}
**Symbols:**

$T_{\NVar{n}}\left(\NVar{x}\right)$: Chebyshev polynomial of the first kind , $\operatorname{dn}\left(\NVar{z},\NVar{k}\right)$: Jacobian elliptic function , $\operatorname{sn}\left(\NVar{z},\NVar{k}\right)$: Jacobian elliptic function , $\mathit{sdE}^{\NVar{m}}_{2\NVar{n}+2}\left(\NVar{z},\NVar{k^{2}}\right)$: LamÃ© polynomial , $m$: nonnegative integer , $n$: nonnegative integer , $p$: nonnegative integer , $z$: complex variable , $k$: real parameter and $C_{2p+1}$: coefficents

**See also:**

Annotations for Â§29.15(ii) , Â§29.15 and Ch.29
:::

$$
\displaystyle\mathit{cdE}^{m}_{2n+2}\left(z,k^{2}\right) \displaystyle=\operatorname{cn}\left(z,k\right)\operatorname{dn}\left(z,k\right)\sum_{p=0}^{n}D_{2p+1}U_{2p}\left(\operatorname{sn}\left(z,k\right)\right), \tag{29.15.49}
$$

:::{note}
**Symbols:**

$U_{\NVar{n}}\left(\NVar{x}\right)$: Chebyshev polynomial of the second kind , $\operatorname{cn}\left(\NVar{z},\NVar{k}\right)$: Jacobian elliptic function , $\operatorname{dn}\left(\NVar{z},\NVar{k}\right)$: Jacobian elliptic function , $\operatorname{sn}\left(\NVar{z},\NVar{k}\right)$: Jacobian elliptic function , $\mathit{cdE}^{\NVar{m}}_{2\NVar{n}+2}\left(\NVar{z},\NVar{k^{2}}\right)$: LamÃ© polynomial , $m$: nonnegative integer , $n$: nonnegative integer , $p$: nonnegative integer , $z$: complex variable , $k$: real parameter and $D_{2p}$: coefficents

**See also:**

Annotations for Â§29.15(ii) , Â§29.15 and Ch.29
:::

$$
\displaystyle\mathit{scdE}^{m}_{2n+3}\left(z,k^{2}\right) \displaystyle=\operatorname{cn}\left(z,k\right)\operatorname{dn}\left(z,k\right)\sum_{p=0}^{n}D_{2p+2}U_{2p+1}\left(\operatorname{sn}\left(z,k\right)\right). \tag{29.15.50}
$$

:::{note}
**Symbols:**

$U_{\NVar{n}}\left(\NVar{x}\right)$: Chebyshev polynomial of the second kind , $\operatorname{cn}\left(\NVar{z},\NVar{k}\right)$: Jacobian elliptic function , $\operatorname{dn}\left(\NVar{z},\NVar{k}\right)$: Jacobian elliptic function , $\operatorname{sn}\left(\NVar{z},\NVar{k}\right)$: Jacobian elliptic function , $\mathit{scdE}^{\NVar{m}}_{2\NVar{n}+3}\left(\NVar{z},\NVar{k^{2}}\right)$: LamÃ© polynomial , $m$: nonnegative integer , $n$: nonnegative integer , $p$: nonnegative integer , $z$: complex variable , $k$: real parameter and $D_{2p+1}$: coefficents

**See also:**

Annotations for Â§29.15(ii) , Â§29.15 and Ch.29
:::

For explicit formulas for LamÃ© polynomials of low degree, see Arscott ([1964b](./bib/index.html#bib142 "Periodic Differential Equations. An Introduction to Mathieu, LamÃ©, and Allied Functions"), p. 205).
