# ¬ß29.6 Fourier Series

:::{note}
**Keywords:**

[Fourier series](http://dlmf.nist.gov/search/search?q=Fourier%20series) , [Lam√© functions](http://dlmf.nist.gov/search/search?q=Lam%C3%A9%20functions)

**Referenced by:**

¬ß29.15(i) , 2nd item , ¬ß29.3(vi)

**See also:**

Annotations for Ch.29
:::


## ¬ß29.6(i) Function ùê∏ùëêŒΩ2‚Å¢m‚Å°(z,k2)

:::{note}
**Keywords:**

[Lam√© functions](http://dlmf.nist.gov/search/search?q=Lam%C3%A9%20functions) , [Lam√© polynomials](http://dlmf.nist.gov/search/search?q=Lam%C3%A9%20polynomials) , [relation to Lam√© functions](http://dlmf.nist.gov/search/search?q=relation%20to%20Lam%C3%A9%20functions) , [relations to Lam√© polynomials](http://dlmf.nist.gov/search/search?q=relations%20to%20Lam%C3%A9%20polynomials)

**Notes:**

See Erd√©lyi et al. ([1955](./bib/E.html#bib755 "Higher Transcendental Functions. Vol. III"), ¬ß15.5.1) and Ince ([1940b](./bib/I.html#bib1127 "Further investigations into the periodic Lam√© functions")). The normalization formula ( 29.6.5 ) is adopted from Jansen ([1977](./bib/J.html#bib1162 "Simple-periodic and Non-periodic Lam√© Functions")).

**See also:**

Annotations for ¬ß29.6 and Ch.29
:::

With $\phi=\frac{1}{2}\pi-\operatorname{am}\left(z,k\right)$ , as in ( 29.2.5 ), we have


<a id="E1"></a>
$$
\mathit{Ec}^{2m}_{\nu}\left(z,k^{2}\right)=\tfrac{1}{2}A_{0}+\sum_{p=1}^{\infty}A_{2p}\cos\left(2p\phi\right). \tag{29.6.1}
$$

Here


<a id="E2"></a>
$$
H=2a^{2m}_{\nu}\left(k^{2}\right)-\nu(\nu+1)k^{2}, \tag{29.6.2}
$$


<a id="E3"></a>
$$
(\beta_{0}-H)A_{0}+\alpha_{0}A_{2}=0, \tag{29.6.3}
$$


<a id="E4"></a>
$$
\gamma_{p}A_{2p-2}+(\beta_{p}-H)A_{2p}+\alpha_{p}A_{2p+2}=0, \tag{29.6.4}
$$

with $\alpha_{p}$ , $\beta_{p}$ , and $\gamma_{p}$ as in ( 29.3.11 ) and ( 29.3.12 ), and


<a id="E5"></a>
$$
\tfrac{1}{2}A_{0}^{2}+\sum_{p=1}^{\infty}A_{2p}^{2}=1, \tag{29.6.5}
$$


<a id="E6"></a>
$$
\tfrac{1}{2}A_{0}+\sum_{p=1}^{\infty}A_{2p}>0. \tag{29.6.6}
$$

When $\nu\neq 2n$ , where $n$ is a nonnegative integer, it follows from ¬ß 2.9(i) that for any value of $H$ the system ( 29.6.4 )‚Äì( 29.6.6 ) has a unique recessive solution $A_{0},A_{2},A_{4},\dots$ ; furthermore


<a id="E7"></a>
$$
\lim_{p\to\infty}\frac{A_{2p+2}}{A_{2p}}=\frac{k^{2}}{(1+k^{\prime})^{2}}, \tag{29.6.7}
$$

In addition, if $H$ satisfies ( 29.6.2 ), then ( 29.6.3 ) applies.

In the special case $\nu=2n$ , $m=0,1,\dots,n$ , there is a unique nontrivial solution with the property $A_{2p}=0$ , $p=n+1,n+2,\dots$ . This solution can be constructed from ( 29.6.4 ) by backward recursion, starting with $A_{2n+2}=0$ and an arbitrary nonzero value of $A_{2n}$ , followed by normalization via ( 29.6.5 ) and ( 29.6.6 ). Consequently, $\mathit{Ec}^{2m}_{\nu}\left(z,k^{2}\right)$ reduces to a Lam√© polynomial; compare ¬ß¬ß 29.12(i) and 29.15(i) .

An alternative version of the Fourier series expansion ( 29.6.1 ) is given by


<a id="E8"></a>
$$
\mathit{Ec}^{2m}_{\nu}\left(z,k^{2}\right)=\operatorname{dn}\left(z,k\right)\left(\tfrac{1}{2}C_{0}+\sum_{p=1}^{\infty}C_{2p}\cos\left(2p\phi\right)\right). \tag{29.6.8}
$$

Here $\operatorname{dn}\left(z,k\right)$ is as in ¬ß [22.2](./22.2.md "¬ß22.2 Definitions ‚Ä£ Properties ‚Ä£ Chapter 22 Jacobian Elliptic Functions") , and


<a id="E9"></a>
$$
(\beta_{0}-H)C_{0}+\alpha_{0}C_{2}=0, \tag{29.6.9}
$$


<a id="E10"></a>
$$
\gamma_{p}C_{2p-2}+(\beta_{p}-H)C_{2p}+\alpha_{p}C_{2p+2}=0, \tag{29.6.10}
$$

with $\alpha_{p},\beta_{p}$ , and $\gamma_{p}$ now defined by

<a id="E11"></a>

<a id="Ex1"></a>
$$
\displaystyle\alpha_{p} \displaystyle=\begin{cases}\nu(\nu+1)k^{2},&p=0,\\
\frac{1}{2}(\nu-2p)(\nu+2p+1)k^{2},&p\geq 1,\end{cases} \tag{29.6.11}
$$

<a id="Ex2"></a>
$$
\displaystyle\beta_{p} \displaystyle=4p^{2}(2-k^{2}),
$$

<a id="Ex3"></a>
$$
\displaystyle\gamma_{p} \displaystyle=\tfrac{1}{2}(\nu-2p+1)(\nu+2p)k^{2},
$$

:::{note}
**Symbols:**

$p$: nonnegative integer , $k$: real parameter , $\nu$: real parameter , $\alpha_{p}$ , $\beta_{p}$ and $\gamma_{p}$

**Referenced by:**

¬ß29.15(i)

**See also:**

Annotations for ¬ß29.6(i) , ¬ß29.6 and Ch.29
:::

and


<a id="E12"></a>
$$
\left(1-\tfrac{1}{2}k^{2}\right)\left(\tfrac{1}{2}C_{0}^{2}+\sum_{p=1}^{\infty}C_{2p}^{2}\right)-\tfrac{1}{2}k^{2}\sum_{p=0}^{\infty}C_{2p}C_{2p+2}=1, \tag{29.6.12}
$$


<a id="E13"></a>
$$
\tfrac{1}{2}C_{0}+\sum_{p=1}^{\infty}C_{2p}>0, \tag{29.6.13}
$$


<a id="E14"></a>
$$
\lim_{p\to\infty}\frac{C_{2p+2}}{C_{2p}}=\frac{k^{2}}{(1+k^{\prime})^{2}}, \tag{29.6.14}
$$


<a id="E15"></a>
$$
\tfrac{1}{2}A_{0}C_{0}+\sum_{p=1}^{\infty}A_{2p}C_{2p}=\frac{4}{\pi}\int_{0}^{K}\left(\mathit{Ec}^{2m}_{\nu}\left(x,k^{2}\right)\right)^{2}\,\mathrm{d}x. \tag{29.6.15}
$$


## ¬ß29.6(ii) Function ùê∏ùëêŒΩ2‚Å¢m+1‚Å°(z,k2)

:::{note}
**Notes:**

See Erd√©lyi et al. ([1955](./bib/E.html#bib755 "Higher Transcendental Functions. Vol. III"), ¬ß15.5.1) and Ince ([1940b](./bib/I.html#bib1127 "Further investigations into the periodic Lam√© functions")). The normalization formula ( 29.6.20 ) is adopted from Jansen ([1977](./bib/J.html#bib1162 "Simple-periodic and Non-periodic Lam√© Functions")).

**See also:**

Annotations for ¬ß29.6 and Ch.29
:::


<a id="E16"></a>
$$
\mathit{Ec}^{2m+1}_{\nu}\left(z,k^{2}\right)=\sum_{p=0}^{\infty}A_{2p+1}\cos\left((2p+1)\phi\right). \tag{29.6.16}
$$

Here


<a id="E17"></a>
$$
H=2a^{2m+1}_{\nu}\left(k^{2}\right)-\nu(\nu+1)k^{2}, \tag{29.6.17}
$$


<a id="E18"></a>
$$
(\beta_{0}-H)A_{1}+\alpha_{0}A_{3}=0, \tag{29.6.18}
$$


<a id="E19"></a>
$$
\gamma_{p}A_{2p-1}+(\beta_{p}-H)A_{2p+1}+\alpha_{p}A_{2p+3}=0, \tag{29.6.19}
$$

with $\alpha_{p}$ , $\beta_{p}$ , and $\gamma_{p}$ as in ( 29.3.13 ) and ( 29.3.14 ), and


<a id="E20"></a>
$$
\sum_{p=0}^{\infty}A_{2p+1}^{2}=1, \tag{29.6.20}
$$


<a id="E21"></a>
$$
\sum_{p=0}^{\infty}A_{2p+1}>0, \tag{29.6.21}
$$


<a id="E22"></a>
$$
\lim_{p\to\infty}\frac{A_{2p+1}}{A_{2p-1}}=\frac{k^{2}}{(1+k^{\prime})^{2}}, \tag{29.6.22}
$$

Also,


<a id="E23"></a>
$$
\mathit{Ec}^{2m+1}_{\nu}\left(z,k^{2}\right)=\operatorname{dn}\left(z,k\right)\sum_{p=0}^{\infty}C_{2p+1}\cos\left((2p+1)\phi\right), \tag{29.6.23}
$$

where


<a id="E24"></a>
$$
(\beta_{0}-H)C_{1}+\alpha_{0}C_{3}=0, \tag{29.6.24}
$$


<a id="E25"></a>
$$
\gamma_{p}C_{2p-1}+(\beta_{p}-H)C_{2p+1}+\alpha_{p}C_{2p+3}=0, \tag{29.6.25}
$$

with

<a id="E26"></a>

<a id="Ex4"></a>
$$
\displaystyle\alpha_{p} \displaystyle=\tfrac{1}{2}(\nu-2p-1)(\nu+2p+2)k^{2}, \tag{29.6.26}
$$

<a id="Ex5"></a>
$$
\displaystyle\beta_{p} \displaystyle=\begin{cases}2-k^{2}+\frac{1}{2}\nu(\nu+1)k^{2},&p=0,\\
(2p+1)^{2}(2-k^{2}),&p\geq 1,\end{cases}
$$

<a id="Ex6"></a>
$$
\displaystyle\gamma_{p} \displaystyle=\tfrac{1}{2}(\nu-2p)(\nu+2p+1)k^{2},
$$

:::{note}
**Symbols:**

$p$: nonnegative integer , $k$: real parameter , $\nu$: real parameter , $\alpha_{p}$ , $\beta_{p}$ and $\gamma_{p}$

**Referenced by:**

¬ß29.15(i)

**See also:**

Annotations for ¬ß29.6(ii) , ¬ß29.6 and Ch.29
:::

and


<a id="E27"></a>
$$
\left(1-\tfrac{1}{2}k^{2}\right)\sum_{p=0}^{\infty}C_{2p+1}^{2}-{\tfrac{1}{2}k^{2}\left(\tfrac{1}{2}C_{1}^{2}+\sum_{p=0}^{\infty}C_{2p+1}C_{2p+3}\right)=1}, \tag{29.6.27}
$$


<a id="E28"></a>
$$
\sum_{p=0}^{\infty}C_{2p+1}>0, \tag{29.6.28}
$$


<a id="E29"></a>
$$
\lim_{p\to\infty}\frac{C_{2p+1}}{C_{2p-1}}=\frac{k^{2}}{(1+k^{\prime})^{2}}, \tag{29.6.29}
$$


<a id="E30"></a>
$$
\sum_{p=0}^{\infty}A_{2p+1}C_{2p+1}=\frac{4}{\pi}\int_{0}^{K}\left(\mathit{Ec}^{2m+1}_{\nu}\left(x,k^{2}\right)\right)^{2}\,\mathrm{d}x. \tag{29.6.30}
$$


## ¬ß29.6(iii) Function ùê∏ùë†ŒΩ2‚Å¢m+1‚Å°(z,k2)

:::{note}
**Notes:**

See Erd√©lyi et al. ([1955](./bib/E.html#bib755 "Higher Transcendental Functions. Vol. III"), ¬ß15.5.1) and Ince ([1940b](./bib/I.html#bib1127 "Further investigations into the periodic Lam√© functions")). The normalization formula ( 29.6.35 ) is adopted from Jansen ([1977](./bib/J.html#bib1162 "Simple-periodic and Non-periodic Lam√© Functions")).

**See also:**

Annotations for ¬ß29.6 and Ch.29
:::


<a id="E31"></a>
$$
\mathit{Es}^{2m+1}_{\nu}\left(z,k^{2}\right)=\sum_{p=0}^{\infty}B_{2p+1}\sin\left((2p+1)\phi\right). \tag{29.6.31}
$$

Here


<a id="E32"></a>
$$
H=2b^{2m+1}_{\nu}\left(k^{2}\right)-\nu(\nu+1)k^{2}, \tag{29.6.32}
$$


<a id="E33"></a>
$$
(\beta_{0}-H)B_{1}+\alpha_{0}B_{3}=0, \tag{29.6.33}
$$


<a id="E34"></a>
$$
\gamma_{p}B_{2p-1}+(\beta_{p}-H)B_{2p+1}+\alpha_{p}B_{2p+3}=0, \tag{29.6.34}
$$

with $\alpha_{p}$ , $\beta_{p}$ , and $\gamma_{p}$ as in ( 29.3.15 ), ( 29.3.16 ), and


<a id="E35"></a>
$$
\sum_{p=0}^{\infty}B_{2p+1}^{2}=1, \tag{29.6.35}
$$


<a id="E36"></a>
$$
\sum_{p=0}^{\infty}(2p+1)B_{2p+1}>0, \tag{29.6.36}
$$


<a id="E37"></a>
$$
\lim_{p\to\infty}\frac{B_{2p+1}}{B_{2p-1}}=\frac{k^{2}}{(1+k^{\prime})^{2}}, \tag{29.6.37}
$$

Also,


<a id="E38"></a>
$$
\mathit{Es}^{2m+1}_{\nu}\left(z,k^{2}\right)=\operatorname{dn}\left(z,k\right)\sum_{p=0}^{\infty}D_{2p+1}\sin\left((2p+1)\phi\right), \tag{29.6.38}
$$

where


<a id="E39"></a>
$$
(\beta_{0}-H)D_{1}+\alpha_{0}D_{3}=0, \tag{29.6.39}
$$


<a id="E40"></a>
$$
\gamma_{p}D_{2p-1}+(\beta_{p}-H)D_{2p+1}+\alpha_{p}D_{2p+3}=0, \tag{29.6.40}
$$

with

<a id="E41"></a>

<a id="Ex7"></a>
$$
\displaystyle\alpha_{p} \displaystyle=\tfrac{1}{2}(\nu-2p-1)(\nu+2p+2)k^{2}, \tag{29.6.41}
$$

<a id="Ex8"></a>
$$
\displaystyle\beta_{p} \displaystyle=\begin{cases}2-k^{2}-\frac{1}{2}\nu(\nu+1)k^{2},&p=0,\\
(2p+1)^{2}(2-k^{2}),&p\geq 1,\end{cases}
$$

<a id="Ex9"></a>
$$
\displaystyle\gamma_{p} \displaystyle=\tfrac{1}{2}(\nu-2p)(\nu+2p+1)k^{2},
$$

:::{note}
**Symbols:**

$p$: nonnegative integer , $k$: real parameter , $\nu$: real parameter , $\alpha_{p}$ , $\beta_{p}$ and $\gamma_{p}$

**Referenced by:**

¬ß29.15(i)

**See also:**

Annotations for ¬ß29.6(iii) , ¬ß29.6 and Ch.29
:::

and


<a id="E42"></a>
$$
\left(1-\tfrac{1}{2}k^{2}\right)\sum_{p=0}^{\infty}D_{2p+1}^{2}+{\tfrac{1}{2}k^{2}\left(\tfrac{1}{2}D_{1}^{2}-\sum_{p=0}^{\infty}D_{2p+1}D_{2p+3}\right)=1}, \tag{29.6.42}
$$


<a id="E43"></a>
$$
\sum_{p=0}^{\infty}(2p+1)D_{2p+1}>0, \tag{29.6.43}
$$


<a id="E44"></a>
$$
\lim_{p\to\infty}\frac{D_{2p+1}}{D_{2p-1}}=\frac{k^{2}}{(1+k^{\prime})^{2}}, \tag{29.6.44}
$$


<a id="E45"></a>
$$
\sum_{p=0}^{\infty}B_{2p+1}D_{2p+1}=\frac{4}{\pi}\int_{0}^{K}\left(\mathit{Es}^{2m+1}_{\nu}\left(x,k^{2}\right)\right)^{2}\,\mathrm{d}x. \tag{29.6.45}
$$


## ¬ß29.6(iv) Function ùê∏ùë†ŒΩ2‚Å¢m+2‚Å°(z,k2)

:::{note}
**Keywords:**

[Fourier series](http://dlmf.nist.gov/search/search?q=Fourier%20series) , [Lam√© functions](http://dlmf.nist.gov/search/search?q=Lam%C3%A9%20functions)

**Notes:**

See Erd√©lyi et al. ([1955](./bib/E.html#bib755 "Higher Transcendental Functions. Vol. III"), ¬ß15.5.1) and Ince ([1940b](./bib/I.html#bib1127 "Further investigations into the periodic Lam√© functions")). The normalization formula ( 29.6.50 ) is adopted from Jansen ([1977](./bib/J.html#bib1162 "Simple-periodic and Non-periodic Lam√© Functions")).

**See also:**

Annotations for ¬ß29.6 and Ch.29
:::


<a id="E46"></a>
$$
\mathit{Es}^{2m+2}_{\nu}\left(z,k^{2}\right)=\sum_{p=1}^{\infty}B_{2p}\sin\left(2p\phi\right). \tag{29.6.46}
$$

Here


<a id="E47"></a>
$$
H=2b^{2m+2}_{\nu}\left(k^{2}\right)-\nu(\nu+1)k^{2}, \tag{29.6.47}
$$


<a id="E48"></a>
$$
(\beta_{0}-H)B_{2}+\alpha_{0}B_{4}=0, \tag{29.6.48}
$$


<a id="E49"></a>
$$
\gamma_{p}B_{2p}+(\beta_{p}-H)B_{2p+2}+\alpha_{p}B_{2p+4}=0, \tag{29.6.49}
$$

with $\alpha_{p}$ , $\beta_{p}$ , and $\gamma_{p}$ as in ( 29.3.17 ), and


<a id="E50"></a>
$$
\sum_{p=1}^{\infty}B_{2p}^{2}=1, \tag{29.6.50}
$$


<a id="E51"></a>
$$
\sum_{p=0}^{\infty}(2p+2)B_{2p+2}>0, \tag{29.6.51}
$$


<a id="E52"></a>
$$
\lim_{p\to\infty}\frac{B_{2p+2}}{B_{2p}}=\frac{k^{2}}{(1+k^{\prime})^{2}}, \tag{29.6.52}
$$

Also,


<a id="E53"></a>
$$
\mathit{Es}^{2m+2}_{\nu}\left(z,k^{2}\right)=\operatorname{dn}\left(z,k\right)\sum_{p=1}^{\infty}D_{2p}\sin\left(2p\phi\right), \tag{29.6.53}
$$

where


<a id="E54"></a>
$$
(\beta_{0}-H)D_{2}+\alpha_{0}D_{4}=0, \tag{29.6.54}
$$


<a id="E55"></a>
$$
\gamma_{p}D_{2p}+(\beta_{p}-H)D_{2p+2}+\alpha_{p}D_{2p+4}=0, \tag{29.6.55}
$$

with

<a id="E56"></a>

<a id="Ex10"></a>
$$
\displaystyle\alpha_{p} \displaystyle=\tfrac{1}{2}(\nu-2p-2)(\nu+2p+3)k^{2}, \tag{29.6.56}
$$

<a id="Ex11"></a>
$$
\displaystyle\beta_{p} \displaystyle=(2p+2)^{2}(2-k^{2}),
$$

<a id="Ex12"></a>
$$
\displaystyle\gamma_{p} \displaystyle=\tfrac{1}{2}(\nu-2p-1)(\nu+2p+2)k^{2},
$$

:::{note}
**Symbols:**

$p$: nonnegative integer , $k$: real parameter , $\nu$: real parameter , $\alpha_{p}$ , $\beta_{p}$ and $\gamma_{p}$

**Referenced by:**

¬ß29.15(i)

**See also:**

Annotations for ¬ß29.6(iv) , ¬ß29.6 and Ch.29
:::

and


<a id="E57"></a>
$$
\left(1-\tfrac{1}{2}k^{2}\right)\sum_{p=1}^{\infty}D_{2p}^{2}-\tfrac{1}{2}k^{2}\sum_{p=1}^{\infty}D_{2p}D_{2p+2}=1, \tag{29.6.57}
$$


<a id="E58"></a>
$$
\sum_{p=0}^{\infty}(2p+2)D_{2p+2}>0, \tag{29.6.58}
$$


<a id="E59"></a>
$$
\lim_{p\to\infty}\frac{D_{2p+2}}{D_{2p}}=\frac{k^{2}}{(1+k^{\prime})^{2}}, \tag{29.6.59}
$$


<a id="E60"></a>
$$
\sum_{p=1}^{\infty}B_{2p}D_{2p}=\frac{4}{\pi}\int_{0}^{K}\left(\mathit{Es}^{2m+2}_{\nu}\left(x,k^{2}\right)\right)^{2}\,\mathrm{d}x. \tag{29.6.60}
$$
